PREFIX :      <http://www.example.org/>
PREFIX dct:   <http://purl.org/dc/terms/>
PREFIX checks: <https://data.digichecks.eu/def/>
PREFIX geo:   <http://www.opengis.net/ont/geosparql#>
PREFIX ids:   <https://w3id.org/idsa/core/>
PREFIX owl:   <http://www.w3.org/2002/07/owl#>
PREFIX prov:  <http://www.w3.org/ns/prov#>
PREFIX rdf:   <http://www.w3.org/1999/02/22-rdf-syntax-ns#>
PREFIX rdfs:  <http://www.w3.org/2000/01/rdf-schema#>
PREFIX sh:    <http://www.w3.org/ns/shacl#>
PREFIX skos:  <http://www.w3.org/2004/02/skos/core#>
PREFIX sml:   <https://w3id.org/sml/def#>
PREFIX vcard: <http://www.w3.org/2006/vcard/ns#>
PREFIX xsd:   <http://www.w3.org/2001/XMLSchema#>



checks:hasRecipient  rdf:type  owl:ObjectProperty;
        skos:definition  "Indicates a relation between a permit request and the Recipient, a prov:Agent, of the request. A Recipient is a legal entity (e.g., authority) or person in charge of receiving the permit application "@en;
        rdfs:label   "has Recipient" .

checks:hasApprover rdf:type owl:ObjectProperty; 
        skos:definition  "Indicates a relation between a permitRequest and the Approver, a prov:Agent, of the Request. An Approver is a legal entity (e.g., competent authority) or person issuing the permit approval. "@en;
        rdfs:label   "has Approver" . 

checks:Allocation  rdf:type  owl:Class;
        rdfs:subClassOf  sml:Objectification;
        skos:definition  "An explicit relation between subject and requirement that shows that the subject needs to fulfill the stated requirement."@en;
        rdfs:label   "Allocation" .

checks:isGeometryOf  rdf:type  owl:ObjectProperty;
        owl:inverseOf    geo:hasGeometry;
        skos:definition  "Indicates that a geometry has a location linked to it."@en;
        rdfs:label   "is geometry of" .

:64da32f2ec98ce2e4c41a232
        rdf:type        sh:NodeShape;
        sh:property     [ sh:class     prov:Agent;
                          sh:maxCount  1;
                          sh:minCount  1;
                          sh:path      prov:wasAssociatedWith
                        ];
        sh:property     [ sh:class     checks:PermitRequest;
                          sh:maxCount  1;
                          sh:minCount  1;
                          sh:path      checks:isDecisionFor
                        ];
        sh:property     [ sh:in        :34e82a97-fdd5-3176-ab61-f75c778939ca;
                          sh:maxCount  1;
                          sh:path      checks:decisionOutcome
                        ];
        sh:property     [ sh:datatype  xsd:date;
                          sh:path      checks:date
                        ];
        sh:targetClass  checks:Decision .

checks:decisionOutcomeValues a rdfs:Class ; 
        rdfs:label  "outcomes for Decision for permits" .

checks:decisionApproved a checks:decisionOutcomeValues ; 
        rdfs:label "Approved" . 

checks:decisionApprovedWithReservations a checks:decisionOutcomeValues ; 
        rdfs:label "Approved With Reservations" . 

checks:decisionRejected a checks:decisionOutcomeValues ; 
        rdfs:label "Rejected" .



checks:hasParcel  rdf:type  owl:ObjectProperty;
        skos:definition  "Indicates the link between location and parcel."@en;
        rdfs:label   "has parcel" .

prov:wasAssociatedWith
        rdf:type        owl:ObjectProperty;
        rdfs:label  "was associated with" .

sh:NodeShape  rdf:type  owl:Class;
        rdfs:label  "Node Shape" .

checks:role  rdf:type     owl:DatatypeProperty;
        skos:definition  "Indicates in what capacity someone/something is linked to a project, permit, ..."@en;
        rdfs:label   "role" .

checks:name  rdf:type     owl:DatatypeProperty;
        skos:definition  "Provides the name/ title for concepts."@en;
        rdfs:label   "name" .

checks:Parcel  rdf:type   owl:Class;
        skos:definition  "Any quantity of land capable of being described with such definiteness that its locations and boundaries may be established."@en;
        rdfs:label   "Parcel" .

checks:decisionOutcome
        rdf:type         owl:DatatypeProperty;
        rdfs:range       xsd:enumeration;
        skos:definition  "Provides a list of possible decision outcomes which impact the permit request."@en;
        rdfs:label   "decision outcome" .

:64eccb68d8a9bc575cd0c914
        rdf:type        sh:NodeShape;
        sh:property     [ sh:class  ids:Resource;
                          sh:path   checks:wasDescribedBy
                        ];
        sh:property     [ sh:class  ids:Resource;
                          sh:path   sml:isDescribedBy
                        ];
        sh:property     [ sh:datatype  xsd:string;
                          sh:path      rdfs:label
                        ];
        sh:property     [ sh:datatype  xsd:string;
                          sh:path      rdfs:comment
                        ];
        sh:targetClass  sh:NodeShape .

:64b000d827b0605cddb2d64c
        rdf:type        sh:NodeShape;
        sh:property     [ sh:class     sml:ConcreteConcept;
                          sh:maxCount  1;
                          sh:minCount  1;
                          sh:path      checks:isAllocationfor
                        ];
        sh:property     [ sh:class  checks:Verification;
                          sh:path   checks:isVerifiedIn
                        ];
        sh:property     [ sh:class     sml:Requirement;
                          sh:maxCount  1;
                          sh:minCount  1;
                          sh:path      sml:hasRequirement
                        ];
        sh:targetClass  checks:Allocation .

sml:hasPart  rdf:type   owl:ObjectProperty;
        rdfs:label  "has part" .

sml:State  rdf:type      owl:Class;
        rdfs:subClassOf  sml:ConcreteConcept;
        rdfs:label   "State" .

sml:PhysicalObject  rdf:type  owl:Class;
        rdfs:subClassOf  sml:Object;
        rdfs:label   "Physical Object" .

sml:AbstractConcept  rdf:type  owl:Class;
        rdfs:subClassOf  sml:TopConcept;
        rdfs:label   "Abstract Concept" .

sml:EnumerationType  rdf:type  owl:Class;
        rdfs:subClassOf  sml:Type;
        rdfs:label   "Enumeration Type" .

:64da327fec98ce2e4c41a229
        rdf:type        sh:NodeShape;
        sh:property     [ sh:datatype  xsd:string;
                          sh:path      checks:version
                        ];
        sh:property     [ sh:class  checks:Permit;
                          sh:path   sml:hasPart
                        ];

        sh:property     [ sh:class     ids:Resource;
                          sh:minCount  1;
                          sh:path      sml:isDescribedBy
                        ];
        sh:property     [ sh:datatype  xsd:date;
                          sh:maxCount  1;
                          sh:minCount  1;
                          sh:path      checks:expirationDate
                        ];
        sh:property     [ sh:class     checks:PermitRequest;
                          sh:minCount  1;
                          sh:path      checks:isPermitFor
                        ];
        sh:property     [ sh:class     sml:Requirement;
                          sh:minCount  1;
                          sh:path      sml:hasRequirement
                        ];
        sh:property     [ sh:datatype  xsd:date;
                          sh:maxCount  1;
                          sh:minCount  1;
                          sh:path      checks:issueDate
                        ];
        sh:targetClass  checks:Permit .

sml:TopConcept  rdf:type  owl:Class;
        rdfs:label  "Top Concept" .

sml:QualityValue  rdf:type  owl:Class;
        rdfs:subClassOf  sml:Objectification;
        rdfs:label   "Quality Value" .

sml:RelationReference
        rdf:type         owl:Class;
        rdfs:subClassOf  sml:Objectification;
        rdfs:label   "Relation Reference" .

checks:isRequestForPermit
        rdf:type         owl:ObjectProperty;
        skos:definition  "Indicates the relation between a request and the specific permit it was requesting."@en;
        rdfs:label   "is request for permit" .

sml:InformationObject
        rdf:type         owl:Class;
        rdfs:subClassOf  sml:Object;
        rdfs:label   "Information Object" .

checks:Permit  rdf:type   owl:Class;
        rdfs:subClassOf  sml:InformationObject;
        skos:definition  "A permit is a written permission or authorisation delivered by a competent authority, entity, or person, that is legally delegated to allow someone to do something or to go somewhere."@en;
        rdfs:label   "Permit" .

checks:isParcelFor  rdf:type  owl:ObjectProperty;
        owl:inverseOf    checks:hasParcel;
        skos:definition  "Indicates that a parcel is located at a certain location."@en;
        rdfs:label   "is parcel for" .



sml:hasInterior  rdf:type  owl:ObjectProperty;
        rdfs:label  "has interior" .

checks:isVerifiedIn  rdf:type  owl:ObjectProperty;
        skos:definition  "Is an association that indicates that the representer object represents the represented object."@en;
        rdfs:label   "is verified in" .

prov:Location  rdf:type  owl:Class;
        rdfs:label  "Location" .

sml:Representation  rdf:type  owl:Class;
        rdfs:subClassOf  sml:InformationObject;
        rdfs:label   "Representation" .

sml:Entity  rdf:type     owl:Class;
        rdfs:subClassOf  sml:ConcreteConcept;
        rdfs:label   "Entitiy" .

checks:isExpressedAs  rdf:type  owl:ObjectProperty;
        skos:definition  "Is a relation that determines how an object is represented similar to a target object"@en;
        rdfs:label   "is expressed as" .

checks:logicalOperator
        rdf:type         owl:DatatypeProperty;
        rdfs:range       xsd:enumeration;
        skos:definition  "Provides the possibility to indicate if certain conditions are complementary (AND) or supplementary (OR)."@en;
        rdfs:label   "logical operator" .

checks:Document  rdf:type  owl:Class;
        rdfs:subClassOf  sml:InformationObject;
        skos:definition  "A piece of written, printed, or electronic matter that provides information or evidence or that serves as an official record or acts as a reference."@en;
        rdfs:label   "Document" .

checks:hasPermitRequest
        rdf:type         owl:ObjectProperty;
        skos:definition  "Indicates the link from a project to a / multiple permit requests."@en;
        rdfs:label   "has permit request" .

sml:isDescribedBy  rdf:type  owl:ObjectProperty;
        skos:definition  "Relation that is used to link various concepts to a resource. Many concepts require to be linked to certain proof documents / descriptions. This relation is set on Top Concept level."@en;
        rdfs:label   "is described by" .

:64d5f40dec98ce2e4c41a100
        rdf:type        sh:NodeShape;
        sh:property     [ sh:class  prov:Agent;
                          sh:path   prov:actedOnBehalfOf
                        ];
        sh:property     [ sh:datatype  xsd:string;
                          sh:path      rdfs:comment
                        ];
        sh:property     [ sh:path  checks:name ];
        sh:property     [ sh:datatype  xsd:string;
                          sh:path      rdfs:label
                        ];
        sh:targetClass  prov:Agent .

vcard:hasAddress  rdf:type  owl:ObjectProperty;
        rdfs:label  "has address" .

sml:triggers  rdf:type  owl:ObjectProperty;
        rdfs:label  "triggers" .

checks:hasApplicant  rdf:type  owl:ObjectProperty;
        skos:definition  "The Permit request was applied for by an agent."@en;
        rdfs:label   "is submitted by" .

sml:Activity  rdf:type   owl:Class;
        rdfs:subClassOf  sml:Entity;
        rdfs:label   "Activity" .

sml:hasTemporalEntity
        rdf:type        owl:ObjectProperty;
        rdfs:label  "has temporal entity" .

sml:Object  rdf:type     owl:Class;
        rdfs:subClassOf  sml:Entity;
        rdfs:label   "Object" .

prov:atLocation  rdf:type  owl:ObjectProperty;
        rdfs:label  "at location" .

sml:transforms  rdf:type  owl:ObjectProperty;
        rdfs:label  "transforms" .

prov:Agent  rdf:type     owl:Class;
        rdfs:subClassOf  <http://w3id.org/gaia-x/participant#Participant>;
        rdfs:label   "Agent" .

checks:shallBeCompliantWith
        rdf:type         owl:ObjectProperty;
        skos:definition  "Is a conceptual requirement for compliancy to a criterion that indicates that a member of the class shall be conformant to a qualitative requirement. Typically an item, story or document of a kind that should be conform to the content of a document."@en;
        rdfs:label   "shall be compliant with" .

:6606a7ae965733652c7f6783
        rdf:type        sh:NodeShape;
        sh:property     [ sh:class  ids:Resource;
                          sh:path   sml:isDescribedBy
                        ];
        sh:property     [ sh:datatype  xsd:string;
                          sh:path      rdfs:label
                        ];
        sh:property     [ sh:datatype  xsd:string;
                          sh:path      rdfs:comment
                        ];
        sh:targetClass  sh:ValidationReport .

# checks:GenericRequirement
#        rdf:type         owl:Class;
#        rdfs:subClassOf  sml:Requirement;
#        skos:definition  "A requirement that is not specific for any projects / use case."@en;
#        rdfs:label   "Generic Requirement" .

sml:QuantityValue  rdf:type  owl:Class;
        rdfs:subClassOf  sml:Objectification;
        rdfs:label   "Quantity Value" .

:64da320fec98ce2e4c41a220
        rdf:type        sh:NodeShape;
        sh:property     [ sh:class  checks:Document;
                          sh:path   checks:hasSource
                        ];
        sh:property     [ sh:class  sml:Requirement;
                          sh:path   sml:hasPart
                        ];
        sh:property     [ sh:or    ( [ sh:class  sh:NodeShape ]
                                     [ sh:class  checks:MachineReadableRule ]
                                   );
                          sh:path  checks:isExpressedAs
                        ];
        sh:property     [ sh:in        :95414b38-5a62-3cf9-beed-42cbc73f4b9e;
                          sh:maxCount  1;
                          sh:path      checks:logicalOperator
                        ];
        sh:targetClass  sml:Requirement .

prov:qualifiedAssociation
        rdf:type        owl:ObjectProperty;
        rdfs:label  "qualified association" .

checks:VerificationMethod
        rdf:type         owl:Class;
        rdfs:subClassOf  sml:Activity;
        skos:definition  "A set of procedures to check if the subject is compliant with requirement."@en;
        rdfs:label   "Verification method" .

:       rdf:type     owl:Ontology;
        rdfs:label   "3.1 Top Ontology";
        owl:imports  sh: , rdfs: , owl: .

ids:Resource  rdf:type  owl:Class;
        rdfs:label  "Resource" .

checks:Verification  rdf:type  owl:Class;
        rdfs:subClassOf  sml:Activity;
        skos:definition  "A Verification is an activity that checks if a subject is compliant with a requirement."@en;
        rdfs:label   "Verification" .

:661525e1fd34eb2f8e03f5bc
        rdf:type        sh:NodeShape;
        sh:property     [ sh:datatype  xsd:string;
                          sh:path      rdfs:label
                        ];
        sh:property     [ sh:datatype  xsd:string;
                          sh:path      rdfs:comment
                        ];
        sh:targetClass  ids:Resource .

:64b000ca27b0605cddb2d646
        rdf:type        sh:NodeShape;
        sh:property     [ sh:class  ids:Resource;
                          sh:path   checks:wasDescribedBy
                        ];
        sh:property     [ sh:class  ids:Resource;
                          sh:path   sml:isDescribedBy
                        ];
        sh:property     [ sh:datatype  xsd:string;
                          sh:path      rdfs:label
                        ];
        sh:property     [ sh:datatype  xsd:string;
                          sh:path      rdfs:comment
                        ];
        sh:targetClass  sml:TopConcept .

rdfs:label  rdf:type  owl:DatatypeProperty;
        rdfs:range      xsd:string;
        rdfs:label  "pref label" .

# checks:ProjectRequirement
#        rdf:type         owl:Class;
#        rdfs:subClassOf  sml:Requirement;
#        skos:definition  "A requirement that is specific to projects / use case. It cannot be generalized over multiple projects / use cases."@en;
#        rdfs:label   "Project Requirement" .

:6615257dfd34eb2f8e03f59a
        rdf:type        sh:NodeShape;
        sh:property     [ sh:class     prov:Location;
                          sh:maxCount  1;
                          sh:minCount  1;
                          sh:path      checks:isAddressFor
                        ];
        sh:property     [ sh:datatype  xsd:string;
                          sh:path      rdfs:label
                        ];
        sh:property     [ sh:datatype  xsd:string;
                          sh:path      rdfs:comment
                        ];
        sh:targetClass  vcard:Address .

sh:ValidationReport  rdf:type  owl:Class;
        rdfs:label  "Validation Report" .

:64dde72c4ef5931bfc406a64
        rdf:type        sh:NodeShape;
        sh:property     [ sh:datatype  xsd:string;
                          sh:path      checks:version
                        ];
        sh:targetClass  checks:Document .

checks:wasDescribedBy  rdf:type  owl:ObjectProperty;
        skos:definition  "Relation that is used to indicate that a concept was linked to certain resource in the past. this is meant to keep track of different versions of resources, keep history on all links ever made from concept to resource."@en;
        rdfs:label   "was described by" .

checks:isMadeBy  rdf:type  owl:ObjectProperty;
        skos:definition  "Is an involvement in an occurrence that indicates that the involved object has a role as performer of the occurrence."@en;
        rdfs:label   "is made by" .

:661525d6fd34eb2f8e03f5b4
        rdf:type        sh:NodeShape;
        sh:property     [ sh:class     prov:Location;
                          sh:maxCount  1;
                          sh:minCount  1;
                          sh:path      checks:isParcelFor
                        ];
        sh:property     [ sh:datatype  xsd:string;
                          sh:path      rdfs:label
                        ];
        sh:property     [ sh:datatype  xsd:string;
                          sh:path      rdfs:comment
                        ];
        sh:targetClass  checks:Parcel .

sml:hasBoundary  rdf:type  owl:ObjectProperty;
        rdfs:label  "has boundary" .

checks:isInputFor  rdf:type  owl:ObjectProperty;
        skos:definition  "Indicates that a / multiple verifications where carried out as a foundation for certain decision taken."@en;
        rdfs:label   "is input for" .

sml:Requirement  rdf:type  owl:Class;
        rdfs:subClassOf  sml:InformationObject;
        skos:definition  "A rule that should hold for something, defined via its attributes or relations"@en;
        rdfs:label   "Requirement" .

:65e60b91ebc1577ef9381cbb
        rdf:type        sh:NodeShape;
        sh:property     [ sh:class  prov:Agent;
                          sh:path   checks:hasRecipient; 
                          sh:minCount 1;
                          sh:maxCount 1; 
                        ];
        sh:property     [ sh:class  prov:Agent;
                          sh:path   checks:hasApprover; 
                          # No minCounts, or max counts > The application may be in a state that it is unclear who the Approver is. 
                          # No sh:maxCount, since there can be multiple Agents involved. 
                        ];
        sh:property     [ sh:class     prov:Agent;
                          sh:minCount  1;
                          sh:path      checks:hasApplicant
                        ];
        sh:property     [ sh:class     checks:Project;
                          sh:minCount  1;
                          sh:path      checks:isPermitForRequest
                        ];
        sh:property     [ sh:class     checks:Permit;
                          sh:maxCount  1;
                          sh:path      checks:isRequestForPermit
                        ];
        sh:property     [ sh:datatype  xsd:date;
                          sh:maxCount  1;
                          sh:minCount  1;
                          sh:path      checks:applicationDate
                        ];
        sh:targetClass  checks:PermitRequest .

checks:size  rdf:type    owl:DatatypeProperty;
        rdfs:label  "size" .

:64d4a25fec98ce2e4c41a07d
        rdf:type        sh:NodeShape;
        sh:property     [ sh:class     checks:Decision;
                          sh:minCount  1;
                          sh:path      checks:isInputFor
                        ];
        sh:property     [ sh:class     prov:Agent;
                          sh:maxCount  1;
                          sh:minCount  1;
                          sh:path      prov:wasAssociatedWith
                        ];
        sh:property     [ sh:class     checks:VerificationMethod;
                          sh:maxCount  1;
                          sh:minCount  1;
                          sh:path      checks:hasVerificationMethod
                        ];
        sh:property     [ sh:datatype  xsd:date;
                          sh:path      checks:date
                        ];
        sh:targetClass  checks:Verification .


:VerificationShapeOutcomes 
        rdf:type        sh:nodeShape; 
        sh:targetClass  checks:Verification ; 
        sh:property     [ sh:or    ( [ sh:class  checks:Document ]
                                     [ sh:class  sh:ValidationReport ]
                                   );
                          sh:path  checks:hasAsOutput
                        ];
        # 
        sh:property     [ sh:class        :ResultValues;
                          sh:maxCount  1;
                          sh:path      checks:result
                        ];

checks:ResultValues 
        rdf:type        rdfs:Class ; 
        rdfs:label  "Compliance values" .

checks:CheckCompliant a checks:ResultValues  ; 
      rdfs:label "Compliant" . 
  
checks:CheckNonCompliant a checks:ResultValues ; 
      rdfs:label "Non compliant" .

checks:version  rdf:type  owl:DatatypeProperty;
        rdfs:range      xsd:string;
        rdfs:label  "version" .

checks:result  rdf:type  owl:DatatypeProperty;
        rdfs:range      xsd:enumeration;
        rdfs:label  "result" .

sml:TemporalEntity  rdf:type  owl:Class;
        rdfs:subClassOf  sml:Representation;
        rdfs:label   "Temporal Entity" .

prov:agent  rdf:type    owl:ObjectProperty;
        rdfs:label  "agent" .

checks:isDecisionFor  rdf:type  owl:ObjectProperty;
        skos:definition  "Is a relation indicating the choice or judgment made based on available resources."@en;
        rdfs:label   "is decision for" .

checks:date  rdf:type     owl:DatatypeProperty;
        rdfs:range       xsd:date;
        skos:definition  "This attribute describes a timing linked to concepts. It may indicate a date when something was submitted, received, checked, has expired, ..."@en;
        rdfs:label   "date " .

checks:isCollectedIn  rdf:type  owl:ObjectProperty;
        skos:definition  "Is a relation between a single thing and a plurality that indicates that the collected object is element of the collection of objects, under the constraint that the element may not be the same object as the plural object. In other words a collection cannot be an element of itself."@en;
        rdfs:label   "is collected in" .

sml:Event  rdf:type      owl:Class;
        rdfs:subClassOf  sml:ConcreteConcept;
        rdfs:label   "Event" .

sml:executes  rdf:type  owl:ObjectProperty;
        rdfs:label  "executes" .

sml:GeometricEntity  rdf:type  owl:Class;
        rdfs:subClassOf  sml:Representation;
        rdfs:label   "Geometric Entity" .

checks:Decision  rdf:type  owl:Class;
        rdfs:subClassOf  sml:Activity;
        skos:definition  "A decision is an activity of making a choice or judgement based on the available resources."@en;
        rdfs:label   "Decision" .

checks:hasVerificationMethod
        rdf:type         owl:ObjectProperty;
        skos:definition  "Is an association that indicates a method to verify if the verification object has a method linked to it."@en;
        rdfs:label   "has verification method" .

checks:isAllocationfor
        rdf:type         owl:ObjectProperty;
        skos:definition  "Is an association to ensure that the involved object has an allocation to the corresponding requirement."@en;
        rdfs:label   "is allocation for" .

checks:isDerivedIn  rdf:type  owl:ObjectProperty;
        skos:definition  "Is an association that indicates that the object has been derived in the source object."@en;
        rdfs:label   "is derived in" .

rdfs:comment  rdf:type  owl:DatatypeProperty;
        rdfs:range      xsd:string;
        rdfs:label  "comment" .

checks:applicationDate
        rdf:type            owl:DatatypeProperty;
        rdfs:range          xsd:date;
        rdfs:subPropertyOf  checks:date;
        rdfs:label      "application date" .

:64ddde554ef5931bfc406a34
        rdf:type        sh:NodeShape;
        sh:property     [ sh:class     vcard:Address;
                          sh:maxCount  1;
                          sh:path      vcard:hasAddress
                        ];
        sh:property     [ sh:class     geo:Geometry;
                          sh:maxCount  1;
                          sh:path      geo:hasGeometry
                        ];
        sh:property     [ sh:class     checks:Parcel;
                          sh:maxCount  1;
                          sh:path      checks:hasParcel
                        ];
        sh:property     [ sh:datatype  xsd:string;
                          sh:path      rdfs:label
                        ];
        sh:property     [ sh:datatype  xsd:string;
                          sh:path      rdfs:comment
                        ];
        sh:targetClass  prov:Location .

:661525befd34eb2f8e03f5a4
        rdf:type        sh:NodeShape;
        sh:property     [ sh:class     prov:Location;
                          sh:maxCount  1;
                          sh:minCount  1;
                          sh:path      checks:isGeometryOf
                        ];
        sh:property     [ sh:datatype  xsd:string;
                          sh:path      rdfs:label
                        ];
        sh:property     [ sh:datatype  xsd:string;
                          sh:path      rdfs:comment
                        ];
        sh:targetClass  geo:Geometry .



sml:hasState  rdf:type  owl:ObjectProperty;
        rdfs:label  "has state" .

checks:issueDate  rdf:type   owl:DatatypeProperty;
        rdfs:range          xsd:date;
        rdfs:subPropertyOf  checks:date;
        rdfs:label      "issue date" .

sml:begins  rdf:type    owl:ObjectProperty;
        rdfs:label  "begins" .

dct:subject  rdf:type   owl:ObjectProperty;
        rdfs:label  "subject" .

checks:MachineReadableRule
        rdf:type         owl:Class;
        rdfs:subClassOf  sml:AbstractConcept;
        skos:definition  "A set of instructions or guidelines that are structured in a format that can be easily interpreted and processed by a computer or software program. The term \"rule\" refers here to checking rules specifically and is not to be confused with inferencing rules for deriving knowledge."@en;
        rdfs:label   "Machine readable rule" .

checks:hasAsOutput  rdf:type  owl:ObjectProperty;
        skos:definition  "Is an involvement in an occurrence that indicates that the involved object has been operated upon by the occurrence."@en;
        rdfs:label   "has as output" .

sml:Type  rdf:type       owl:Class;
        rdfs:subClassOf  sml:AbstractConcept;
        rdfs:label   "Type" .

prov:actedOnBehalfOf  rdf:type  owl:ObjectProperty;
        rdfs:label  "acted on behalf of" .

sml:hasRequirement  rdf:type  owl:ObjectProperty;
        rdfs:label  "has requirement" .

geo:Geometry  rdf:type  owl:Class;
        rdfs:label  "Geometry" .

geo:hasGeometry  rdf:type  owl:ObjectProperty;
        rdfs:label  "has geometry" .

checks:isPermitForRequest
        rdf:type         owl:ObjectProperty;
        owl:inverseOf    checks:hasPermitRequest;
        skos:definition  "Indicates the relation between a permit and the related request for it"@en;
        rdfs:label   "is permit for request" .

checks:hasUsecase
      rdf:type          owl:ObjectProperty; 
      skos:definition   "Indicates which use case is applicable for a specific project"@en ; 
      rdfs:label    "has usecase" . 


:64da30f3ec98ce2e4c41a20b
        rdf:type        sh:NodeShape;
        sh:property     [ sh:class     prov:Association;
                          sh:minCount  1;
                          sh:path      prov:qualifiedAssociation
                        ];
        sh:property     [ sh:class  sml:TopConcept;
                          sh:path   dct:subject
                        ];
        sh:property     [ sh:class  checks:PermitRequest;
                          sh:path   checks:hasPermitRequest
                        ];
        sh:property     [ sh:class  prov:Location;
                          sh:path   prov:atLocation
                        ];
        sh:property     [ sh:path  checks:size ];
        sh:property   [ sh:path  checks:hasUsecase 
                        sh:class checks:UsecaseValues ] ; 
        sh:targetClass  checks:Project .

checks:UsecaseValues a rdfs:Class ; 
    rdfs:label "Values for the different use cases" . 

checks:Residential a checks:UsecaseValues ; 
rdfs:label "Residential" . 

checks:Office a checks:UsecaseValues ; 
rdfs:label "Office" . 
checks:CommercialBuilding a checks:UsecaseValues ;
skos:editorialNote "A building open to the general public with a commercial purpose, such as shops." 
rdfs:label "Commercial building" . 


checks:PublicServices a checks:UsecaseValues ;
skos:note "A building open to the general public with a non-commercial purpose, such as hospitals or schools. " 
rdfs:label "Public services" . 

checks:Industrial a checks:UsecaseValues ; 
rdfs:label "Industrial" . 


checks:expirationDate  rdf:type  owl:DatatypeProperty;
        rdfs:range          xsd:date;
        rdfs:subPropertyOf  checks:date;
        rdfs:label      "expiration date" .

sml:ConcreteConcept  rdf:type  owl:Class;
        rdfs:subClassOf  sml:TopConcept;
        rdfs:label   "Concrete Concept" .

:65d3dc1c13b8ea5093980dfc
        rdf:type        sh:NodeShape;
        sh:property     [ sh:class     prov:Agent;
                          sh:maxCount  1;
                          sh:minCount  1;
                          sh:path      prov:agent
                        ];
        sh:property     [ sh:path  checks:role ];
        sh:targetClass  prov:Association .

checks:PermitRequest  rdf:type  owl:Class;
        rdfs:subClassOf  sml:InformationObject;
        skos:definition  """A permit request is a written appeal or application made to obtain official approval for something from a designated authority.
It is used as the central hub in the permitting process, with, if issued, a checks:Permit as a result."""@en;
        rdfs:label   "Permit request" .

prov:Association  rdf:type  owl:Class;
        rdfs:subClassOf  sml:InformationObject;
        rdfs:label   "Association" .

checks:isPermitFor  rdf:type  owl:ObjectProperty;
        owl:inverseOf    checks:isRequestForPermit;
        skos:definition  "Indicates the link between a permit and corresponding permit request that are / were made to obtain certain permit"@en;
        rdfs:label   "is permit for" .

checks:isAddressFor  rdf:type  owl:ObjectProperty;
        owl:inverseOf    vcard:hasAddress;
        skos:definition  "Relation to check if the address is linked to a location."@en;
        rdfs:label   "is address for" .

checks:Project  rdf:type  owl:Class;
        rdfs:subClassOf  sml:Entity;
        skos:definition  "A temporary process undertaken to solve a well-defined goal or objective with clearly defined start and end times, a set of clearly defined tasks, and a budget."@en;
        rdfs:label   "Project" .

checks:hasSource  rdf:type  owl:ObjectProperty;
        skos:definition  "Is a relation that indicates the involved object has a origin or source from another object."@en;
        rdfs:label   "has source" .

prov:Organization  rdf:type  owl:Class;
        rdfs:subClassOf  prov:Agent;
        rdfs:label   "Organization" .

:95414b38-5a62-3cf9-beed-42cbc73f4b9e
        rdf:type        rdf:List;
        rdf:first       "OR";
        rdf:rest        ( "AND" );
        rdfs:label  "Logical operator list for requirements" .

sml:ConceptType  rdf:type  owl:Class;
        rdfs:subClassOf  sml:Type;
        rdfs:label   "Concept Type" .

sml:ends  rdf:type      owl:ObjectProperty;
        rdfs:label  "ends" .

vcard:Address  rdf:type  owl:Class;
        rdfs:label  "Address" .

prov:Person  rdf:type    owl:Class;
        rdfs:subClassOf  prov:Agent;
        rdfs:label   "Person" .

sml:Objectification  rdf:type  owl:Class;
        rdfs:subClassOf  sml:AbstractConcept;
        rdfs:label   "Objectification" .
