@prefix : <https://data.digichecks.eu/def/> .
@prefix owl: <http://www.w3.org/2002/07/owl#> .
@prefix rdf: <http://www.w3.org/1999/02/22-rdf-syntax-ns#> .
@prefix xml: <http://www.w3.org/XML/1998/namespace> .
@prefix xsd: <http://www.w3.org/2001/XMLSchema#> .
@prefix rdfs: <http://www.w3.org/2000/01/rdf-schema#> .
@base <https://data.digichecks.eu/def/> .

<https://data.digichecks.eu/def/> rdf:type owl:Ontology ;
                                   owl:imports rdfs: ,
                                               owl: ,
                                               <http://www.w3.org/ns/shacl#> ,
                                               <https://w3id.org/sml/def#> ;
                                   <http://purl.org/dc/terms/creator> "DigiChecks" ;
                                   <http://purl.org/dc/terms/date> "2024-06-10T17:27:04.485561856" ;
                                   <http://purl.org/dc/terms/description> "The top-level permit ontology contains the relevant terminology related to permitting processes. Based on Semantic Modelling and Linking (SML, EN 17632),  it contains the core terminology for DigiChecks services to communicate unambiguously about a permitting process." ;
                                   rdfs:label "Permit ontology based on the SML framework" ;
                                   owl:versionInfo "1.0" .

#################################################################
#    Annotation properties
#################################################################

###  http://purl.org/dc/terms/creator
<http://purl.org/dc/terms/creator> rdf:type owl:AnnotationProperty .


###  http://purl.org/dc/terms/date
<http://purl.org/dc/terms/date> rdf:type owl:AnnotationProperty .


###  http://purl.org/dc/terms/description
<http://purl.org/dc/terms/description> rdf:type owl:AnnotationProperty .


###  http://www.w3.org/2000/01/rdf-schema#isDefinedBy
rdfs:isDefinedBy rdfs:subPropertyOf rdfs:seeAlso ;
                 rdfs:range rdfs:Resource ;
                 rdfs:domain rdfs:Resource .


###  http://www.w3.org/2000/01/rdf-schema#label
rdfs:label rdfs:range rdfs:Literal ;
           rdfs:domain rdfs:Resource .


###  http://www.w3.org/2000/01/rdf-schema#seeAlso
rdfs:seeAlso rdfs:range rdfs:Resource ;
             rdfs:domain rdfs:Resource .


###  http://www.w3.org/2002/07/owl#backwardCompatibleWith
owl:backwardCompatibleWith rdf:type owl:AnnotationProperty ;
                           rdfs:range owl:Ontology ;
                           rdfs:domain owl:Ontology .


###  http://www.w3.org/2002/07/owl#deprecated
owl:deprecated rdf:type owl:AnnotationProperty ;
               rdfs:range rdfs:Resource ;
               rdfs:domain rdfs:Resource .


###  http://www.w3.org/2002/07/owl#imports
owl:imports rdf:type owl:AnnotationProperty ;
            rdfs:range owl:Ontology ;
            rdfs:domain owl:Ontology .


###  http://www.w3.org/2002/07/owl#incompatibleWith
owl:incompatibleWith rdf:type owl:AnnotationProperty ;
                     rdfs:range owl:Ontology ;
                     rdfs:domain owl:Ontology .


###  http://www.w3.org/2002/07/owl#priorVersion
owl:priorVersion rdf:type owl:AnnotationProperty ;
                 rdfs:range owl:Ontology ;
                 rdfs:domain owl:Ontology .


###  http://www.w3.org/2002/07/owl#versionIRI
owl:versionIRI rdf:type owl:AnnotationProperty ;
               rdfs:range owl:Ontology ;
               rdfs:domain owl:Ontology .


###  http://www.w3.org/2002/07/owl#versionInfo
owl:versionInfo rdf:type owl:AnnotationProperty ;
                rdfs:range rdfs:Resource ;
                rdfs:domain rdfs:Resource .


###  http://www.w3.org/2004/02/skos/core#definition
<http://www.w3.org/2004/02/skos/core#definition> rdf:type owl:AnnotationProperty .


###  http://www.w3.org/ns/shacl#annotationValue
<http://www.w3.org/ns/shacl#annotationValue> rdfs:domain <http://www.w3.org/ns/shacl#ResultAnnotation> .


###  http://www.w3.org/ns/shacl#defaultValue
<http://www.w3.org/ns/shacl#defaultValue> rdfs:domain <http://www.w3.org/ns/shacl#PropertyShape> .


###  http://www.w3.org/ns/shacl#description
<http://www.w3.org/ns/shacl#description> rdfs:domain <http://www.w3.org/ns/shacl#PropertyShape> .


###  http://www.w3.org/ns/shacl#focusNode
<http://www.w3.org/ns/shacl#focusNode> rdfs:domain <http://www.w3.org/ns/shacl#AbstractResult> .


###  http://www.w3.org/ns/shacl#labelTemplate
<http://www.w3.org/ns/shacl#labelTemplate> rdfs:domain <http://www.w3.org/ns/shacl#Parameterizable> .


###  http://www.w3.org/ns/shacl#name
<http://www.w3.org/ns/shacl#name> rdfs:domain <http://www.w3.org/ns/shacl#PropertyShape> .


###  http://www.w3.org/ns/shacl#object
<http://www.w3.org/ns/shacl#object> rdfs:domain <http://www.w3.org/ns/shacl#TripleRule> .


###  http://www.w3.org/ns/shacl#predicate
<http://www.w3.org/ns/shacl#predicate> rdfs:domain <http://www.w3.org/ns/shacl#TripleRule> .


###  http://www.w3.org/ns/shacl#resultMessage
<http://www.w3.org/ns/shacl#resultMessage> rdfs:domain <http://www.w3.org/ns/shacl#AbstractResult> .


###  http://www.w3.org/ns/shacl#sourceConstraint
<http://www.w3.org/ns/shacl#sourceConstraint> rdfs:domain <http://www.w3.org/ns/shacl#AbstractResult> .


###  http://www.w3.org/ns/shacl#subject
<http://www.w3.org/ns/shacl#subject> rdfs:domain <http://www.w3.org/ns/shacl#TripleRule> .


###  http://www.w3.org/ns/shacl#targetNode
<http://www.w3.org/ns/shacl#targetNode> rdfs:domain <http://www.w3.org/ns/shacl#Shape> .


###  http://www.w3.org/ns/shacl#value
<http://www.w3.org/ns/shacl#value> rdfs:domain <http://www.w3.org/ns/shacl#AbstractResult> .


#################################################################
#    Object Properties
#################################################################

###  http://purl.org/dc/terms/subject
<http://purl.org/dc/terms/subject> rdf:type owl:ObjectProperty .


###  http://www.opengis.net/ont/geosparql#hasGeometry
<http://www.opengis.net/ont/geosparql#hasGeometry> rdf:type owl:ObjectProperty .


###  http://www.w3.org/2000/01/rdf-schema#domain
rdfs:domain rdfs:domain rdf:Property ;
            rdfs:range rdfs:Class .


###  http://www.w3.org/2000/01/rdf-schema#member
rdfs:member rdfs:domain rdfs:Resource ;
            rdfs:range rdfs:Resource .


###  http://www.w3.org/2000/01/rdf-schema#range
rdfs:range rdfs:domain rdf:Property ;
           rdfs:range rdfs:Class .


###  http://www.w3.org/2000/01/rdf-schema#subClassOf
rdfs:subClassOf rdfs:domain rdfs:Class ;
                rdfs:range rdfs:Class .


###  http://www.w3.org/2000/01/rdf-schema#subPropertyOf
rdfs:subPropertyOf rdfs:domain rdf:Property ;
                   rdfs:range rdf:Property .


###  http://www.w3.org/2002/07/owl#allValuesFrom
owl:allValuesFrom rdfs:domain owl:Restriction ;
                  rdfs:range rdfs:Class .


###  http://www.w3.org/2002/07/owl#annotatedProperty
owl:annotatedProperty rdfs:domain rdfs:Resource ;
                      rdfs:range rdfs:Resource .


###  http://www.w3.org/2002/07/owl#annotatedSource
owl:annotatedSource rdfs:domain rdfs:Resource ;
                    rdfs:range rdfs:Resource .


###  http://www.w3.org/2002/07/owl#annotatedTarget
owl:annotatedTarget rdfs:domain rdfs:Resource ;
                    rdfs:range rdfs:Resource .


###  http://www.w3.org/2002/07/owl#assertionProperty
owl:assertionProperty rdfs:domain owl:NegativePropertyAssertion ;
                      rdfs:range rdf:Property .


###  http://www.w3.org/2002/07/owl#bottomObjectProperty
owl:bottomObjectProperty rdf:type owl:ObjectProperty ;
                         rdfs:domain owl:Thing ;
                         rdfs:range owl:Thing .


###  http://www.w3.org/2002/07/owl#complementOf
owl:complementOf rdfs:domain owl:Class ;
                 rdfs:range owl:Class .


###  http://www.w3.org/2002/07/owl#datatypeComplementOf
owl:datatypeComplementOf rdfs:domain rdfs:Datatype ;
                         rdfs:range rdfs:Datatype .


###  http://www.w3.org/2002/07/owl#differentFrom
owl:differentFrom rdfs:domain owl:Thing ;
                  rdfs:range owl:Thing .


###  http://www.w3.org/2002/07/owl#disjointUnionOf
owl:disjointUnionOf rdfs:domain owl:Class ;
                    rdfs:range rdf:List .


###  http://www.w3.org/2002/07/owl#disjointWith
owl:disjointWith rdfs:domain owl:Class ;
                 rdfs:range owl:Class .


###  http://www.w3.org/2002/07/owl#distinctMembers
owl:distinctMembers rdfs:domain owl:AllDifferent ;
                    rdfs:range rdf:List .


###  http://www.w3.org/2002/07/owl#equivalentClass
owl:equivalentClass rdfs:domain rdfs:Class ;
                    rdfs:range rdfs:Class .


###  http://www.w3.org/2002/07/owl#equivalentProperty
owl:equivalentProperty rdfs:domain rdf:Property ;
                       rdfs:range rdf:Property .


###  http://www.w3.org/2002/07/owl#hasKey
owl:hasKey rdfs:domain owl:Class ;
           rdfs:range rdf:List .


###  http://www.w3.org/2002/07/owl#hasSelf
owl:hasSelf rdfs:domain owl:Restriction ;
            rdfs:range rdfs:Resource .


###  http://www.w3.org/2002/07/owl#hasValue
owl:hasValue rdfs:domain owl:Restriction ;
             rdfs:range rdfs:Resource .


###  http://www.w3.org/2002/07/owl#intersectionOf
owl:intersectionOf rdfs:domain rdfs:Class ;
                   rdfs:range rdf:List .


###  http://www.w3.org/2002/07/owl#inverseOf
owl:inverseOf rdfs:domain owl:ObjectProperty ;
              rdfs:range owl:ObjectProperty .


###  http://www.w3.org/2002/07/owl#members
owl:members rdfs:domain rdfs:Resource ;
            rdfs:range rdf:List .


###  http://www.w3.org/2002/07/owl#onClass
owl:onClass rdfs:domain owl:Restriction ;
            rdfs:range owl:Class .


###  http://www.w3.org/2002/07/owl#onDataRange
owl:onDataRange rdfs:domain owl:Restriction ;
                rdfs:range rdfs:Datatype .


###  http://www.w3.org/2002/07/owl#onDatatype
owl:onDatatype rdfs:domain rdfs:Datatype ;
               rdfs:range rdfs:Datatype .


###  http://www.w3.org/2002/07/owl#onProperties
owl:onProperties rdfs:domain owl:Restriction ;
                 rdfs:range rdf:List .


###  http://www.w3.org/2002/07/owl#onProperty
owl:onProperty rdfs:domain owl:Restriction ;
               rdfs:range rdf:Property .


###  http://www.w3.org/2002/07/owl#oneOf
owl:oneOf rdfs:domain rdfs:Class ;
          rdfs:range rdf:List .


###  http://www.w3.org/2002/07/owl#propertyChainAxiom
owl:propertyChainAxiom rdfs:domain owl:ObjectProperty ;
                       rdfs:range rdf:List .


###  http://www.w3.org/2002/07/owl#propertyDisjointWith
owl:propertyDisjointWith rdfs:domain rdf:Property ;
                         rdfs:range rdf:Property .


###  http://www.w3.org/2002/07/owl#sameAs
owl:sameAs rdfs:domain owl:Thing ;
           rdfs:range owl:Thing .


###  http://www.w3.org/2002/07/owl#someValuesFrom
owl:someValuesFrom rdfs:domain owl:Restriction ;
                   rdfs:range rdfs:Class .


###  http://www.w3.org/2002/07/owl#sourceIndividual
owl:sourceIndividual rdfs:domain owl:NegativePropertyAssertion ;
                     rdfs:range owl:Thing .


###  http://www.w3.org/2002/07/owl#targetIndividual
owl:targetIndividual rdfs:domain owl:NegativePropertyAssertion ;
                     rdfs:range owl:Thing .


###  http://www.w3.org/2002/07/owl#targetValue
owl:targetValue rdfs:domain owl:NegativePropertyAssertion ;
                rdfs:range rdfs:Literal .


###  http://www.w3.org/2002/07/owl#topObjectProperty
owl:topObjectProperty rdf:type owl:ObjectProperty ;
                      rdfs:domain owl:Thing ;
                      rdfs:range owl:Thing .


###  http://www.w3.org/2002/07/owl#unionOf
owl:unionOf rdfs:domain rdfs:Class ;
            rdfs:range rdf:List .


###  http://www.w3.org/2002/07/owl#withRestrictions
owl:withRestrictions rdfs:domain rdfs:Datatype ;
                     rdfs:range rdf:List .


###  http://www.w3.org/2006/vcard/ns#hasAddress
<http://www.w3.org/2006/vcard/ns#hasAddress> rdf:type owl:ObjectProperty .


###  http://www.w3.org/ns/prov#actedOnBehalfOf
<http://www.w3.org/ns/prov#actedOnBehalfOf> rdf:type owl:ObjectProperty .


###  http://www.w3.org/ns/prov#agent
<http://www.w3.org/ns/prov#agent> rdf:type owl:ObjectProperty .


###  http://www.w3.org/ns/prov#atLocation
<http://www.w3.org/ns/prov#atLocation> rdf:type owl:ObjectProperty .


###  http://www.w3.org/ns/prov#qualifiedAssociation
<http://www.w3.org/ns/prov#qualifiedAssociation> rdf:type owl:ObjectProperty .


###  http://www.w3.org/ns/prov#wasAssociatedWith
<http://www.w3.org/ns/prov#wasAssociatedWith> rdf:type owl:ObjectProperty .


###  http://www.w3.org/ns/shacl#alternativePath
<http://www.w3.org/ns/shacl#alternativePath> rdfs:range rdf:List .


###  http://www.w3.org/ns/shacl#and
<http://www.w3.org/ns/shacl#and> rdfs:range rdf:List .


###  http://www.w3.org/ns/shacl#annotationProperty
<http://www.w3.org/ns/shacl#annotationProperty> rdfs:domain <http://www.w3.org/ns/shacl#ResultAnnotation> ;
                                                rdfs:range rdf:Property .


###  http://www.w3.org/ns/shacl#class
<http://www.w3.org/ns/shacl#class> rdfs:range rdfs:Class .


###  http://www.w3.org/ns/shacl#condition
<http://www.w3.org/ns/shacl#condition> rdfs:domain <http://www.w3.org/ns/shacl#Rule> ;
                                       rdfs:range <http://www.w3.org/ns/shacl#Shape> .


###  http://www.w3.org/ns/shacl#datatype
<http://www.w3.org/ns/shacl#datatype> rdfs:range rdfs:Datatype .


###  http://www.w3.org/ns/shacl#declare
<http://www.w3.org/ns/shacl#declare> rdfs:domain owl:Ontology ;
                                     rdfs:range <http://www.w3.org/ns/shacl#PrefixDeclaration> .


###  http://www.w3.org/ns/shacl#detail
<http://www.w3.org/ns/shacl#detail> rdfs:domain <http://www.w3.org/ns/shacl#AbstractResult> ;
                                    rdfs:range <http://www.w3.org/ns/shacl#AbstractResult> .


###  http://www.w3.org/ns/shacl#disjoint
<http://www.w3.org/ns/shacl#disjoint> rdfs:range rdf:Property .


###  http://www.w3.org/ns/shacl#entailment
<http://www.w3.org/ns/shacl#entailment> rdfs:domain owl:Ontology ;
                                        rdfs:range rdfs:Resource .


###  http://www.w3.org/ns/shacl#equals
<http://www.w3.org/ns/shacl#equals> rdfs:range rdf:Property .


###  http://www.w3.org/ns/shacl#filterShape
<http://www.w3.org/ns/shacl#filterShape> rdfs:range <http://www.w3.org/ns/shacl#Shape> .


###  http://www.w3.org/ns/shacl#group
<http://www.w3.org/ns/shacl#group> rdfs:domain <http://www.w3.org/ns/shacl#PropertyShape> ;
                                   rdfs:range <http://www.w3.org/ns/shacl#PropertyGroup> .


###  http://www.w3.org/ns/shacl#ignoredProperties
<http://www.w3.org/ns/shacl#ignoredProperties> rdfs:range rdf:List .


###  http://www.w3.org/ns/shacl#in
<http://www.w3.org/ns/shacl#in> rdfs:range rdf:List .


###  http://www.w3.org/ns/shacl#inversePath
<http://www.w3.org/ns/shacl#inversePath> rdfs:range rdfs:Resource .


###  http://www.w3.org/ns/shacl#js
<http://www.w3.org/ns/shacl#js> rdfs:range <http://www.w3.org/ns/shacl#JSConstraint> .


###  http://www.w3.org/ns/shacl#jsLibrary
<http://www.w3.org/ns/shacl#jsLibrary> rdfs:range <http://www.w3.org/ns/shacl#JSLibrary> .


###  http://www.w3.org/ns/shacl#languageIn
<http://www.w3.org/ns/shacl#languageIn> rdfs:range rdf:List .


###  http://www.w3.org/ns/shacl#lessThan
<http://www.w3.org/ns/shacl#lessThan> rdfs:range rdf:Property .


###  http://www.w3.org/ns/shacl#lessThanOrEquals
<http://www.w3.org/ns/shacl#lessThanOrEquals> rdfs:range rdf:Property .


###  http://www.w3.org/ns/shacl#node
<http://www.w3.org/ns/shacl#node> rdfs:range <http://www.w3.org/ns/shacl#NodeShape> .


###  http://www.w3.org/ns/shacl#nodeKind
<http://www.w3.org/ns/shacl#nodeKind> rdfs:range <http://www.w3.org/ns/shacl#NodeKind> .


###  http://www.w3.org/ns/shacl#nodeValidator
<http://www.w3.org/ns/shacl#nodeValidator> rdfs:domain <http://www.w3.org/ns/shacl#ConstraintComponent> ;
                                           rdfs:range <http://www.w3.org/ns/shacl#Validator> .


###  http://www.w3.org/ns/shacl#not
<http://www.w3.org/ns/shacl#not> rdfs:range <http://www.w3.org/ns/shacl#Shape> .


###  http://www.w3.org/ns/shacl#oneOrMorePath
<http://www.w3.org/ns/shacl#oneOrMorePath> rdfs:range rdfs:Resource .


###  http://www.w3.org/ns/shacl#or
<http://www.w3.org/ns/shacl#or> rdfs:range rdf:List .


###  http://www.w3.org/ns/shacl#parameter
<http://www.w3.org/ns/shacl#parameter> rdfs:domain <http://www.w3.org/ns/shacl#Parameterizable> ;
                                       rdfs:range <http://www.w3.org/ns/shacl#Parameter> .


###  http://www.w3.org/ns/shacl#path
<http://www.w3.org/ns/shacl#path> rdfs:domain <http://www.w3.org/ns/shacl#PropertyShape> ;
                                  rdfs:range rdfs:Resource .


###  http://www.w3.org/ns/shacl#prefixes
<http://www.w3.org/ns/shacl#prefixes> rdfs:domain <http://www.w3.org/ns/shacl#SPARQLExecutable> ;
                                      rdfs:range owl:Ontology .


###  http://www.w3.org/ns/shacl#property
<http://www.w3.org/ns/shacl#property> rdfs:domain <http://www.w3.org/ns/shacl#Shape> ;
                                      rdfs:range <http://www.w3.org/ns/shacl#PropertyShape> .


###  http://www.w3.org/ns/shacl#propertyValidator
<http://www.w3.org/ns/shacl#propertyValidator> rdfs:domain <http://www.w3.org/ns/shacl#ConstraintComponent> ;
                                               rdfs:range <http://www.w3.org/ns/shacl#Validator> .


###  http://www.w3.org/ns/shacl#qualifiedValueShape
<http://www.w3.org/ns/shacl#qualifiedValueShape> rdfs:range <http://www.w3.org/ns/shacl#Shape> .


###  http://www.w3.org/ns/shacl#result
<http://www.w3.org/ns/shacl#result> rdfs:domain <http://www.w3.org/ns/shacl#ValidationReport> ;
                                    rdfs:range <http://www.w3.org/ns/shacl#ValidationResult> .


###  http://www.w3.org/ns/shacl#resultAnnotation
<http://www.w3.org/ns/shacl#resultAnnotation> rdfs:domain <http://www.w3.org/ns/shacl#SPARQLSelectValidator> ;
                                              rdfs:range <http://www.w3.org/ns/shacl#ResultAnnotation> .


###  http://www.w3.org/ns/shacl#resultPath
<http://www.w3.org/ns/shacl#resultPath> rdfs:domain <http://www.w3.org/ns/shacl#AbstractResult> ;
                                        rdfs:range rdfs:Resource .


###  http://www.w3.org/ns/shacl#resultSeverity
<http://www.w3.org/ns/shacl#resultSeverity> rdfs:domain <http://www.w3.org/ns/shacl#AbstractResult> ;
                                            rdfs:range <http://www.w3.org/ns/shacl#Severity> .


###  http://www.w3.org/ns/shacl#returnType
<http://www.w3.org/ns/shacl#returnType> rdfs:domain <http://www.w3.org/ns/shacl#Function> ;
                                        rdfs:range rdfs:Class .


###  http://www.w3.org/ns/shacl#rule
<http://www.w3.org/ns/shacl#rule> rdfs:domain <http://www.w3.org/ns/shacl#Shape> ;
                                  rdfs:range <http://www.w3.org/ns/shacl#Rule> .


###  http://www.w3.org/ns/shacl#severity
<http://www.w3.org/ns/shacl#severity> rdfs:domain <http://www.w3.org/ns/shacl#Shape> ;
                                      rdfs:range <http://www.w3.org/ns/shacl#Severity> .


###  http://www.w3.org/ns/shacl#shapesGraph
<http://www.w3.org/ns/shacl#shapesGraph> rdfs:domain owl:Ontology ;
                                         rdfs:range owl:Ontology .


###  http://www.w3.org/ns/shacl#sourceConstraintComponent
<http://www.w3.org/ns/shacl#sourceConstraintComponent> rdfs:domain <http://www.w3.org/ns/shacl#AbstractResult> ;
                                                       rdfs:range <http://www.w3.org/ns/shacl#ConstraintComponent> .


###  http://www.w3.org/ns/shacl#sourceShape
<http://www.w3.org/ns/shacl#sourceShape> rdfs:domain <http://www.w3.org/ns/shacl#AbstractResult> ;
                                         rdfs:range <http://www.w3.org/ns/shacl#Shape> .


###  http://www.w3.org/ns/shacl#sparql
<http://www.w3.org/ns/shacl#sparql> rdfs:domain <http://www.w3.org/ns/shacl#Shape> ;
                                    rdfs:range <http://www.w3.org/ns/shacl#SPARQLConstraint> .


###  http://www.w3.org/ns/shacl#suggestedShapesGraph
<http://www.w3.org/ns/shacl#suggestedShapesGraph> rdfs:domain owl:Ontology ;
                                                  rdfs:range owl:Ontology .


###  http://www.w3.org/ns/shacl#target
<http://www.w3.org/ns/shacl#target> rdfs:domain <http://www.w3.org/ns/shacl#Shape> ;
                                    rdfs:range <http://www.w3.org/ns/shacl#Target> .


###  http://www.w3.org/ns/shacl#targetClass
<http://www.w3.org/ns/shacl#targetClass> rdfs:domain <http://www.w3.org/ns/shacl#Shape> ;
                                         rdfs:range rdfs:Class .


###  http://www.w3.org/ns/shacl#targetObjectsOf
<http://www.w3.org/ns/shacl#targetObjectsOf> rdfs:domain <http://www.w3.org/ns/shacl#Shape> ;
                                             rdfs:range rdf:Property .


###  http://www.w3.org/ns/shacl#targetSubjectsOf
<http://www.w3.org/ns/shacl#targetSubjectsOf> rdfs:domain <http://www.w3.org/ns/shacl#Shape> ;
                                              rdfs:range rdf:Property .


###  http://www.w3.org/ns/shacl#validator
<http://www.w3.org/ns/shacl#validator> rdfs:domain <http://www.w3.org/ns/shacl#ConstraintComponent> ;
                                       rdfs:range <http://www.w3.org/ns/shacl#Validator> .


###  http://www.w3.org/ns/shacl#xone
<http://www.w3.org/ns/shacl#xone> rdfs:range rdf:List .


###  http://www.w3.org/ns/shacl#zeroOrMorePath
<http://www.w3.org/ns/shacl#zeroOrMorePath> rdfs:range rdfs:Resource .


###  http://www.w3.org/ns/shacl#zeroOrOnePath
<http://www.w3.org/ns/shacl#zeroOrOnePath> rdfs:range rdfs:Resource .


###  https://data.digichecks.eu/def/decisionOutcome
:decisionOutcome rdf:type owl:ObjectProperty ;
                 rdfs:range xsd:enumeration .


###  https://data.digichecks.eu/def/hasAsOutput
:hasAsOutput rdf:type owl:ObjectProperty .


###  https://data.digichecks.eu/def/hasParcel
:hasParcel rdf:type owl:ObjectProperty .


###  https://data.digichecks.eu/def/hasPermitRequest
:hasPermitRequest rdf:type owl:ObjectProperty .


###  https://data.digichecks.eu/def/hasSource
:hasSource rdf:type owl:ObjectProperty .


###  https://data.digichecks.eu/def/hasVerificationMethod
:hasVerificationMethod rdf:type owl:ObjectProperty .


###  https://data.digichecks.eu/def/isAddressFor
:isAddressFor rdf:type owl:ObjectProperty ;
              owl:inverseOf <http://www.w3.org/2006/vcard/ns#hasAddress> .


###  https://data.digichecks.eu/def/isAllocationfor
:isAllocationfor rdf:type owl:ObjectProperty .


###  https://data.digichecks.eu/def/isCollectedIn
:isCollectedIn rdf:type owl:ObjectProperty .


###  https://data.digichecks.eu/def/isControlledBy
:isControlledBy rdf:type owl:ObjectProperty .


###  https://data.digichecks.eu/def/isDecisionFor
:isDecisionFor rdf:type owl:ObjectProperty .


###  https://data.digichecks.eu/def/isDerivedIn
:isDerivedIn rdf:type owl:ObjectProperty .


###  https://data.digichecks.eu/def/isExpressedAs
:isExpressedAs rdf:type owl:ObjectProperty .


###  https://data.digichecks.eu/def/isGeometryOf
:isGeometryOf rdf:type owl:ObjectProperty ;
              owl:inverseOf <http://www.opengis.net/ont/geosparql#hasGeometry> .


###  https://data.digichecks.eu/def/isInputFor
:isInputFor rdf:type owl:ObjectProperty .


###  https://data.digichecks.eu/def/isMadeBy
:isMadeBy rdf:type owl:ObjectProperty .


###  https://data.digichecks.eu/def/isParcelFor
:isParcelFor rdf:type owl:ObjectProperty ;
             owl:inverseOf :hasParcel .


###  https://data.digichecks.eu/def/isPermitFor
:isPermitFor rdf:type owl:ObjectProperty ;
             owl:inverseOf :isRequestForPermit .


###  https://data.digichecks.eu/def/isPermitForRequest
:isPermitForRequest rdf:type owl:ObjectProperty ;
                    owl:inverseOf :hasPermitRequest .


###  https://data.digichecks.eu/def/isRequestForPermit
:isRequestForPermit rdf:type owl:ObjectProperty .


###  https://data.digichecks.eu/def/isSubmittedBy
:isSubmittedBy rdf:type owl:ObjectProperty .


###  https://data.digichecks.eu/def/isVerifiedIn
:isVerifiedIn rdf:type owl:ObjectProperty .


###  https://data.digichecks.eu/def/logicalOperator
:logicalOperator rdf:type owl:ObjectProperty ;
                 rdfs:range xsd:enumeration .


###  https://data.digichecks.eu/def/shallBeCompliantWith
:shallBeCompliantWith rdf:type owl:ObjectProperty .


###  https://data.digichecks.eu/def/wasDescribedBy
:wasDescribedBy rdf:type owl:ObjectProperty .


###  https://w3id.org/sml/def#hasPart
<https://w3id.org/sml/def#hasPart> rdf:type owl:ObjectProperty .


###  https://w3id.org/sml/def#hasRequirement
<https://w3id.org/sml/def#hasRequirement> rdf:type owl:ObjectProperty .


###  https://w3id.org/sml/def#isDescribedBy
<https://w3id.org/sml/def#isDescribedBy> rdf:type owl:ObjectProperty .


#################################################################
#    Data properties
#################################################################

###  http://www.w3.org/2000/01/rdf-schema#comment
rdfs:comment rdf:type owl:DatatypeProperty ;
             rdfs:domain rdfs:Resource ;
             rdfs:range rdfs:Literal ,
                        xsd:string .


###  http://www.w3.org/2002/07/owl#bottomDataProperty
owl:bottomDataProperty rdf:type owl:DatatypeProperty ;
                       rdfs:domain owl:Thing ;
                       rdfs:range rdfs:Literal .


###  http://www.w3.org/2002/07/owl#cardinality
owl:cardinality rdfs:domain owl:Restriction ;
                rdfs:range xsd:nonNegativeInteger .


###  http://www.w3.org/2002/07/owl#maxCardinality
owl:maxCardinality rdfs:domain owl:Restriction ;
                   rdfs:range xsd:nonNegativeInteger .


###  http://www.w3.org/2002/07/owl#maxQualifiedCardinality
owl:maxQualifiedCardinality rdfs:domain owl:Restriction ;
                            rdfs:range xsd:nonNegativeInteger .


###  http://www.w3.org/2002/07/owl#minCardinality
owl:minCardinality rdfs:domain owl:Restriction ;
                   rdfs:range xsd:nonNegativeInteger .


###  http://www.w3.org/2002/07/owl#minQualifiedCardinality
owl:minQualifiedCardinality rdfs:domain owl:Restriction ;
                            rdfs:range xsd:nonNegativeInteger .


###  http://www.w3.org/2002/07/owl#qualifiedCardinality
owl:qualifiedCardinality rdfs:domain owl:Restriction ;
                         rdfs:range xsd:nonNegativeInteger .


###  http://www.w3.org/2002/07/owl#topDataProperty
owl:topDataProperty rdf:type owl:DatatypeProperty ;
                    rdfs:domain owl:Thing ;
                    rdfs:range rdfs:Literal .


###  http://www.w3.org/2004/02/skos/core#prefLabel
<http://www.w3.org/2004/02/skos/core#prefLabel> rdf:type owl:DatatypeProperty ;
                                                rdfs:range xsd:string .


###  http://www.w3.org/ns/shacl#annotationVarName
<http://www.w3.org/ns/shacl#annotationVarName> rdfs:domain <http://www.w3.org/ns/shacl#ResultAnnotation> ;
                                               rdfs:range xsd:string .


###  http://www.w3.org/ns/shacl#ask
<http://www.w3.org/ns/shacl#ask> rdfs:domain <http://www.w3.org/ns/shacl#SPARQLAskExecutable> ;
                                 rdfs:range xsd:string .


###  http://www.w3.org/ns/shacl#closed
<http://www.w3.org/ns/shacl#closed> rdfs:range xsd:boolean .


###  http://www.w3.org/ns/shacl#conforms
<http://www.w3.org/ns/shacl#conforms> rdfs:domain <http://www.w3.org/ns/shacl#ValidationReport> ;
                                      rdfs:range xsd:boolean .


###  http://www.w3.org/ns/shacl#construct
<http://www.w3.org/ns/shacl#construct> rdfs:domain <http://www.w3.org/ns/shacl#SPARQLConstructExecutable> ;
                                       rdfs:range xsd:string .


###  http://www.w3.org/ns/shacl#deactivated
<http://www.w3.org/ns/shacl#deactivated> rdfs:range xsd:boolean .


###  http://www.w3.org/ns/shacl#flags
<http://www.w3.org/ns/shacl#flags> rdfs:range xsd:string .


###  http://www.w3.org/ns/shacl#jsFunctionName
<http://www.w3.org/ns/shacl#jsFunctionName> rdfs:domain <http://www.w3.org/ns/shacl#JSExecutable> ;
                                            rdfs:range xsd:string .


###  http://www.w3.org/ns/shacl#jsLibraryURL
<http://www.w3.org/ns/shacl#jsLibraryURL> rdfs:domain <http://www.w3.org/ns/shacl#JSLibrary> ;
                                          rdfs:range xsd:anyURI .


###  http://www.w3.org/ns/shacl#maxCount
<http://www.w3.org/ns/shacl#maxCount> rdfs:range xsd:integer .


###  http://www.w3.org/ns/shacl#maxLength
<http://www.w3.org/ns/shacl#maxLength> rdfs:range xsd:integer .


###  http://www.w3.org/ns/shacl#minCount
<http://www.w3.org/ns/shacl#minCount> rdfs:range xsd:integer .


###  http://www.w3.org/ns/shacl#minLength
<http://www.w3.org/ns/shacl#minLength> rdfs:range xsd:integer .


###  http://www.w3.org/ns/shacl#namespace
<http://www.w3.org/ns/shacl#namespace> rdfs:domain <http://www.w3.org/ns/shacl#PrefixDeclaration> ;
                                       rdfs:range xsd:anyURI .


###  http://www.w3.org/ns/shacl#optional
<http://www.w3.org/ns/shacl#optional> rdfs:domain <http://www.w3.org/ns/shacl#Parameter> ;
                                      rdfs:range xsd:boolean .


###  http://www.w3.org/ns/shacl#pattern
<http://www.w3.org/ns/shacl#pattern> rdfs:range xsd:string .


###  http://www.w3.org/ns/shacl#prefix
<http://www.w3.org/ns/shacl#prefix> rdfs:domain <http://www.w3.org/ns/shacl#PrefixDeclaration> ;
                                    rdfs:range xsd:string .


###  http://www.w3.org/ns/shacl#qualifiedMaxCount
<http://www.w3.org/ns/shacl#qualifiedMaxCount> rdfs:range xsd:integer .


###  http://www.w3.org/ns/shacl#qualifiedMinCount
<http://www.w3.org/ns/shacl#qualifiedMinCount> rdfs:range xsd:integer .


###  http://www.w3.org/ns/shacl#qualifiedValueShapesDisjoint
<http://www.w3.org/ns/shacl#qualifiedValueShapesDisjoint> rdfs:range xsd:boolean .


###  http://www.w3.org/ns/shacl#select
<http://www.w3.org/ns/shacl#select> rdfs:domain <http://www.w3.org/ns/shacl#SPARQLSelectExecutable> ;
                                    rdfs:range xsd:string .


###  http://www.w3.org/ns/shacl#shapesGraphWellFormed
<http://www.w3.org/ns/shacl#shapesGraphWellFormed> rdfs:domain <http://www.w3.org/ns/shacl#ValidationReport> ;
                                                   rdfs:range xsd:boolean .


###  http://www.w3.org/ns/shacl#uniqueLang
<http://www.w3.org/ns/shacl#uniqueLang> rdfs:range xsd:boolean .


###  http://www.w3.org/ns/shacl#update
<http://www.w3.org/ns/shacl#update> rdfs:domain <http://www.w3.org/ns/shacl#SPARQLUpdateExecutable> ;
                                    rdfs:range xsd:string .


###  https://data.digichecks.eu/def/decisionOutcome
:decisionOutcome rdf:type owl:DatatypeProperty .


###  https://data.digichecks.eu/def/logicalOperator
:logicalOperator rdf:type owl:DatatypeProperty .


###  https://data.digichecks.eu/def/role
:role rdf:type owl:DatatypeProperty .


#################################################################
#    Classes
#################################################################

###  http://w3id.org/gaia-x/participant#Participant
<http://w3id.org/gaia-x/participant#Participant> rdf:type owl:Class .


###  http://www.opengis.net/ont/geosparql#Geometry
<http://www.opengis.net/ont/geosparql#Geometry> rdf:type owl:Class .


###  http://www.w3.org/2000/01/rdf-schema#Class
rdfs:Class rdf:type owl:Class ;
           rdfs:subClassOf rdfs:Resource .


###  http://www.w3.org/2000/01/rdf-schema#Container
rdfs:Container rdf:type owl:Class ;
               rdfs:subClassOf rdfs:Resource .


###  http://www.w3.org/2000/01/rdf-schema#ContainerMembershipProperty
rdfs:ContainerMembershipProperty rdf:type owl:Class ;
                                 rdfs:subClassOf rdf:Property .


###  http://www.w3.org/2000/01/rdf-schema#Datatype
rdfs:Datatype rdf:type owl:Class ;
              rdfs:subClassOf rdfs:Class .


###  http://www.w3.org/2000/01/rdf-schema#Literal
rdfs:Literal rdf:type owl:Class ;
             rdfs:subClassOf rdfs:Resource .


###  http://www.w3.org/2000/01/rdf-schema#Resource
rdfs:Resource rdf:type owl:Class .


###  http://www.w3.org/2001/XMLSchema#enumeration
xsd:enumeration rdf:type owl:Class .


###  http://www.w3.org/2002/07/owl#AllDifferent
owl:AllDifferent rdf:type owl:Class ;
                 rdfs:subClassOf rdfs:Resource .


###  http://www.w3.org/2002/07/owl#AllDisjointClasses
owl:AllDisjointClasses rdf:type owl:Class ;
                       rdfs:subClassOf rdfs:Resource .


###  http://www.w3.org/2002/07/owl#AllDisjointProperties
owl:AllDisjointProperties rdf:type owl:Class ;
                          rdfs:subClassOf rdfs:Resource .


###  http://www.w3.org/2002/07/owl#Annotation
owl:Annotation rdf:type owl:Class ;
               rdfs:subClassOf rdfs:Resource .


###  http://www.w3.org/2002/07/owl#AnnotationProperty
owl:AnnotationProperty rdf:type owl:Class ;
                       rdfs:subClassOf rdf:Property .


###  http://www.w3.org/2002/07/owl#AsymmetricProperty
owl:AsymmetricProperty rdf:type owl:Class ;
                       rdfs:subClassOf owl:ObjectProperty .


###  http://www.w3.org/2002/07/owl#Axiom
owl:Axiom rdf:type owl:Class ;
          rdfs:subClassOf rdfs:Resource .


###  http://www.w3.org/2002/07/owl#Class
owl:Class rdf:type owl:Class ;
          rdfs:subClassOf rdfs:Class .


###  http://www.w3.org/2002/07/owl#DataRange
owl:DataRange rdf:type owl:Class ;
              rdfs:subClassOf rdfs:Datatype .


###  http://www.w3.org/2002/07/owl#DatatypeProperty
owl:DatatypeProperty rdf:type owl:Class ;
                     rdfs:subClassOf rdf:Property .


###  http://www.w3.org/2002/07/owl#DeprecatedClass
owl:DeprecatedClass rdf:type owl:Class ;
                    rdfs:subClassOf rdfs:Class .


###  http://www.w3.org/2002/07/owl#DeprecatedProperty
owl:DeprecatedProperty rdf:type owl:Class ;
                       rdfs:subClassOf rdf:Property .


###  http://www.w3.org/2002/07/owl#FunctionalProperty
owl:FunctionalProperty rdf:type owl:Class ;
                       rdfs:subClassOf rdf:Property .


###  http://www.w3.org/2002/07/owl#InverseFunctionalProperty
owl:InverseFunctionalProperty rdf:type owl:Class ;
                              rdfs:subClassOf owl:ObjectProperty .


###  http://www.w3.org/2002/07/owl#IrreflexiveProperty
owl:IrreflexiveProperty rdf:type owl:Class ;
                        rdfs:subClassOf owl:ObjectProperty .


###  http://www.w3.org/2002/07/owl#NamedIndividual
owl:NamedIndividual rdf:type owl:Class ;
                    rdfs:subClassOf owl:Thing .


###  http://www.w3.org/2002/07/owl#NegativePropertyAssertion
owl:NegativePropertyAssertion rdf:type owl:Class ;
                              rdfs:subClassOf rdfs:Resource .


###  http://www.w3.org/2002/07/owl#Nothing
owl:Nothing rdf:type owl:Class ;
            rdfs:subClassOf owl:Thing .


###  http://www.w3.org/2002/07/owl#ObjectProperty
owl:ObjectProperty rdf:type owl:Class ;
                   rdfs:subClassOf rdf:Property .


###  http://www.w3.org/2002/07/owl#Ontology
owl:Ontology rdf:type owl:Class ;
             rdfs:subClassOf rdfs:Resource .


###  http://www.w3.org/2002/07/owl#OntologyProperty
owl:OntologyProperty rdf:type owl:Class ;
                     rdfs:subClassOf rdf:Property .


###  http://www.w3.org/2002/07/owl#ReflexiveProperty
owl:ReflexiveProperty rdf:type owl:Class ;
                      rdfs:subClassOf owl:ObjectProperty .


###  http://www.w3.org/2002/07/owl#Restriction
owl:Restriction rdf:type owl:Class ;
                rdfs:subClassOf owl:Class .


###  http://www.w3.org/2002/07/owl#SymmetricProperty
owl:SymmetricProperty rdf:type owl:Class ;
                      rdfs:subClassOf owl:ObjectProperty .


###  http://www.w3.org/2002/07/owl#Thing
owl:Thing rdf:type owl:Class .


###  http://www.w3.org/2002/07/owl#TransitiveProperty
owl:TransitiveProperty rdf:type owl:Class ;
                       rdfs:subClassOf owl:ObjectProperty .


###  http://www.w3.org/2006/vcard/ns#Address
<http://www.w3.org/2006/vcard/ns#Address> rdf:type owl:Class .


###  http://www.w3.org/ns/prov#Agent
<http://www.w3.org/ns/prov#Agent> rdf:type owl:Class ;
                                  rdfs:subClassOf <http://w3id.org/gaia-x/participant#Participant> .


###  http://www.w3.org/ns/prov#Association
<http://www.w3.org/ns/prov#Association> rdf:type owl:Class ;
                                        rdfs:subClassOf <https://w3id.org/sml/def#InformationObject> .


###  http://www.w3.org/ns/prov#Location
<http://www.w3.org/ns/prov#Location> rdf:type owl:Class .


###  http://www.w3.org/ns/prov#Organization
<http://www.w3.org/ns/prov#Organization> rdf:type owl:Class ;
                                         rdfs:subClassOf <http://www.w3.org/ns/prov#Agent> .


###  http://www.w3.org/ns/prov#Person
<http://www.w3.org/ns/prov#Person> rdf:type owl:Class ;
                                   rdfs:subClassOf <http://www.w3.org/ns/prov#Agent> .


###  http://www.w3.org/ns/shacl#AbstractResult
<http://www.w3.org/ns/shacl#AbstractResult> rdf:type owl:Class ;
                                            rdfs:subClassOf rdfs:Resource .


###  http://www.w3.org/ns/shacl#ConstraintComponent
<http://www.w3.org/ns/shacl#ConstraintComponent> rdf:type owl:Class ;
                                                 rdfs:subClassOf <http://www.w3.org/ns/shacl#Parameterizable> .


###  http://www.w3.org/ns/shacl#Function
<http://www.w3.org/ns/shacl#Function> rdf:type owl:Class ;
                                      rdfs:subClassOf <http://www.w3.org/ns/shacl#Parameterizable> .


###  http://www.w3.org/ns/shacl#JSConstraint
<http://www.w3.org/ns/shacl#JSConstraint> rdf:type owl:Class ;
                                          rdfs:subClassOf <http://www.w3.org/ns/shacl#JSExecutable> .


###  http://www.w3.org/ns/shacl#JSExecutable
<http://www.w3.org/ns/shacl#JSExecutable> rdf:type owl:Class ;
                                          rdfs:subClassOf rdfs:Resource .


###  http://www.w3.org/ns/shacl#JSFunction
<http://www.w3.org/ns/shacl#JSFunction> rdf:type owl:Class ;
                                        rdfs:subClassOf <http://www.w3.org/ns/shacl#Function> ,
                                                        <http://www.w3.org/ns/shacl#JSExecutable> .


###  http://www.w3.org/ns/shacl#JSLibrary
<http://www.w3.org/ns/shacl#JSLibrary> rdf:type owl:Class ;
                                       rdfs:subClassOf rdfs:Resource .


###  http://www.w3.org/ns/shacl#JSRule
<http://www.w3.org/ns/shacl#JSRule> rdf:type owl:Class ;
                                    rdfs:subClassOf <http://www.w3.org/ns/shacl#JSExecutable> ,
                                                    <http://www.w3.org/ns/shacl#Rule> .


###  http://www.w3.org/ns/shacl#JSTarget
<http://www.w3.org/ns/shacl#JSTarget> rdf:type owl:Class ;
                                      rdfs:subClassOf <http://www.w3.org/ns/shacl#JSExecutable> ,
                                                      <http://www.w3.org/ns/shacl#Target> .


###  http://www.w3.org/ns/shacl#JSTargetType
<http://www.w3.org/ns/shacl#JSTargetType> rdf:type owl:Class ;
                                          rdfs:subClassOf <http://www.w3.org/ns/shacl#JSExecutable> ,
                                                          <http://www.w3.org/ns/shacl#TargetType> .


###  http://www.w3.org/ns/shacl#JSValidator
<http://www.w3.org/ns/shacl#JSValidator> rdf:type owl:Class ;
                                         rdfs:subClassOf <http://www.w3.org/ns/shacl#JSExecutable> ,
                                                         <http://www.w3.org/ns/shacl#Validator> .


###  http://www.w3.org/ns/shacl#NodeKind
<http://www.w3.org/ns/shacl#NodeKind> rdf:type owl:Class ;
                                      rdfs:subClassOf rdfs:Resource .


###  http://www.w3.org/ns/shacl#NodeShape
<http://www.w3.org/ns/shacl#NodeShape> rdf:type owl:Class ;
                                       rdfs:subClassOf <http://www.w3.org/ns/shacl#Shape> .


###  http://www.w3.org/ns/shacl#Parameter
<http://www.w3.org/ns/shacl#Parameter> rdf:type owl:Class ;
                                       rdfs:subClassOf <http://www.w3.org/ns/shacl#PropertyShape> .


###  http://www.w3.org/ns/shacl#Parameterizable
<http://www.w3.org/ns/shacl#Parameterizable> rdf:type owl:Class ;
                                             rdfs:subClassOf rdfs:Resource .


###  http://www.w3.org/ns/shacl#PrefixDeclaration
<http://www.w3.org/ns/shacl#PrefixDeclaration> rdf:type owl:Class ;
                                               rdfs:subClassOf rdfs:Resource .


###  http://www.w3.org/ns/shacl#PropertyGroup
<http://www.w3.org/ns/shacl#PropertyGroup> rdf:type owl:Class ;
                                           rdfs:subClassOf rdfs:Resource .


###  http://www.w3.org/ns/shacl#PropertyShape
<http://www.w3.org/ns/shacl#PropertyShape> rdf:type owl:Class ;
                                           rdfs:subClassOf <http://www.w3.org/ns/shacl#Shape> .


###  http://www.w3.org/ns/shacl#ResultAnnotation
<http://www.w3.org/ns/shacl#ResultAnnotation> rdf:type owl:Class ;
                                              rdfs:subClassOf rdfs:Resource .


###  http://www.w3.org/ns/shacl#Rule
<http://www.w3.org/ns/shacl#Rule> rdf:type owl:Class ;
                                  rdfs:subClassOf rdfs:Resource .


###  http://www.w3.org/ns/shacl#SPARQLAskExecutable
<http://www.w3.org/ns/shacl#SPARQLAskExecutable> rdf:type owl:Class ;
                                                 rdfs:subClassOf <http://www.w3.org/ns/shacl#SPARQLExecutable> .


###  http://www.w3.org/ns/shacl#SPARQLAskValidator
<http://www.w3.org/ns/shacl#SPARQLAskValidator> rdf:type owl:Class ;
                                                rdfs:subClassOf <http://www.w3.org/ns/shacl#SPARQLAskExecutable> ,
                                                                <http://www.w3.org/ns/shacl#Validator> .


###  http://www.w3.org/ns/shacl#SPARQLConstraint
<http://www.w3.org/ns/shacl#SPARQLConstraint> rdf:type owl:Class ;
                                              rdfs:subClassOf <http://www.w3.org/ns/shacl#SPARQLSelectExecutable> .


###  http://www.w3.org/ns/shacl#SPARQLConstructExecutable
<http://www.w3.org/ns/shacl#SPARQLConstructExecutable> rdf:type owl:Class ;
                                                       rdfs:subClassOf <http://www.w3.org/ns/shacl#SPARQLExecutable> .


###  http://www.w3.org/ns/shacl#SPARQLExecutable
<http://www.w3.org/ns/shacl#SPARQLExecutable> rdf:type owl:Class ;
                                              rdfs:subClassOf rdfs:Resource .


###  http://www.w3.org/ns/shacl#SPARQLFunction
<http://www.w3.org/ns/shacl#SPARQLFunction> rdf:type owl:Class ;
                                            rdfs:subClassOf <http://www.w3.org/ns/shacl#Function> ,
                                                            <http://www.w3.org/ns/shacl#SPARQLAskExecutable> ,
                                                            <http://www.w3.org/ns/shacl#SPARQLSelectExecutable> .


###  http://www.w3.org/ns/shacl#SPARQLRule
<http://www.w3.org/ns/shacl#SPARQLRule> rdf:type owl:Class ;
                                        rdfs:subClassOf <http://www.w3.org/ns/shacl#Rule> ,
                                                        <http://www.w3.org/ns/shacl#SPARQLConstructExecutable> .


###  http://www.w3.org/ns/shacl#SPARQLSelectExecutable
<http://www.w3.org/ns/shacl#SPARQLSelectExecutable> rdf:type owl:Class ;
                                                    rdfs:subClassOf <http://www.w3.org/ns/shacl#SPARQLExecutable> .


###  http://www.w3.org/ns/shacl#SPARQLSelectValidator
<http://www.w3.org/ns/shacl#SPARQLSelectValidator> rdf:type owl:Class ;
                                                   rdfs:subClassOf <http://www.w3.org/ns/shacl#SPARQLSelectExecutable> ,
                                                                   <http://www.w3.org/ns/shacl#Validator> .


###  http://www.w3.org/ns/shacl#SPARQLTarget
<http://www.w3.org/ns/shacl#SPARQLTarget> rdf:type owl:Class ;
                                          rdfs:subClassOf <http://www.w3.org/ns/shacl#SPARQLAskExecutable> ,
                                                          <http://www.w3.org/ns/shacl#SPARQLSelectExecutable> ,
                                                          <http://www.w3.org/ns/shacl#Target> .


###  http://www.w3.org/ns/shacl#SPARQLTargetType
<http://www.w3.org/ns/shacl#SPARQLTargetType> rdf:type owl:Class ;
                                              rdfs:subClassOf <http://www.w3.org/ns/shacl#SPARQLAskExecutable> ,
                                                              <http://www.w3.org/ns/shacl#SPARQLSelectExecutable> ,
                                                              <http://www.w3.org/ns/shacl#TargetType> .


###  http://www.w3.org/ns/shacl#SPARQLUpdateExecutable
<http://www.w3.org/ns/shacl#SPARQLUpdateExecutable> rdf:type owl:Class ;
                                                    rdfs:subClassOf <http://www.w3.org/ns/shacl#SPARQLExecutable> .


###  http://www.w3.org/ns/shacl#Severity
<http://www.w3.org/ns/shacl#Severity> rdf:type owl:Class ;
                                      rdfs:subClassOf rdfs:Resource .


###  http://www.w3.org/ns/shacl#Shape
<http://www.w3.org/ns/shacl#Shape> rdf:type owl:Class ;
                                   rdfs:subClassOf rdfs:Resource .


###  http://www.w3.org/ns/shacl#Target
<http://www.w3.org/ns/shacl#Target> rdf:type owl:Class ;
                                    rdfs:subClassOf rdfs:Resource .


###  http://www.w3.org/ns/shacl#TargetType
<http://www.w3.org/ns/shacl#TargetType> rdf:type owl:Class ;
                                        rdfs:subClassOf rdfs:Class ,
                                                        <http://www.w3.org/ns/shacl#Parameterizable> .


###  http://www.w3.org/ns/shacl#TripleRule
<http://www.w3.org/ns/shacl#TripleRule> rdf:type owl:Class ;
                                        rdfs:subClassOf <http://www.w3.org/ns/shacl#Rule> ;
                                        rdfs:isDefinedBy <http://www.w3.org/ns/shacl#> ;
                                        rdfs:label "A rule based on triple (subject, predicate, object) pattern."@en .


###  http://www.w3.org/ns/shacl#ValidationReport
<http://www.w3.org/ns/shacl#ValidationReport> rdf:type owl:Class ;
                                              rdfs:subClassOf rdfs:Resource .


###  http://www.w3.org/ns/shacl#ValidationResult
<http://www.w3.org/ns/shacl#ValidationResult> rdf:type owl:Class ;
                                              rdfs:subClassOf <http://www.w3.org/ns/shacl#AbstractResult> .


###  http://www.w3.org/ns/shacl#Validator
<http://www.w3.org/ns/shacl#Validator> rdf:type owl:Class ;
                                       rdfs:subClassOf rdfs:Resource .


###  https://data.digichecks.eu/def/Allocation
:Allocation rdf:type owl:Class ;
            rdfs:subClassOf <https://w3id.org/sml/def#InformationObject> .


###  https://data.digichecks.eu/def/Decision
:Decision rdf:type owl:Class ;
          rdfs:subClassOf <https://w3id.org/sml/def#Activity> .


###  https://data.digichecks.eu/def/Document
:Document rdf:type owl:Class ;
          rdfs:subClassOf <https://w3id.org/sml/def#InformationObject> .


###  https://data.digichecks.eu/def/GenericRequirement
:GenericRequirement rdf:type owl:Class ;
                    rdfs:subClassOf <https://w3id.org/sml/def#Requirement> .


###  https://data.digichecks.eu/def/MachineReadableRule
:MachineReadableRule rdf:type owl:Class ;
                     rdfs:subClassOf <https://w3id.org/sml/def#InformationObject> .


###  https://data.digichecks.eu/def/Parcel
:Parcel rdf:type owl:Class .


###  https://data.digichecks.eu/def/Permit
:Permit rdf:type owl:Class ;
        rdfs:subClassOf <https://w3id.org/sml/def#InformationObject> .


###  https://data.digichecks.eu/def/PermitRequest
:PermitRequest rdf:type owl:Class ;
               rdfs:subClassOf <https://w3id.org/sml/def#InformationObject> .


###  https://data.digichecks.eu/def/Project
:Project rdf:type owl:Class ;
         rdfs:subClassOf <https://w3id.org/sml/def#Entity> .


###  https://data.digichecks.eu/def/ProjectRequirement
:ProjectRequirement rdf:type owl:Class ;
                    rdfs:subClassOf <https://w3id.org/sml/def#Requirement> .


###  https://data.digichecks.eu/def/Verification
:Verification rdf:type owl:Class ;
              rdfs:subClassOf <https://w3id.org/sml/def#Activity> .


###  https://data.digichecks.eu/def/VerificationMethod
:VerificationMethod rdf:type owl:Class ;
                    rdfs:subClassOf <https://w3id.org/sml/def#Activity> .


###  https://w3id.org/idsa/core/Resource
<https://w3id.org/idsa/core/Resource> rdf:type owl:Class .


###  https://w3id.org/sml/def#AbstractConcept
<https://w3id.org/sml/def#AbstractConcept> rdf:type owl:Class ;
                                           rdfs:subClassOf <https://w3id.org/sml/def#TopConcept> .


###  https://w3id.org/sml/def#Activity
<https://w3id.org/sml/def#Activity> rdf:type owl:Class ;
                                    rdfs:subClassOf <https://w3id.org/sml/def#Entity> .


###  https://w3id.org/sml/def#ConceptType
<https://w3id.org/sml/def#ConceptType> rdf:type owl:Class ;
                                       rdfs:subClassOf <https://w3id.org/sml/def#Type> .


###  https://w3id.org/sml/def#ConcreteConcept
<https://w3id.org/sml/def#ConcreteConcept> rdf:type owl:Class ;
                                           rdfs:subClassOf <https://w3id.org/sml/def#TopConcept> .


###  https://w3id.org/sml/def#Entity
<https://w3id.org/sml/def#Entity> rdf:type owl:Class ;
                                  rdfs:subClassOf <https://w3id.org/sml/def#ConcreteConcept> .


###  https://w3id.org/sml/def#EnumerationType
<https://w3id.org/sml/def#EnumerationType> rdf:type owl:Class ;
                                           rdfs:subClassOf <https://w3id.org/sml/def#Type> .


###  https://w3id.org/sml/def#Event
<https://w3id.org/sml/def#Event> rdf:type owl:Class ;
                                 rdfs:subClassOf <https://w3id.org/sml/def#ConcreteConcept> .


###  https://w3id.org/sml/def#GeometricEntity
<https://w3id.org/sml/def#GeometricEntity> rdf:type owl:Class ;
                                           rdfs:subClassOf <https://w3id.org/sml/def#Representation> .


###  https://w3id.org/sml/def#InformationObject
<https://w3id.org/sml/def#InformationObject> rdf:type owl:Class ;
                                             rdfs:subClassOf <https://w3id.org/sml/def#Object> .


###  https://w3id.org/sml/def#Object
<https://w3id.org/sml/def#Object> rdf:type owl:Class ;
                                  rdfs:subClassOf <https://w3id.org/sml/def#Entity> .


###  https://w3id.org/sml/def#Objectification
<https://w3id.org/sml/def#Objectification> rdf:type owl:Class ;
                                           rdfs:subClassOf <https://w3id.org/sml/def#AbstractConcept> .


###  https://w3id.org/sml/def#PhysicalObject
<https://w3id.org/sml/def#PhysicalObject> rdf:type owl:Class ;
                                          rdfs:subClassOf <https://w3id.org/sml/def#Object> .


###  https://w3id.org/sml/def#QualityValue
<https://w3id.org/sml/def#QualityValue> rdf:type owl:Class ;
                                        rdfs:subClassOf <https://w3id.org/sml/def#Objectification> .


###  https://w3id.org/sml/def#QuantityValue
<https://w3id.org/sml/def#QuantityValue> rdf:type owl:Class ;
                                         rdfs:subClassOf <https://w3id.org/sml/def#Objectification> .


###  https://w3id.org/sml/def#RelationReference
<https://w3id.org/sml/def#RelationReference> rdf:type owl:Class ;
                                             rdfs:subClassOf <https://w3id.org/sml/def#Objectification> .


###  https://w3id.org/sml/def#Representation
<https://w3id.org/sml/def#Representation> rdf:type owl:Class ;
                                          rdfs:subClassOf <https://w3id.org/sml/def#InformationObject> .


###  https://w3id.org/sml/def#Requirement
<https://w3id.org/sml/def#Requirement> rdf:type owl:Class ;
                                       rdfs:subClassOf <https://w3id.org/sml/def#InformationObject> .


###  https://w3id.org/sml/def#State
<https://w3id.org/sml/def#State> rdf:type owl:Class ;
                                 rdfs:subClassOf <https://w3id.org/sml/def#ConcreteConcept> .


###  https://w3id.org/sml/def#TemporalEntity
<https://w3id.org/sml/def#TemporalEntity> rdf:type owl:Class ;
                                          rdfs:subClassOf <https://w3id.org/sml/def#Representation> .


###  https://w3id.org/sml/def#TopConcept
<https://w3id.org/sml/def#TopConcept> rdf:type owl:Class .


###  https://w3id.org/sml/def#Type
<https://w3id.org/sml/def#Type> rdf:type owl:Class ;
                                rdfs:subClassOf <https://w3id.org/sml/def#AbstractConcept> .


#################################################################
#    Individuals
#################################################################

###  http://purl.org/dc/terms/subject
<http://purl.org/dc/terms/subject> rdf:type owl:NamedIndividual ;
                                   <http://www.w3.org/2004/02/skos/core#prefLabel> "subject" .


###  http://www.opengis.net/ont/geosparql#Geometry
<http://www.opengis.net/ont/geosparql#Geometry> rdf:type owl:NamedIndividual ;
                                                <http://www.w3.org/2004/02/skos/core#prefLabel> "Geometry" .


###  http://www.opengis.net/ont/geosparql#hasGeometry
<http://www.opengis.net/ont/geosparql#hasGeometry> rdf:type owl:NamedIndividual ;
                                                   <http://www.w3.org/2004/02/skos/core#prefLabel> "has geometry" .


###  http://www.w3.org/2000/01/rdf-schema#Class
rdfs:Class rdfs:comment "The class of classes." .


###  http://www.w3.org/2000/01/rdf-schema#Container
rdfs:Container rdfs:comment "The class of RDF containers." .


###  http://www.w3.org/2000/01/rdf-schema#ContainerMembershipProperty
rdfs:ContainerMembershipProperty rdfs:comment "The class of container membership properties, rdf:_1, rdf:_2, ..., all of which are sub-properties of 'member'." .


###  http://www.w3.org/2000/01/rdf-schema#Datatype
rdfs:Datatype rdfs:comment "The class of RDF datatypes." .


###  http://www.w3.org/2000/01/rdf-schema#Literal
rdfs:Literal rdfs:comment "The class of literal values, eg. textual strings and integers." .


###  http://www.w3.org/2000/01/rdf-schema#Resource
rdfs:Resource rdfs:comment "The class resource, everything." .


###  http://www.w3.org/2000/01/rdf-schema#comment
rdfs:comment rdfs:comment "A description of the subject resource." ;
             <http://www.w3.org/2004/02/skos/core#prefLabel> "comment" .


###  http://www.w3.org/2000/01/rdf-schema#domain
rdfs:domain rdfs:comment "A domain of the subject property." .


###  http://www.w3.org/2000/01/rdf-schema#isDefinedBy
rdfs:isDefinedBy rdfs:comment "The definition of the subject resource." .


###  http://www.w3.org/2000/01/rdf-schema#label
rdfs:label rdfs:comment "A human-readable name for the subject." .


###  http://www.w3.org/2000/01/rdf-schema#member
rdfs:member rdfs:comment "A member of the subject resource." .


###  http://www.w3.org/2000/01/rdf-schema#range
rdfs:range rdfs:comment "A range of the subject property." .


###  http://www.w3.org/2000/01/rdf-schema#seeAlso
rdfs:seeAlso rdfs:comment "Further information about the subject resource." .


###  http://www.w3.org/2000/01/rdf-schema#subClassOf
rdfs:subClassOf rdfs:comment "The subject is a subclass of a class." .


###  http://www.w3.org/2000/01/rdf-schema#subPropertyOf
rdfs:subPropertyOf rdfs:comment "The subject is a subproperty of a property." .


###  http://www.w3.org/2002/07/owl#AllDifferent
owl:AllDifferent rdfs:comment "The class of collections of pairwise different individuals." .


###  http://www.w3.org/2002/07/owl#AllDisjointClasses
owl:AllDisjointClasses rdfs:comment "The class of collections of pairwise disjoint classes." .


###  http://www.w3.org/2002/07/owl#AllDisjointProperties
owl:AllDisjointProperties rdfs:comment "The class of collections of pairwise disjoint properties." .


###  http://www.w3.org/2002/07/owl#Annotation
owl:Annotation rdfs:comment "The class of annotated annotations for which the RDF serialization consists of an annotated subject, predicate and object." .


###  http://www.w3.org/2002/07/owl#AnnotationProperty
owl:AnnotationProperty rdfs:comment "The class of annotation properties." .


###  http://www.w3.org/2002/07/owl#AsymmetricProperty
owl:AsymmetricProperty rdfs:comment "The class of asymmetric properties." .


###  http://www.w3.org/2002/07/owl#Axiom
owl:Axiom rdfs:comment "The class of annotated axioms for which the RDF serialization consists of an annotated subject, predicate and object." .


###  http://www.w3.org/2002/07/owl#Class
owl:Class rdfs:comment "The class of OWL classes." .


###  http://www.w3.org/2002/07/owl#DataRange
owl:DataRange rdfs:comment "The class of OWL data ranges, which are special kinds of datatypes. Note: The use of the IRI owl:DataRange has been deprecated as of OWL 2. The IRI rdfs:Datatype SHOULD be used instead." .


###  http://www.w3.org/2002/07/owl#DatatypeProperty
owl:DatatypeProperty rdfs:comment "The class of data properties." .


###  http://www.w3.org/2002/07/owl#DeprecatedClass
owl:DeprecatedClass rdfs:comment "The class of deprecated classes." .


###  http://www.w3.org/2002/07/owl#DeprecatedProperty
owl:DeprecatedProperty rdfs:comment "The class of deprecated properties." .


###  http://www.w3.org/2002/07/owl#FunctionalProperty
owl:FunctionalProperty rdfs:comment "The class of functional properties." .


###  http://www.w3.org/2002/07/owl#InverseFunctionalProperty
owl:InverseFunctionalProperty rdfs:comment "The class of inverse-functional properties." .


###  http://www.w3.org/2002/07/owl#IrreflexiveProperty
owl:IrreflexiveProperty rdfs:comment "The class of irreflexive properties." .


###  http://www.w3.org/2002/07/owl#NamedIndividual
owl:NamedIndividual rdfs:comment "The class of named individuals." .


###  http://www.w3.org/2002/07/owl#NegativePropertyAssertion
owl:NegativePropertyAssertion rdfs:comment "The class of negative property assertions." .


###  http://www.w3.org/2002/07/owl#Nothing
owl:Nothing rdfs:comment "This is the empty class." .


###  http://www.w3.org/2002/07/owl#ObjectProperty
owl:ObjectProperty rdfs:comment "The class of object properties." .


###  http://www.w3.org/2002/07/owl#Ontology
owl:Ontology rdfs:comment "The class of ontologies." .


###  http://www.w3.org/2002/07/owl#OntologyProperty
owl:OntologyProperty rdfs:comment "The class of ontology properties." .


###  http://www.w3.org/2002/07/owl#ReflexiveProperty
owl:ReflexiveProperty rdfs:comment "The class of reflexive properties." .


###  http://www.w3.org/2002/07/owl#Restriction
owl:Restriction rdfs:comment "The class of property restrictions." .


###  http://www.w3.org/2002/07/owl#SymmetricProperty
owl:SymmetricProperty rdfs:comment "The class of symmetric properties." .


###  http://www.w3.org/2002/07/owl#Thing
owl:Thing rdfs:comment "The class of OWL individuals." .


###  http://www.w3.org/2002/07/owl#TransitiveProperty
owl:TransitiveProperty rdfs:comment "The class of transitive properties." .


###  http://www.w3.org/2002/07/owl#allValuesFrom
owl:allValuesFrom rdfs:comment "The property that determines the class that a universal property restriction refers to." .


###  http://www.w3.org/2002/07/owl#annotatedProperty
owl:annotatedProperty rdfs:comment "The property that determines the predicate of an annotated axiom or annotated annotation." .


###  http://www.w3.org/2002/07/owl#annotatedSource
owl:annotatedSource rdfs:comment "The property that determines the subject of an annotated axiom or annotated annotation." .


###  http://www.w3.org/2002/07/owl#annotatedTarget
owl:annotatedTarget rdfs:comment "The property that determines the object of an annotated axiom or annotated annotation." .


###  http://www.w3.org/2002/07/owl#assertionProperty
owl:assertionProperty rdfs:comment "The property that determines the predicate of a negative property assertion." .


###  http://www.w3.org/2002/07/owl#backwardCompatibleWith
owl:backwardCompatibleWith rdfs:comment "The annotation property that indicates that a given ontology is backward compatible with another ontology." .


###  http://www.w3.org/2002/07/owl#bottomDataProperty
owl:bottomDataProperty rdfs:comment "The data property that does not relate any individual to any data value." .


###  http://www.w3.org/2002/07/owl#bottomObjectProperty
owl:bottomObjectProperty rdfs:comment "The object property that does not relate any two individuals." .


###  http://www.w3.org/2002/07/owl#cardinality
owl:cardinality rdfs:comment "The property that determines the cardinality of an exact cardinality restriction." .


###  http://www.w3.org/2002/07/owl#complementOf
owl:complementOf rdfs:comment "The property that determines that a given class is the complement of another class." .


###  http://www.w3.org/2002/07/owl#datatypeComplementOf
owl:datatypeComplementOf rdfs:comment "The property that determines that a given data range is the complement of another data range with respect to the data domain." .


###  http://www.w3.org/2002/07/owl#deprecated
owl:deprecated rdfs:comment "The annotation property that indicates that a given entity has been deprecated." .


###  http://www.w3.org/2002/07/owl#differentFrom
owl:differentFrom rdfs:comment "The property that determines that two given individuals are different." .


###  http://www.w3.org/2002/07/owl#disjointUnionOf
owl:disjointUnionOf rdfs:comment "The property that determines that a given class is equivalent to the disjoint union of a collection of other classes." .


###  http://www.w3.org/2002/07/owl#disjointWith
owl:disjointWith rdfs:comment "The property that determines that two given classes are disjoint." .


###  http://www.w3.org/2002/07/owl#distinctMembers
owl:distinctMembers rdfs:comment "The property that determines the collection of pairwise different individuals in a owl:AllDifferent axiom." .


###  http://www.w3.org/2002/07/owl#equivalentClass
owl:equivalentClass rdfs:comment "The property that determines that two given classes are equivalent, and that is used to specify datatype definitions." .


###  http://www.w3.org/2002/07/owl#equivalentProperty
owl:equivalentProperty rdfs:comment "The property that determines that two given properties are equivalent." .


###  http://www.w3.org/2002/07/owl#hasKey
owl:hasKey rdfs:comment "The property that determines the collection of properties that jointly build a key." .


###  http://www.w3.org/2002/07/owl#hasSelf
owl:hasSelf rdfs:comment "The property that determines the property that a self restriction refers to." .


###  http://www.w3.org/2002/07/owl#hasValue
owl:hasValue rdfs:comment "The property that determines the individual that a has-value restriction refers to." .


###  http://www.w3.org/2002/07/owl#imports
owl:imports rdfs:comment "The property that is used for importing other ontologies into a given ontology." .


###  http://www.w3.org/2002/07/owl#incompatibleWith
owl:incompatibleWith rdfs:comment "The annotation property that indicates that a given ontology is incompatible with another ontology." .


###  http://www.w3.org/2002/07/owl#intersectionOf
owl:intersectionOf rdfs:comment "The property that determines the collection of classes or data ranges that build an intersection." .


###  http://www.w3.org/2002/07/owl#inverseOf
owl:inverseOf rdfs:comment "The property that determines that two given properties are inverse." .


###  http://www.w3.org/2002/07/owl#maxCardinality
owl:maxCardinality rdfs:comment "The property that determines the cardinality of a maximum cardinality restriction." .


###  http://www.w3.org/2002/07/owl#maxQualifiedCardinality
owl:maxQualifiedCardinality rdfs:comment "The property that determines the cardinality of a maximum qualified cardinality restriction." .


###  http://www.w3.org/2002/07/owl#members
owl:members rdfs:comment "The property that determines the collection of members in either a owl:AllDifferent, owl:AllDisjointClasses or owl:AllDisjointProperties axiom." .


###  http://www.w3.org/2002/07/owl#minCardinality
owl:minCardinality rdfs:comment "The property that determines the cardinality of a minimum cardinality restriction." .


###  http://www.w3.org/2002/07/owl#minQualifiedCardinality
owl:minQualifiedCardinality rdfs:comment "The property that determines the cardinality of a minimum qualified cardinality restriction." .


###  http://www.w3.org/2002/07/owl#onClass
owl:onClass rdfs:comment "The property that determines the class that a qualified object cardinality restriction refers to." .


###  http://www.w3.org/2002/07/owl#onDataRange
owl:onDataRange rdfs:comment "The property that determines the data range that a qualified data cardinality restriction refers to." .


###  http://www.w3.org/2002/07/owl#onDatatype
owl:onDatatype rdfs:comment "The property that determines the datatype that a datatype restriction refers to." .


###  http://www.w3.org/2002/07/owl#onProperties
owl:onProperties rdfs:comment "The property that determines the n-tuple of properties that a property restriction on an n-ary data range refers to." .


###  http://www.w3.org/2002/07/owl#onProperty
owl:onProperty rdfs:comment "The property that determines the property that a property restriction refers to." .


###  http://www.w3.org/2002/07/owl#oneOf
owl:oneOf rdfs:comment "The property that determines the collection of individuals or data values that build an enumeration." .


###  http://www.w3.org/2002/07/owl#priorVersion
owl:priorVersion rdfs:comment "The annotation property that indicates the predecessor ontology of a given ontology." .


###  http://www.w3.org/2002/07/owl#propertyChainAxiom
owl:propertyChainAxiom rdfs:comment "The property that determines the n-tuple of properties that build a sub property chain of a given property." .


###  http://www.w3.org/2002/07/owl#propertyDisjointWith
owl:propertyDisjointWith rdfs:comment "The property that determines that two given properties are disjoint." .


###  http://www.w3.org/2002/07/owl#qualifiedCardinality
owl:qualifiedCardinality rdfs:comment "The property that determines the cardinality of an exact qualified cardinality restriction." .


###  http://www.w3.org/2002/07/owl#sameAs
owl:sameAs rdfs:comment "The property that determines that two given individuals are equal." .


###  http://www.w3.org/2002/07/owl#someValuesFrom
owl:someValuesFrom rdfs:comment "The property that determines the class that an existential property restriction refers to." .


###  http://www.w3.org/2002/07/owl#sourceIndividual
owl:sourceIndividual rdfs:comment "The property that determines the subject of a negative property assertion." .


###  http://www.w3.org/2002/07/owl#targetIndividual
owl:targetIndividual rdfs:comment "The property that determines the object of a negative object property assertion." .


###  http://www.w3.org/2002/07/owl#targetValue
owl:targetValue rdfs:comment "The property that determines the value of a negative data property assertion." .


###  http://www.w3.org/2002/07/owl#topDataProperty
owl:topDataProperty rdfs:comment "The data property that relates every individual to every data value." .


###  http://www.w3.org/2002/07/owl#topObjectProperty
owl:topObjectProperty rdfs:comment "The object property that relates every two individuals." .


###  http://www.w3.org/2002/07/owl#unionOf
owl:unionOf rdfs:comment "The property that determines the collection of classes or data ranges that build a union." .


###  http://www.w3.org/2002/07/owl#versionIRI
owl:versionIRI rdfs:comment "The property that identifies the version IRI of an ontology." .


###  http://www.w3.org/2002/07/owl#versionInfo
owl:versionInfo rdfs:comment "The annotation property that provides version information for an ontology or another OWL construct." .


###  http://www.w3.org/2002/07/owl#withRestrictions
owl:withRestrictions rdfs:comment "The property that determines the collection of facet-value pairs that define a datatype restriction." .


###  http://www.w3.org/2004/02/skos/core#prefLabel
<http://www.w3.org/2004/02/skos/core#prefLabel> rdf:type owl:NamedIndividual ;
                                                <http://www.w3.org/2004/02/skos/core#prefLabel> "pref label" .


###  http://www.w3.org/2006/vcard/ns#Address
<http://www.w3.org/2006/vcard/ns#Address> rdf:type owl:NamedIndividual ;
                                          <http://www.w3.org/2004/02/skos/core#prefLabel> "Address" .


###  http://www.w3.org/2006/vcard/ns#hasAddress
<http://www.w3.org/2006/vcard/ns#hasAddress> rdf:type owl:NamedIndividual ;
                                             <http://www.w3.org/2004/02/skos/core#prefLabel> "has address" .


###  http://www.w3.org/ns/prov#Agent
<http://www.w3.org/ns/prov#Agent> rdf:type owl:NamedIndividual ;
                                  <http://www.w3.org/2004/02/skos/core#prefLabel> "Agent" .


###  http://www.w3.org/ns/prov#Association
<http://www.w3.org/ns/prov#Association> rdf:type owl:NamedIndividual ;
                                        <http://www.w3.org/2004/02/skos/core#prefLabel> "Association" .


###  http://www.w3.org/ns/prov#Location
<http://www.w3.org/ns/prov#Location> rdf:type owl:NamedIndividual ;
                                     <http://www.w3.org/2004/02/skos/core#prefLabel> "Location" .


###  http://www.w3.org/ns/prov#Organization
<http://www.w3.org/ns/prov#Organization> rdf:type owl:NamedIndividual ;
                                         <http://www.w3.org/2004/02/skos/core#prefLabel> "Organization" .


###  http://www.w3.org/ns/prov#Person
<http://www.w3.org/ns/prov#Person> rdf:type owl:NamedIndividual ;
                                   <http://www.w3.org/2004/02/skos/core#prefLabel> "Person" .


###  http://www.w3.org/ns/prov#actedOnBehalfOf
<http://www.w3.org/ns/prov#actedOnBehalfOf> rdf:type owl:NamedIndividual ;
                                            <http://www.w3.org/2004/02/skos/core#prefLabel> "acted on behalf of" .


###  http://www.w3.org/ns/prov#agent
<http://www.w3.org/ns/prov#agent> rdf:type owl:NamedIndividual ;
                                  <http://www.w3.org/2004/02/skos/core#prefLabel> "agent" .


###  http://www.w3.org/ns/prov#atLocation
<http://www.w3.org/ns/prov#atLocation> rdf:type owl:NamedIndividual ;
                                       <http://www.w3.org/2004/02/skos/core#prefLabel> "at location" .


###  http://www.w3.org/ns/prov#qualifiedAssociation
<http://www.w3.org/ns/prov#qualifiedAssociation> rdf:type owl:NamedIndividual ;
                                                 <http://www.w3.org/2004/02/skos/core#prefLabel> "qualified association" .


###  http://www.w3.org/ns/prov#wasAssociatedWith
<http://www.w3.org/ns/prov#wasAssociatedWith> rdf:type owl:NamedIndividual ;
                                              <http://www.w3.org/2004/02/skos/core#prefLabel> "was associated with" .


###  http://www.w3.org/ns/shacl#
<http://www.w3.org/ns/shacl#> <http://www.w3.org/ns/shacl#declare> _:genid1 ;
                              <http://www.w3.org/ns/shacl#suggestedShapesGraph> <http://www.w3.org/ns/shacl-shacl#> .

_:genid1 <http://www.w3.org/ns/shacl#namespace> "http://www.w3.org/ns/shacl#" ;
          <http://www.w3.org/ns/shacl#prefix> "sh" .


###  http://www.w3.org/ns/shacl#AbstractResult
<http://www.w3.org/ns/shacl#AbstractResult> rdfs:comment "The base class of validation results, typically not instantiated directly."@en .


###  http://www.w3.org/ns/shacl#AndConstraintComponent
<http://www.w3.org/ns/shacl#AndConstraintComponent> rdf:type <http://www.w3.org/ns/shacl#ConstraintComponent> ;
                                                    <http://www.w3.org/ns/shacl#parameter> <http://www.w3.org/ns/shacl#AndConstraintComponent-and> ;
                                                    rdfs:comment "A constraint component that can be used to test whether a value node conforms to all members of a provided list of shapes."@en ;
                                                    rdfs:isDefinedBy <http://www.w3.org/ns/shacl#> ;
                                                    rdfs:label "And constraint component"@en .


###  http://www.w3.org/ns/shacl#AndConstraintComponent-and
<http://www.w3.org/ns/shacl#AndConstraintComponent-and> rdf:type <http://www.w3.org/ns/shacl#Parameter> ;
                                                        <http://www.w3.org/ns/shacl#path> <http://www.w3.org/ns/shacl#and> ;
                                                        rdfs:isDefinedBy <http://www.w3.org/ns/shacl#> .


###  http://www.w3.org/ns/shacl#BlankNode
<http://www.w3.org/ns/shacl#BlankNode> rdf:type <http://www.w3.org/ns/shacl#NodeKind> ;
                                       rdfs:comment "The node kind of all blank nodes."@en ;
                                       rdfs:isDefinedBy <http://www.w3.org/ns/shacl#> ;
                                       rdfs:label "Blank node"@en .


###  http://www.w3.org/ns/shacl#BlankNodeOrIRI
<http://www.w3.org/ns/shacl#BlankNodeOrIRI> rdf:type <http://www.w3.org/ns/shacl#NodeKind> ;
                                            rdfs:comment "The node kind of all blank nodes or IRIs."@en ;
                                            rdfs:isDefinedBy <http://www.w3.org/ns/shacl#> ;
                                            rdfs:label "Blank node or IRI"@en .


###  http://www.w3.org/ns/shacl#BlankNodeOrLiteral
<http://www.w3.org/ns/shacl#BlankNodeOrLiteral> rdf:type <http://www.w3.org/ns/shacl#NodeKind> ;
                                                rdfs:comment "The node kind of all blank nodes or literals."@en ;
                                                rdfs:isDefinedBy <http://www.w3.org/ns/shacl#> ;
                                                rdfs:label "Blank node or literal"@en .


###  http://www.w3.org/ns/shacl#ClassConstraintComponent
<http://www.w3.org/ns/shacl#ClassConstraintComponent> rdf:type <http://www.w3.org/ns/shacl#ConstraintComponent> ;
                                                      <http://www.w3.org/ns/shacl#parameter> <http://www.w3.org/ns/shacl#ClassConstraintComponent-class> ;
                                                      rdfs:comment "A constraint component that can be used to verify that each value node is an instance of a given type."@en ;
                                                      rdfs:isDefinedBy <http://www.w3.org/ns/shacl#> ;
                                                      rdfs:label "Class constraint component"@en .


###  http://www.w3.org/ns/shacl#ClassConstraintComponent-class
<http://www.w3.org/ns/shacl#ClassConstraintComponent-class> rdf:type <http://www.w3.org/ns/shacl#Parameter> ;
                                                            <http://www.w3.org/ns/shacl#nodeKind> <http://www.w3.org/ns/shacl#IRI> ;
                                                            <http://www.w3.org/ns/shacl#path> <http://www.w3.org/ns/shacl#class> ;
                                                            rdfs:isDefinedBy <http://www.w3.org/ns/shacl#> .


###  http://www.w3.org/ns/shacl#ClosedConstraintComponent
<http://www.w3.org/ns/shacl#ClosedConstraintComponent> rdf:type <http://www.w3.org/ns/shacl#ConstraintComponent> ;
                                                       <http://www.w3.org/ns/shacl#parameter> <http://www.w3.org/ns/shacl#ClosedConstraintComponent-closed> ,
                                                                                              <http://www.w3.org/ns/shacl#ClosedConstraintComponent-ignoredProperties> ;
                                                       rdfs:comment "A constraint component that can be used to indicate that focus nodes must only have values for those properties that have been explicitly enumerated via sh:property/sh:path."@en ;
                                                       rdfs:isDefinedBy <http://www.w3.org/ns/shacl#> ;
                                                       rdfs:label "Closed constraint component"@en .


###  http://www.w3.org/ns/shacl#ClosedConstraintComponent-closed
<http://www.w3.org/ns/shacl#ClosedConstraintComponent-closed> rdf:type <http://www.w3.org/ns/shacl#Parameter> ;
                                                              <http://www.w3.org/ns/shacl#datatype> xsd:boolean ;
                                                              <http://www.w3.org/ns/shacl#path> <http://www.w3.org/ns/shacl#closed> ;
                                                              rdfs:isDefinedBy <http://www.w3.org/ns/shacl#> .


###  http://www.w3.org/ns/shacl#ClosedConstraintComponent-ignoredProperties
<http://www.w3.org/ns/shacl#ClosedConstraintComponent-ignoredProperties> rdf:type <http://www.w3.org/ns/shacl#Parameter> ;
                                                                         <http://www.w3.org/ns/shacl#path> <http://www.w3.org/ns/shacl#ignoredProperties> ;
                                                                         <http://www.w3.org/ns/shacl#optional> "true"^^xsd:boolean ;
                                                                         rdfs:isDefinedBy <http://www.w3.org/ns/shacl#> .


###  http://www.w3.org/ns/shacl#ConstraintComponent
<http://www.w3.org/ns/shacl#ConstraintComponent> rdfs:comment "The class of constraint components."@en .


###  http://www.w3.org/ns/shacl#DatatypeConstraintComponent
<http://www.w3.org/ns/shacl#DatatypeConstraintComponent> rdf:type <http://www.w3.org/ns/shacl#ConstraintComponent> ;
                                                         <http://www.w3.org/ns/shacl#parameter> <http://www.w3.org/ns/shacl#DatatypeConstraintComponent-datatype> ;
                                                         rdfs:comment "A constraint component that can be used to restrict the datatype of all value nodes."@en ;
                                                         rdfs:isDefinedBy <http://www.w3.org/ns/shacl#> ;
                                                         rdfs:label "Datatype constraint component"@en .


###  http://www.w3.org/ns/shacl#DatatypeConstraintComponent-datatype
<http://www.w3.org/ns/shacl#DatatypeConstraintComponent-datatype> rdf:type <http://www.w3.org/ns/shacl#Parameter> ;
                                                                  <http://www.w3.org/ns/shacl#nodeKind> <http://www.w3.org/ns/shacl#IRI> ;
                                                                  <http://www.w3.org/ns/shacl#path> <http://www.w3.org/ns/shacl#datatype> ;
                                                                  <http://www.w3.org/ns/shacl#maxCount> 1 ;
                                                                  rdfs:isDefinedBy <http://www.w3.org/ns/shacl#> .


###  http://www.w3.org/ns/shacl#DisjointConstraintComponent
<http://www.w3.org/ns/shacl#DisjointConstraintComponent> rdf:type <http://www.w3.org/ns/shacl#ConstraintComponent> ;
                                                         <http://www.w3.org/ns/shacl#parameter> <http://www.w3.org/ns/shacl#DisjointConstraintComponent-disjoint> ;
                                                         rdfs:comment "A constraint component that can be used to verify that the set of value nodes is disjoint with the the set of nodes that have the focus node as subject and the value of a given property as predicate."@en ;
                                                         rdfs:isDefinedBy <http://www.w3.org/ns/shacl#> ;
                                                         rdfs:label "Disjoint constraint component"@en .


###  http://www.w3.org/ns/shacl#DisjointConstraintComponent-disjoint
<http://www.w3.org/ns/shacl#DisjointConstraintComponent-disjoint> rdf:type <http://www.w3.org/ns/shacl#Parameter> ;
                                                                  <http://www.w3.org/ns/shacl#nodeKind> <http://www.w3.org/ns/shacl#IRI> ;
                                                                  <http://www.w3.org/ns/shacl#path> <http://www.w3.org/ns/shacl#disjoint> ;
                                                                  rdfs:isDefinedBy <http://www.w3.org/ns/shacl#> .


###  http://www.w3.org/ns/shacl#EqualsConstraintComponent
<http://www.w3.org/ns/shacl#EqualsConstraintComponent> rdf:type <http://www.w3.org/ns/shacl#ConstraintComponent> ;
                                                       <http://www.w3.org/ns/shacl#parameter> <http://www.w3.org/ns/shacl#EqualsConstraintComponent-equals> ;
                                                       rdfs:comment "A constraint component that can be used to verify that the set of value nodes is equal to the set of nodes that have the focus node as subject and the value of a given property as predicate."@en ;
                                                       rdfs:isDefinedBy <http://www.w3.org/ns/shacl#> ;
                                                       rdfs:label "Equals constraint component"@en .


###  http://www.w3.org/ns/shacl#EqualsConstraintComponent-equals
<http://www.w3.org/ns/shacl#EqualsConstraintComponent-equals> rdf:type <http://www.w3.org/ns/shacl#Parameter> ;
                                                              <http://www.w3.org/ns/shacl#nodeKind> <http://www.w3.org/ns/shacl#IRI> ;
                                                              <http://www.w3.org/ns/shacl#path> <http://www.w3.org/ns/shacl#equals> ;
                                                              rdfs:isDefinedBy <http://www.w3.org/ns/shacl#> .


###  http://www.w3.org/ns/shacl#ExpressionConstraintComponent
<http://www.w3.org/ns/shacl#ExpressionConstraintComponent> rdf:type <http://www.w3.org/ns/shacl#ConstraintComponent> ;
                                                           <http://www.w3.org/ns/shacl#parameter> <http://www.w3.org/ns/shacl#ExpressionConstraintComponent-expression> ;
                                                           rdfs:comment "A constraint component that can be used to verify that a given node expression produces true for all value nodes."@en ;
                                                           rdfs:isDefinedBy <http://www.w3.org/ns/shacl#> ;
                                                           rdfs:label "Expression constraint component"@en .


###  http://www.w3.org/ns/shacl#ExpressionConstraintComponent-expression
<http://www.w3.org/ns/shacl#ExpressionConstraintComponent-expression> rdf:type <http://www.w3.org/ns/shacl#Parameter> ;
                                                                      <http://www.w3.org/ns/shacl#path> <http://www.w3.org/ns/shacl#expression> ;
                                                                      rdfs:isDefinedBy <http://www.w3.org/ns/shacl#> .


###  http://www.w3.org/ns/shacl#Function
<http://www.w3.org/ns/shacl#Function> rdfs:comment "The class of SHACL functions."@en .


###  http://www.w3.org/ns/shacl#HasValueConstraintComponent
<http://www.w3.org/ns/shacl#HasValueConstraintComponent> rdf:type <http://www.w3.org/ns/shacl#ConstraintComponent> ;
                                                         <http://www.w3.org/ns/shacl#parameter> <http://www.w3.org/ns/shacl#HasValueConstraintComponent-hasValue> ;
                                                         rdfs:comment "A constraint component that can be used to verify that one of the value nodes is a given RDF node."@en ;
                                                         rdfs:isDefinedBy <http://www.w3.org/ns/shacl#> ;
                                                         rdfs:label "Has-value constraint component"@en .


###  http://www.w3.org/ns/shacl#HasValueConstraintComponent-hasValue
<http://www.w3.org/ns/shacl#HasValueConstraintComponent-hasValue> rdf:type <http://www.w3.org/ns/shacl#Parameter> ;
                                                                  <http://www.w3.org/ns/shacl#path> <http://www.w3.org/ns/shacl#hasValue> ;
                                                                  rdfs:isDefinedBy <http://www.w3.org/ns/shacl#> .


###  http://www.w3.org/ns/shacl#IRI
<http://www.w3.org/ns/shacl#IRI> rdf:type <http://www.w3.org/ns/shacl#NodeKind> ;
                                 rdfs:comment "The node kind of all IRIs."@en ;
                                 rdfs:isDefinedBy <http://www.w3.org/ns/shacl#> ;
                                 rdfs:label "IRI"@en .


###  http://www.w3.org/ns/shacl#IRIOrLiteral
<http://www.w3.org/ns/shacl#IRIOrLiteral> rdf:type <http://www.w3.org/ns/shacl#NodeKind> ;
                                          rdfs:comment "The node kind of all IRIs or literals."@en ;
                                          rdfs:isDefinedBy <http://www.w3.org/ns/shacl#> ;
                                          rdfs:label "IRI or literal"@en .


###  http://www.w3.org/ns/shacl#InConstraintComponent
<http://www.w3.org/ns/shacl#InConstraintComponent> rdf:type <http://www.w3.org/ns/shacl#ConstraintComponent> ;
                                                   <http://www.w3.org/ns/shacl#parameter> <http://www.w3.org/ns/shacl#InConstraintComponent-in> ;
                                                   rdfs:comment "A constraint component that can be used to exclusively enumerate the permitted value nodes."@en ;
                                                   rdfs:isDefinedBy <http://www.w3.org/ns/shacl#> ;
                                                   rdfs:label "In constraint component"@en .


###  http://www.w3.org/ns/shacl#InConstraintComponent-in
<http://www.w3.org/ns/shacl#InConstraintComponent-in> rdf:type <http://www.w3.org/ns/shacl#Parameter> ;
                                                      <http://www.w3.org/ns/shacl#path> <http://www.w3.org/ns/shacl#in> ;
                                                      <http://www.w3.org/ns/shacl#maxCount> 1 ;
                                                      rdfs:isDefinedBy <http://www.w3.org/ns/shacl#> .


###  http://www.w3.org/ns/shacl#Info
<http://www.w3.org/ns/shacl#Info> rdf:type <http://www.w3.org/ns/shacl#Severity> ;
                                  rdfs:comment "The severity for an informational validation result."@en ;
                                  rdfs:isDefinedBy <http://www.w3.org/ns/shacl#> ;
                                  rdfs:label "Info"@en .


###  http://www.w3.org/ns/shacl#JSConstraint
<http://www.w3.org/ns/shacl#JSConstraint> rdfs:comment "The class of constraints backed by a JavaScript function."@en .


###  http://www.w3.org/ns/shacl#JSConstraint-js
<http://www.w3.org/ns/shacl#JSConstraint-js> rdf:type <http://www.w3.org/ns/shacl#Parameter> ;
                                             <http://www.w3.org/ns/shacl#path> <http://www.w3.org/ns/shacl#js> ;
                                             rdfs:isDefinedBy <http://www.w3.org/ns/shacl#> .


###  http://www.w3.org/ns/shacl#JSConstraintComponent
<http://www.w3.org/ns/shacl#JSConstraintComponent> rdf:type <http://www.w3.org/ns/shacl#ConstraintComponent> ;
                                                   <http://www.w3.org/ns/shacl#parameter> <http://www.w3.org/ns/shacl#JSConstraint-js> ;
                                                   rdfs:comment "A constraint component with the parameter sh:js linking to a sh:JSConstraint containing a sh:script."@en ;
                                                   rdfs:isDefinedBy <http://www.w3.org/ns/shacl#> ;
                                                   rdfs:label "JavaScript constraint component"@en .


###  http://www.w3.org/ns/shacl#JSExecutable
<http://www.w3.org/ns/shacl#JSExecutable> rdfs:comment "Abstract base class of resources that declare an executable JavaScript."@en .


###  http://www.w3.org/ns/shacl#JSFunction
<http://www.w3.org/ns/shacl#JSFunction> rdfs:comment "The class of SHACL functions that execute a JavaScript function when called."@en .


###  http://www.w3.org/ns/shacl#JSLibrary
<http://www.w3.org/ns/shacl#JSLibrary> rdfs:comment "Represents a JavaScript library, typically identified by one or more URLs of files to include."@en .


###  http://www.w3.org/ns/shacl#JSRule
<http://www.w3.org/ns/shacl#JSRule> rdfs:comment "The class of SHACL rules expressed using JavaScript."@en .


###  http://www.w3.org/ns/shacl#JSTarget
<http://www.w3.org/ns/shacl#JSTarget> rdfs:comment "The class of targets that are based on JavaScript functions."@en .


###  http://www.w3.org/ns/shacl#JSTargetType
<http://www.w3.org/ns/shacl#JSTargetType> rdfs:comment "The (meta) class for parameterizable targets that are based on JavaScript functions."@en .


###  http://www.w3.org/ns/shacl#JSValidator
<http://www.w3.org/ns/shacl#JSValidator> rdfs:comment "A SHACL validator based on JavaScript. This can be used to declare SHACL constraint components that perform JavaScript-based validation when used."@en .


###  http://www.w3.org/ns/shacl#LanguageInConstraintComponent
<http://www.w3.org/ns/shacl#LanguageInConstraintComponent> rdf:type <http://www.w3.org/ns/shacl#ConstraintComponent> ;
                                                           <http://www.w3.org/ns/shacl#parameter> <http://www.w3.org/ns/shacl#LanguageInConstraintComponent-languageIn> ;
                                                           rdfs:comment "A constraint component that can be used to enumerate language tags that all value nodes must have."@en ;
                                                           rdfs:isDefinedBy <http://www.w3.org/ns/shacl#> ;
                                                           rdfs:label "Language-in constraint component"@en .


###  http://www.w3.org/ns/shacl#LanguageInConstraintComponent-languageIn
<http://www.w3.org/ns/shacl#LanguageInConstraintComponent-languageIn> rdf:type <http://www.w3.org/ns/shacl#Parameter> ;
                                                                      <http://www.w3.org/ns/shacl#path> <http://www.w3.org/ns/shacl#languageIn> ;
                                                                      <http://www.w3.org/ns/shacl#maxCount> 1 ;
                                                                      rdfs:isDefinedBy <http://www.w3.org/ns/shacl#> .


###  http://www.w3.org/ns/shacl#LessThanConstraintComponent
<http://www.w3.org/ns/shacl#LessThanConstraintComponent> rdf:type <http://www.w3.org/ns/shacl#ConstraintComponent> ;
                                                         <http://www.w3.org/ns/shacl#parameter> <http://www.w3.org/ns/shacl#LessThanConstraintComponent-lessThan> ;
                                                         rdfs:comment "A constraint component that can be used to verify that each value node is smaller than all the nodes that have the focus node as subject and the value of a given property as predicate."@en ;
                                                         rdfs:isDefinedBy <http://www.w3.org/ns/shacl#> ;
                                                         rdfs:label "Less-than constraint component"@en .


###  http://www.w3.org/ns/shacl#LessThanConstraintComponent-lessThan
<http://www.w3.org/ns/shacl#LessThanConstraintComponent-lessThan> rdf:type <http://www.w3.org/ns/shacl#Parameter> ;
                                                                  <http://www.w3.org/ns/shacl#nodeKind> <http://www.w3.org/ns/shacl#IRI> ;
                                                                  <http://www.w3.org/ns/shacl#path> <http://www.w3.org/ns/shacl#lessThan> ;
                                                                  rdfs:isDefinedBy <http://www.w3.org/ns/shacl#> .


###  http://www.w3.org/ns/shacl#LessThanOrEqualsConstraintComponent
<http://www.w3.org/ns/shacl#LessThanOrEqualsConstraintComponent> rdf:type <http://www.w3.org/ns/shacl#ConstraintComponent> ;
                                                                 <http://www.w3.org/ns/shacl#parameter> <http://www.w3.org/ns/shacl#LessThanOrEqualsConstraintComponent-lessThanOrEquals> ;
                                                                 rdfs:comment "A constraint component that can be used to verify that every value node is smaller than all the nodes that have the focus node as subject and the value of a given property as predicate."@en ;
                                                                 rdfs:isDefinedBy <http://www.w3.org/ns/shacl#> ;
                                                                 rdfs:label "less-than-or-equals constraint component"@en .


###  http://www.w3.org/ns/shacl#LessThanOrEqualsConstraintComponent-lessThanOrEquals
<http://www.w3.org/ns/shacl#LessThanOrEqualsConstraintComponent-lessThanOrEquals> rdf:type <http://www.w3.org/ns/shacl#Parameter> ;
                                                                                  <http://www.w3.org/ns/shacl#nodeKind> <http://www.w3.org/ns/shacl#IRI> ;
                                                                                  <http://www.w3.org/ns/shacl#path> <http://www.w3.org/ns/shacl#lessThanOrEquals> ;
                                                                                  rdfs:isDefinedBy <http://www.w3.org/ns/shacl#> .


###  http://www.w3.org/ns/shacl#Literal
<http://www.w3.org/ns/shacl#Literal> rdf:type <http://www.w3.org/ns/shacl#NodeKind> ;
                                     rdfs:comment "The node kind of all literals."@en ;
                                     rdfs:isDefinedBy <http://www.w3.org/ns/shacl#> ;
                                     rdfs:label "Literal"@en .


###  http://www.w3.org/ns/shacl#MaxCountConstraintComponent
<http://www.w3.org/ns/shacl#MaxCountConstraintComponent> rdf:type <http://www.w3.org/ns/shacl#ConstraintComponent> ;
                                                         <http://www.w3.org/ns/shacl#parameter> <http://www.w3.org/ns/shacl#MaxCountConstraintComponent-maxCount> ;
                                                         rdfs:comment "A constraint component that can be used to restrict the maximum number of value nodes."@en ;
                                                         rdfs:isDefinedBy <http://www.w3.org/ns/shacl#> ;
                                                         rdfs:label "Max-count constraint component"@en .


###  http://www.w3.org/ns/shacl#MaxCountConstraintComponent-maxCount
<http://www.w3.org/ns/shacl#MaxCountConstraintComponent-maxCount> rdf:type <http://www.w3.org/ns/shacl#Parameter> ;
                                                                  <http://www.w3.org/ns/shacl#datatype> xsd:integer ;
                                                                  <http://www.w3.org/ns/shacl#path> <http://www.w3.org/ns/shacl#maxCount> ;
                                                                  <http://www.w3.org/ns/shacl#maxCount> 1 ;
                                                                  rdfs:isDefinedBy <http://www.w3.org/ns/shacl#> .


###  http://www.w3.org/ns/shacl#MaxExclusiveConstraintComponent
<http://www.w3.org/ns/shacl#MaxExclusiveConstraintComponent> rdf:type <http://www.w3.org/ns/shacl#ConstraintComponent> ;
                                                             <http://www.w3.org/ns/shacl#parameter> <http://www.w3.org/ns/shacl#MaxExclusiveConstraintComponent-maxExclusive> ;
                                                             rdfs:comment "A constraint component that can be used to restrict the range of value nodes with a maximum exclusive value."@en ;
                                                             rdfs:isDefinedBy <http://www.w3.org/ns/shacl#> ;
                                                             rdfs:label "Max-exclusive constraint component"@en .


###  http://www.w3.org/ns/shacl#MaxExclusiveConstraintComponent-maxExclusive
<http://www.w3.org/ns/shacl#MaxExclusiveConstraintComponent-maxExclusive> rdf:type <http://www.w3.org/ns/shacl#Parameter> ;
                                                                          <http://www.w3.org/ns/shacl#nodeKind> <http://www.w3.org/ns/shacl#Literal> ;
                                                                          <http://www.w3.org/ns/shacl#path> <http://www.w3.org/ns/shacl#maxExclusive> ;
                                                                          <http://www.w3.org/ns/shacl#maxCount> 1 ;
                                                                          rdfs:isDefinedBy <http://www.w3.org/ns/shacl#> .


###  http://www.w3.org/ns/shacl#MaxInclusiveConstraintComponent
<http://www.w3.org/ns/shacl#MaxInclusiveConstraintComponent> rdf:type <http://www.w3.org/ns/shacl#ConstraintComponent> ;
                                                             <http://www.w3.org/ns/shacl#parameter> <http://www.w3.org/ns/shacl#MaxInclusiveConstraintComponent-maxInclusive> ;
                                                             rdfs:comment "A constraint component that can be used to restrict the range of value nodes with a maximum inclusive value."@en ;
                                                             rdfs:isDefinedBy <http://www.w3.org/ns/shacl#> ;
                                                             rdfs:label "Max-inclusive constraint component"@en .


###  http://www.w3.org/ns/shacl#MaxInclusiveConstraintComponent-maxInclusive
<http://www.w3.org/ns/shacl#MaxInclusiveConstraintComponent-maxInclusive> rdf:type <http://www.w3.org/ns/shacl#Parameter> ;
                                                                          <http://www.w3.org/ns/shacl#nodeKind> <http://www.w3.org/ns/shacl#Literal> ;
                                                                          <http://www.w3.org/ns/shacl#path> <http://www.w3.org/ns/shacl#maxInclusive> ;
                                                                          <http://www.w3.org/ns/shacl#maxCount> 1 ;
                                                                          rdfs:isDefinedBy <http://www.w3.org/ns/shacl#> .


###  http://www.w3.org/ns/shacl#MaxLengthConstraintComponent
<http://www.w3.org/ns/shacl#MaxLengthConstraintComponent> rdf:type <http://www.w3.org/ns/shacl#ConstraintComponent> ;
                                                          <http://www.w3.org/ns/shacl#parameter> <http://www.w3.org/ns/shacl#MaxLengthConstraintComponent-maxLength> ;
                                                          rdfs:comment "A constraint component that can be used to restrict the maximum string length of value nodes."@en ;
                                                          rdfs:isDefinedBy <http://www.w3.org/ns/shacl#> ;
                                                          rdfs:label "Max-length constraint component"@en .


###  http://www.w3.org/ns/shacl#MaxLengthConstraintComponent-maxLength
<http://www.w3.org/ns/shacl#MaxLengthConstraintComponent-maxLength> rdf:type <http://www.w3.org/ns/shacl#Parameter> ;
                                                                    <http://www.w3.org/ns/shacl#datatype> xsd:integer ;
                                                                    <http://www.w3.org/ns/shacl#path> <http://www.w3.org/ns/shacl#maxLength> ;
                                                                    <http://www.w3.org/ns/shacl#maxCount> 1 ;
                                                                    rdfs:isDefinedBy <http://www.w3.org/ns/shacl#> .


###  http://www.w3.org/ns/shacl#MinCountConstraintComponent
<http://www.w3.org/ns/shacl#MinCountConstraintComponent> rdf:type <http://www.w3.org/ns/shacl#ConstraintComponent> ;
                                                         <http://www.w3.org/ns/shacl#parameter> <http://www.w3.org/ns/shacl#MinCountConstraintComponent-minCount> ;
                                                         rdfs:comment "A constraint component that can be used to restrict the minimum number of value nodes."@en ;
                                                         rdfs:isDefinedBy <http://www.w3.org/ns/shacl#> ;
                                                         rdfs:label "Min-count constraint component"@en .


###  http://www.w3.org/ns/shacl#MinCountConstraintComponent-minCount
<http://www.w3.org/ns/shacl#MinCountConstraintComponent-minCount> rdf:type <http://www.w3.org/ns/shacl#Parameter> ;
                                                                  <http://www.w3.org/ns/shacl#datatype> xsd:integer ;
                                                                  <http://www.w3.org/ns/shacl#path> <http://www.w3.org/ns/shacl#minCount> ;
                                                                  <http://www.w3.org/ns/shacl#maxCount> 1 ;
                                                                  rdfs:isDefinedBy <http://www.w3.org/ns/shacl#> .


###  http://www.w3.org/ns/shacl#MinExclusiveConstraintComponent
<http://www.w3.org/ns/shacl#MinExclusiveConstraintComponent> rdf:type <http://www.w3.org/ns/shacl#ConstraintComponent> ;
                                                             <http://www.w3.org/ns/shacl#parameter> <http://www.w3.org/ns/shacl#MinExclusiveConstraintComponent-minExclusive> ;
                                                             rdfs:comment "A constraint component that can be used to restrict the range of value nodes with a minimum exclusive value."@en ;
                                                             rdfs:isDefinedBy <http://www.w3.org/ns/shacl#> ;
                                                             rdfs:label "Min-exclusive constraint component"@en .


###  http://www.w3.org/ns/shacl#MinExclusiveConstraintComponent-minExclusive
<http://www.w3.org/ns/shacl#MinExclusiveConstraintComponent-minExclusive> rdf:type <http://www.w3.org/ns/shacl#Parameter> ;
                                                                          <http://www.w3.org/ns/shacl#nodeKind> <http://www.w3.org/ns/shacl#Literal> ;
                                                                          <http://www.w3.org/ns/shacl#path> <http://www.w3.org/ns/shacl#minExclusive> ;
                                                                          <http://www.w3.org/ns/shacl#maxCount> 1 ;
                                                                          rdfs:isDefinedBy <http://www.w3.org/ns/shacl#> .


###  http://www.w3.org/ns/shacl#MinInclusiveConstraintComponent
<http://www.w3.org/ns/shacl#MinInclusiveConstraintComponent> rdf:type <http://www.w3.org/ns/shacl#ConstraintComponent> ;
                                                             <http://www.w3.org/ns/shacl#parameter> <http://www.w3.org/ns/shacl#MinInclusiveConstraintComponent-minInclusive> ;
                                                             rdfs:comment "A constraint component that can be used to restrict the range of value nodes with a minimum inclusive value."@en ;
                                                             rdfs:isDefinedBy <http://www.w3.org/ns/shacl#> ;
                                                             rdfs:label "Min-inclusive constraint component"@en .


###  http://www.w3.org/ns/shacl#MinInclusiveConstraintComponent-minInclusive
<http://www.w3.org/ns/shacl#MinInclusiveConstraintComponent-minInclusive> rdf:type <http://www.w3.org/ns/shacl#Parameter> ;
                                                                          <http://www.w3.org/ns/shacl#nodeKind> <http://www.w3.org/ns/shacl#Literal> ;
                                                                          <http://www.w3.org/ns/shacl#path> <http://www.w3.org/ns/shacl#minInclusive> ;
                                                                          <http://www.w3.org/ns/shacl#maxCount> 1 ;
                                                                          rdfs:isDefinedBy <http://www.w3.org/ns/shacl#> .


###  http://www.w3.org/ns/shacl#MinLengthConstraintComponent
<http://www.w3.org/ns/shacl#MinLengthConstraintComponent> rdf:type <http://www.w3.org/ns/shacl#ConstraintComponent> ;
                                                          <http://www.w3.org/ns/shacl#parameter> <http://www.w3.org/ns/shacl#MinLengthConstraintComponent-minLength> ;
                                                          rdfs:comment "A constraint component that can be used to restrict the minimum string length of value nodes."@en ;
                                                          rdfs:isDefinedBy <http://www.w3.org/ns/shacl#> ;
                                                          rdfs:label "Min-length constraint component"@en .


###  http://www.w3.org/ns/shacl#MinLengthConstraintComponent-minLength
<http://www.w3.org/ns/shacl#MinLengthConstraintComponent-minLength> rdf:type <http://www.w3.org/ns/shacl#Parameter> ;
                                                                    <http://www.w3.org/ns/shacl#datatype> xsd:integer ;
                                                                    <http://www.w3.org/ns/shacl#path> <http://www.w3.org/ns/shacl#minLength> ;
                                                                    <http://www.w3.org/ns/shacl#maxCount> 1 ;
                                                                    rdfs:isDefinedBy <http://www.w3.org/ns/shacl#> .


###  http://www.w3.org/ns/shacl#NodeConstraintComponent
<http://www.w3.org/ns/shacl#NodeConstraintComponent> rdf:type <http://www.w3.org/ns/shacl#ConstraintComponent> ;
                                                     <http://www.w3.org/ns/shacl#parameter> <http://www.w3.org/ns/shacl#NodeConstraintComponent-node> ;
                                                     rdfs:comment "A constraint component that can be used to verify that all value nodes conform to the given node shape."@en ;
                                                     rdfs:isDefinedBy <http://www.w3.org/ns/shacl#> ;
                                                     rdfs:label "Node constraint component"@en .


###  http://www.w3.org/ns/shacl#NodeConstraintComponent-node
<http://www.w3.org/ns/shacl#NodeConstraintComponent-node> rdf:type <http://www.w3.org/ns/shacl#Parameter> ;
                                                          <http://www.w3.org/ns/shacl#path> <http://www.w3.org/ns/shacl#node> ;
                                                          rdfs:isDefinedBy <http://www.w3.org/ns/shacl#> .


###  http://www.w3.org/ns/shacl#NodeKind
<http://www.w3.org/ns/shacl#NodeKind> rdfs:comment "The class of all node kinds, including sh:BlankNode, sh:IRI, sh:Literal or the combinations of these: sh:BlankNodeOrIRI, sh:BlankNodeOrLiteral, sh:IRIOrLiteral."@en .


###  http://www.w3.org/ns/shacl#NodeKindConstraintComponent
<http://www.w3.org/ns/shacl#NodeKindConstraintComponent> rdf:type <http://www.w3.org/ns/shacl#ConstraintComponent> ;
                                                         <http://www.w3.org/ns/shacl#parameter> <http://www.w3.org/ns/shacl#NodeKindConstraintComponent-nodeKind> ;
                                                         rdfs:comment "A constraint component that can be used to restrict the RDF node kind of each value node."@en ;
                                                         rdfs:isDefinedBy <http://www.w3.org/ns/shacl#> ;
                                                         rdfs:label "Node-kind constraint component"@en .


###  http://www.w3.org/ns/shacl#NodeKindConstraintComponent-nodeKind
<http://www.w3.org/ns/shacl#NodeKindConstraintComponent-nodeKind> rdf:type <http://www.w3.org/ns/shacl#Parameter> ;
                                                                  <http://www.w3.org/ns/shacl#in> [ ] ;
<http://www.w3.org/ns/shacl#path> <http://www.w3.org/ns/shacl#nodeKind> ;
<http://www.w3.org/ns/shacl#maxCount> 1 ;
rdfs:isDefinedBy <http://www.w3.org/ns/shacl#> .


###  http://www.w3.org/ns/shacl#NodeShape
<http://www.w3.org/ns/shacl#NodeShape> rdfs:comment "A node shape is a shape that specifies constraint that need to be met with respect to focus nodes."@en ;
                                       <http://www.w3.org/2004/02/skos/core#prefLabel> "Node Shape" .


###  http://www.w3.org/ns/shacl#NotConstraintComponent
<http://www.w3.org/ns/shacl#NotConstraintComponent> rdf:type <http://www.w3.org/ns/shacl#ConstraintComponent> ;
                                                    <http://www.w3.org/ns/shacl#parameter> <http://www.w3.org/ns/shacl#NotConstraintComponent-not> ;
                                                    rdfs:comment "A constraint component that can be used to verify that value nodes do not conform to a given shape."@en ;
                                                    rdfs:isDefinedBy <http://www.w3.org/ns/shacl#> ;
                                                    rdfs:label "Not constraint component"@en .


###  http://www.w3.org/ns/shacl#NotConstraintComponent-not
<http://www.w3.org/ns/shacl#NotConstraintComponent-not> rdf:type <http://www.w3.org/ns/shacl#Parameter> ;
                                                        <http://www.w3.org/ns/shacl#path> <http://www.w3.org/ns/shacl#not> ;
                                                        rdfs:isDefinedBy <http://www.w3.org/ns/shacl#> .


###  http://www.w3.org/ns/shacl#OrConstraintComponent
<http://www.w3.org/ns/shacl#OrConstraintComponent> rdf:type <http://www.w3.org/ns/shacl#ConstraintComponent> ;
                                                   <http://www.w3.org/ns/shacl#parameter> <http://www.w3.org/ns/shacl#OrConstraintComponent-or> ;
                                                   rdfs:comment "A constraint component that can be used to restrict the value nodes so that they conform to at least one out of several provided shapes."@en ;
                                                   rdfs:isDefinedBy <http://www.w3.org/ns/shacl#> ;
                                                   rdfs:label "Or constraint component"@en .


###  http://www.w3.org/ns/shacl#OrConstraintComponent-or
<http://www.w3.org/ns/shacl#OrConstraintComponent-or> rdf:type <http://www.w3.org/ns/shacl#Parameter> ;
                                                      <http://www.w3.org/ns/shacl#path> <http://www.w3.org/ns/shacl#or> ;
                                                      rdfs:isDefinedBy <http://www.w3.org/ns/shacl#> .


###  http://www.w3.org/ns/shacl#Parameter
<http://www.w3.org/ns/shacl#Parameter> rdfs:comment "The class of parameter declarations, consisting of a path predicate and (possibly) information about allowed value type, cardinality and other characteristics."@en .


###  http://www.w3.org/ns/shacl#Parameterizable
<http://www.w3.org/ns/shacl#Parameterizable> rdfs:comment "Superclass of components that can take parameters, especially functions and constraint components."@en .


###  http://www.w3.org/ns/shacl#PatternConstraintComponent
<http://www.w3.org/ns/shacl#PatternConstraintComponent> rdf:type <http://www.w3.org/ns/shacl#ConstraintComponent> ;
                                                        <http://www.w3.org/ns/shacl#parameter> <http://www.w3.org/ns/shacl#PatternConstraintComponent-flags> ,
                                                                                               <http://www.w3.org/ns/shacl#PatternConstraintComponent-pattern> ;
                                                        rdfs:comment "A constraint component that can be used to verify that every value node matches a given regular expression."@en ;
                                                        rdfs:isDefinedBy <http://www.w3.org/ns/shacl#> ;
                                                        rdfs:label "Pattern constraint component"@en .


###  http://www.w3.org/ns/shacl#PatternConstraintComponent-flags
<http://www.w3.org/ns/shacl#PatternConstraintComponent-flags> rdf:type <http://www.w3.org/ns/shacl#Parameter> ;
                                                              <http://www.w3.org/ns/shacl#datatype> xsd:string ;
                                                              <http://www.w3.org/ns/shacl#path> <http://www.w3.org/ns/shacl#flags> ;
                                                              <http://www.w3.org/ns/shacl#optional> "true"^^xsd:boolean ;
                                                              rdfs:isDefinedBy <http://www.w3.org/ns/shacl#> .


###  http://www.w3.org/ns/shacl#PatternConstraintComponent-pattern
<http://www.w3.org/ns/shacl#PatternConstraintComponent-pattern> rdf:type <http://www.w3.org/ns/shacl#Parameter> ;
                                                                <http://www.w3.org/ns/shacl#datatype> xsd:string ;
                                                                <http://www.w3.org/ns/shacl#path> <http://www.w3.org/ns/shacl#pattern> ;
                                                                rdfs:isDefinedBy <http://www.w3.org/ns/shacl#> .


###  http://www.w3.org/ns/shacl#PrefixDeclaration
<http://www.w3.org/ns/shacl#PrefixDeclaration> rdfs:comment "The class of prefix declarations, consisting of pairs of a prefix with a namespace."@en .


###  http://www.w3.org/ns/shacl#PropertyConstraintComponent
<http://www.w3.org/ns/shacl#PropertyConstraintComponent> rdf:type <http://www.w3.org/ns/shacl#ConstraintComponent> ;
                                                         <http://www.w3.org/ns/shacl#parameter> <http://www.w3.org/ns/shacl#PropertyConstraintComponent-property> ;
                                                         rdfs:comment "A constraint component that can be used to verify that all value nodes conform to the given property shape."@en ;
                                                         rdfs:isDefinedBy <http://www.w3.org/ns/shacl#> ;
                                                         rdfs:label "Property constraint component"@en .


###  http://www.w3.org/ns/shacl#PropertyConstraintComponent-property
<http://www.w3.org/ns/shacl#PropertyConstraintComponent-property> rdf:type <http://www.w3.org/ns/shacl#Parameter> ;
                                                                  <http://www.w3.org/ns/shacl#path> <http://www.w3.org/ns/shacl#property> ;
                                                                  rdfs:isDefinedBy <http://www.w3.org/ns/shacl#> .


###  http://www.w3.org/ns/shacl#PropertyGroup
<http://www.w3.org/ns/shacl#PropertyGroup> rdfs:comment "Instances of this class represent groups of property shapes that belong together."@en .


###  http://www.w3.org/ns/shacl#PropertyShape
<http://www.w3.org/ns/shacl#PropertyShape> rdfs:comment "A property shape is a shape that specifies constraints on the values of a focus node for a given property or path."@en .


###  http://www.w3.org/ns/shacl#QualifiedMaxCountConstraintComponent
<http://www.w3.org/ns/shacl#QualifiedMaxCountConstraintComponent> rdf:type <http://www.w3.org/ns/shacl#ConstraintComponent> ;
                                                                  <http://www.w3.org/ns/shacl#parameter> <http://www.w3.org/ns/shacl#QualifiedMaxCountConstraintComponent-qualifiedMaxCount> ,
                                                                                                         <http://www.w3.org/ns/shacl#QualifiedMaxCountConstraintComponent-qualifiedValueShape> ,
                                                                                                         <http://www.w3.org/ns/shacl#QualifiedMaxCountConstraintComponent-qualifiedValueShapesDisjoint> ;
                                                                  rdfs:comment "A constraint component that can be used to verify that a specified maximum number of value nodes conforms to a given shape."@en ;
                                                                  rdfs:isDefinedBy <http://www.w3.org/ns/shacl#> ;
                                                                  rdfs:label "Qualified-max-count constraint component"@en .


###  http://www.w3.org/ns/shacl#QualifiedMaxCountConstraintComponent-qualifiedMaxCount
<http://www.w3.org/ns/shacl#QualifiedMaxCountConstraintComponent-qualifiedMaxCount> rdf:type <http://www.w3.org/ns/shacl#Parameter> ;
                                                                                    <http://www.w3.org/ns/shacl#datatype> xsd:integer ;
                                                                                    <http://www.w3.org/ns/shacl#path> <http://www.w3.org/ns/shacl#qualifiedMaxCount> ;
                                                                                    rdfs:isDefinedBy <http://www.w3.org/ns/shacl#> .


###  http://www.w3.org/ns/shacl#QualifiedMaxCountConstraintComponent-qualifiedValueShape
<http://www.w3.org/ns/shacl#QualifiedMaxCountConstraintComponent-qualifiedValueShape> rdf:type <http://www.w3.org/ns/shacl#Parameter> ;
                                                                                      <http://www.w3.org/ns/shacl#path> <http://www.w3.org/ns/shacl#qualifiedValueShape> ;
                                                                                      rdfs:isDefinedBy <http://www.w3.org/ns/shacl#> .


###  http://www.w3.org/ns/shacl#QualifiedMaxCountConstraintComponent-qualifiedValueShapesDisjoint
<http://www.w3.org/ns/shacl#QualifiedMaxCountConstraintComponent-qualifiedValueShapesDisjoint> rdf:type <http://www.w3.org/ns/shacl#Parameter> ;
                                                                                               <http://www.w3.org/ns/shacl#datatype> xsd:boolean ;
                                                                                               <http://www.w3.org/ns/shacl#path> <http://www.w3.org/ns/shacl#qualifiedValueShapesDisjoint> ;
                                                                                               <http://www.w3.org/ns/shacl#optional> "true"^^xsd:boolean ;
                                                                                               rdfs:isDefinedBy <http://www.w3.org/ns/shacl#> .


###  http://www.w3.org/ns/shacl#QualifiedMinCountConstraintComponent
<http://www.w3.org/ns/shacl#QualifiedMinCountConstraintComponent> rdf:type <http://www.w3.org/ns/shacl#ConstraintComponent> ;
                                                                  <http://www.w3.org/ns/shacl#parameter> <http://www.w3.org/ns/shacl#QualifiedMinCountConstraintComponent-qualifiedMinCount> ,
                                                                                                         <http://www.w3.org/ns/shacl#QualifiedMinCountConstraintComponent-qualifiedValueShape> ,
                                                                                                         <http://www.w3.org/ns/shacl#QualifiedMinCountConstraintComponent-qualifiedValueShapesDisjoint> ;
                                                                  rdfs:comment "A constraint component that can be used to verify that a specified minimum number of value nodes conforms to a given shape."@en ;
                                                                  rdfs:isDefinedBy <http://www.w3.org/ns/shacl#> ;
                                                                  rdfs:label "Qualified-min-count constraint component"@en .


###  http://www.w3.org/ns/shacl#QualifiedMinCountConstraintComponent-qualifiedMinCount
<http://www.w3.org/ns/shacl#QualifiedMinCountConstraintComponent-qualifiedMinCount> rdf:type <http://www.w3.org/ns/shacl#Parameter> ;
                                                                                    <http://www.w3.org/ns/shacl#datatype> xsd:integer ;
                                                                                    <http://www.w3.org/ns/shacl#path> <http://www.w3.org/ns/shacl#qualifiedMinCount> ;
                                                                                    rdfs:isDefinedBy <http://www.w3.org/ns/shacl#> .


###  http://www.w3.org/ns/shacl#QualifiedMinCountConstraintComponent-qualifiedValueShape
<http://www.w3.org/ns/shacl#QualifiedMinCountConstraintComponent-qualifiedValueShape> rdf:type <http://www.w3.org/ns/shacl#Parameter> ;
                                                                                      <http://www.w3.org/ns/shacl#path> <http://www.w3.org/ns/shacl#qualifiedValueShape> ;
                                                                                      rdfs:isDefinedBy <http://www.w3.org/ns/shacl#> .


###  http://www.w3.org/ns/shacl#QualifiedMinCountConstraintComponent-qualifiedValueShapesDisjoint
<http://www.w3.org/ns/shacl#QualifiedMinCountConstraintComponent-qualifiedValueShapesDisjoint> rdf:type <http://www.w3.org/ns/shacl#Parameter> ;
                                                                                               <http://www.w3.org/ns/shacl#datatype> xsd:boolean ;
                                                                                               <http://www.w3.org/ns/shacl#path> <http://www.w3.org/ns/shacl#qualifiedValueShapesDisjoint> ;
                                                                                               <http://www.w3.org/ns/shacl#optional> "true"^^xsd:boolean ;
                                                                                               rdfs:isDefinedBy <http://www.w3.org/ns/shacl#> .


###  http://www.w3.org/ns/shacl#ResultAnnotation
<http://www.w3.org/ns/shacl#ResultAnnotation> rdfs:comment "A class of result annotations, which define the rules to derive the values of a given annotation property as extra values for a validation result."@en .


###  http://www.w3.org/ns/shacl#Rule
<http://www.w3.org/ns/shacl#Rule> rdfs:comment "The class of SHACL rules. Never instantiated directly."@en .


###  http://www.w3.org/ns/shacl#SPARQLAskExecutable
<http://www.w3.org/ns/shacl#SPARQLAskExecutable> rdfs:comment "The class of SPARQL executables that are based on an ASK query."@en .


###  http://www.w3.org/ns/shacl#SPARQLAskValidator
<http://www.w3.org/ns/shacl#SPARQLAskValidator> rdfs:comment "The class of validators based on SPARQL ASK queries. The queries are evaluated for each value node and are supposed to return true if the given node conforms."@en .


###  http://www.w3.org/ns/shacl#SPARQLConstraint
<http://www.w3.org/ns/shacl#SPARQLConstraint> rdfs:comment "The class of constraints based on SPARQL SELECT queries."@en .


###  http://www.w3.org/ns/shacl#SPARQLConstraintComponent
<http://www.w3.org/ns/shacl#SPARQLConstraintComponent> rdf:type <http://www.w3.org/ns/shacl#ConstraintComponent> ;
                                                       <http://www.w3.org/ns/shacl#parameter> <http://www.w3.org/ns/shacl#SPARQLConstraintComponent-sparql> ;
                                                       rdfs:comment "A constraint component that can be used to define constraints based on SPARQL queries."@en ;
                                                       rdfs:isDefinedBy <http://www.w3.org/ns/shacl#> ;
                                                       rdfs:label "SPARQL constraint component"@en .


###  http://www.w3.org/ns/shacl#SPARQLConstraintComponent-sparql
<http://www.w3.org/ns/shacl#SPARQLConstraintComponent-sparql> rdf:type <http://www.w3.org/ns/shacl#Parameter> ;
                                                              <http://www.w3.org/ns/shacl#path> <http://www.w3.org/ns/shacl#sparql> ;
                                                              rdfs:isDefinedBy <http://www.w3.org/ns/shacl#> .


###  http://www.w3.org/ns/shacl#SPARQLConstructExecutable
<http://www.w3.org/ns/shacl#SPARQLConstructExecutable> rdfs:comment "The class of SPARQL executables that are based on a CONSTRUCT query."@en .


###  http://www.w3.org/ns/shacl#SPARQLExecutable
<http://www.w3.org/ns/shacl#SPARQLExecutable> rdfs:comment "The class of resources that encapsulate a SPARQL query."@en .


###  http://www.w3.org/ns/shacl#SPARQLFunction
<http://www.w3.org/ns/shacl#SPARQLFunction> rdfs:comment "A function backed by a SPARQL query - either ASK or SELECT."@en .


###  http://www.w3.org/ns/shacl#SPARQLRule
<http://www.w3.org/ns/shacl#SPARQLRule> rdfs:comment "The class of SHACL rules based on SPARQL CONSTRUCT queries."@en .


###  http://www.w3.org/ns/shacl#SPARQLSelectExecutable
<http://www.w3.org/ns/shacl#SPARQLSelectExecutable> rdfs:comment "The class of SPARQL executables based on a SELECT query."@en .


###  http://www.w3.org/ns/shacl#SPARQLSelectValidator
<http://www.w3.org/ns/shacl#SPARQLSelectValidator> rdfs:comment "The class of validators based on SPARQL SELECT queries. The queries are evaluated for each focus node and are supposed to produce bindings for all focus nodes that do not conform."@en .


###  http://www.w3.org/ns/shacl#SPARQLTarget
<http://www.w3.org/ns/shacl#SPARQLTarget> rdfs:comment "The class of targets that are based on SPARQL queries."@en .


###  http://www.w3.org/ns/shacl#SPARQLTargetType
<http://www.w3.org/ns/shacl#SPARQLTargetType> rdfs:comment "The (meta) class for parameterizable targets that are based on SPARQL queries."@en .


###  http://www.w3.org/ns/shacl#SPARQLUpdateExecutable
<http://www.w3.org/ns/shacl#SPARQLUpdateExecutable> rdfs:comment "The class of SPARQL executables based on a SPARQL UPDATE."@en .


###  http://www.w3.org/ns/shacl#Severity
<http://www.w3.org/ns/shacl#Severity> rdfs:comment "The class of validation result severity levels, including violation and warning levels."@en .


###  http://www.w3.org/ns/shacl#Shape
<http://www.w3.org/ns/shacl#Shape> rdfs:comment "A shape is a collection of constraints that may be targeted for certain nodes."@en .


###  http://www.w3.org/ns/shacl#Target
<http://www.w3.org/ns/shacl#Target> rdfs:comment "The base class of targets such as those based on SPARQL queries."@en .


###  http://www.w3.org/ns/shacl#TargetType
<http://www.w3.org/ns/shacl#TargetType> rdfs:comment "The (meta) class for parameterizable targets.	Instances of this are instantiated as values of the sh:target property."@en .


###  http://www.w3.org/ns/shacl#UniqueLangConstraintComponent
<http://www.w3.org/ns/shacl#UniqueLangConstraintComponent> rdf:type <http://www.w3.org/ns/shacl#ConstraintComponent> ;
                                                           <http://www.w3.org/ns/shacl#parameter> <http://www.w3.org/ns/shacl#UniqueLangConstraintComponent-uniqueLang> ;
                                                           rdfs:comment "A constraint component that can be used to specify that no pair of value nodes may use the same language tag."@en ;
                                                           rdfs:isDefinedBy <http://www.w3.org/ns/shacl#> ;
                                                           rdfs:label "Unique-languages constraint component"@en .


###  http://www.w3.org/ns/shacl#UniqueLangConstraintComponent-uniqueLang
<http://www.w3.org/ns/shacl#UniqueLangConstraintComponent-uniqueLang> rdf:type <http://www.w3.org/ns/shacl#Parameter> ;
                                                                      <http://www.w3.org/ns/shacl#datatype> xsd:boolean ;
                                                                      <http://www.w3.org/ns/shacl#path> <http://www.w3.org/ns/shacl#uniqueLang> ;
                                                                      <http://www.w3.org/ns/shacl#maxCount> 1 ;
                                                                      rdfs:isDefinedBy <http://www.w3.org/ns/shacl#> .


###  http://www.w3.org/ns/shacl#ValidationReport
<http://www.w3.org/ns/shacl#ValidationReport> rdfs:comment "The class of SHACL validation reports."@en ;
                                              <http://www.w3.org/2004/02/skos/core#prefLabel> "Validation Report" .


###  http://www.w3.org/ns/shacl#ValidationResult
<http://www.w3.org/ns/shacl#ValidationResult> rdfs:comment "The class of validation results."@en .


###  http://www.w3.org/ns/shacl#Validator
<http://www.w3.org/ns/shacl#Validator> rdfs:comment "The class of validators, which provide instructions on how to process a constraint definition. This class serves as base class for the SPARQL-based validators and other possible implementations."@en .


###  http://www.w3.org/ns/shacl#Violation
<http://www.w3.org/ns/shacl#Violation> rdf:type <http://www.w3.org/ns/shacl#Severity> ;
                                       rdfs:comment "The severity for a violation validation result."@en ;
                                       rdfs:isDefinedBy <http://www.w3.org/ns/shacl#> ;
                                       rdfs:label "Violation"@en .


###  http://www.w3.org/ns/shacl#Warning
<http://www.w3.org/ns/shacl#Warning> rdf:type <http://www.w3.org/ns/shacl#Severity> ;
                                     rdfs:comment "The severity for a warning validation result."@en ;
                                     rdfs:isDefinedBy <http://www.w3.org/ns/shacl#> ;
                                     rdfs:label "Warning"@en .


###  http://www.w3.org/ns/shacl#XoneConstraintComponent
<http://www.w3.org/ns/shacl#XoneConstraintComponent> rdf:type <http://www.w3.org/ns/shacl#ConstraintComponent> ;
                                                     <http://www.w3.org/ns/shacl#parameter> <http://www.w3.org/ns/shacl#XoneConstraintComponent-xone> ;
                                                     rdfs:comment "A constraint component that can be used to restrict the value nodes so that they conform to exactly one out of several provided shapes."@en ;
                                                     rdfs:isDefinedBy <http://www.w3.org/ns/shacl#> ;
                                                     rdfs:label "Exactly one constraint component"@en .


###  http://www.w3.org/ns/shacl#XoneConstraintComponent-xone
<http://www.w3.org/ns/shacl#XoneConstraintComponent-xone> rdf:type <http://www.w3.org/ns/shacl#Parameter> ;
                                                          <http://www.w3.org/ns/shacl#path> <http://www.w3.org/ns/shacl#xone> ;
                                                          rdfs:isDefinedBy <http://www.w3.org/ns/shacl#> .


###  http://www.w3.org/ns/shacl#alternativePath
<http://www.w3.org/ns/shacl#alternativePath> rdfs:comment "The (single) value of this property must be a list of path elements, representing the elements of alternative paths."@en .


###  http://www.w3.org/ns/shacl#and
<http://www.w3.org/ns/shacl#and> rdfs:comment "RDF list of shapes to validate the value nodes against."@en .


###  http://www.w3.org/ns/shacl#annotationProperty
<http://www.w3.org/ns/shacl#annotationProperty> rdfs:comment "The annotation property that shall be set."@en .


###  http://www.w3.org/ns/shacl#annotationValue
<http://www.w3.org/ns/shacl#annotationValue> rdfs:comment "The (default) values of the annotation property."@en .


###  http://www.w3.org/ns/shacl#annotationVarName
<http://www.w3.org/ns/shacl#annotationVarName> rdfs:comment "The name of the SPARQL variable from the SELECT clause that shall be used for the values."@en .


###  http://www.w3.org/ns/shacl#ask
<http://www.w3.org/ns/shacl#ask> rdfs:comment "The SPARQL ASK query to execute."@en .


###  http://www.w3.org/ns/shacl#class
<http://www.w3.org/ns/shacl#class> rdfs:comment "The type that all value nodes must have."@en .


###  http://www.w3.org/ns/shacl#closed
<http://www.w3.org/ns/shacl#closed> rdfs:comment "If set to true then the shape is closed."@en .


###  http://www.w3.org/ns/shacl#condition
<http://www.w3.org/ns/shacl#condition> rdfs:comment "The shapes that the focus nodes need to conform to before a rule is executed on them."@en .


###  http://www.w3.org/ns/shacl#conforms
<http://www.w3.org/ns/shacl#conforms> rdfs:comment "True if the validation did not produce any validation results, and false otherwise."@en .


###  http://www.w3.org/ns/shacl#construct
<http://www.w3.org/ns/shacl#construct> rdfs:comment "The SPARQL CONSTRUCT query to execute."@en .


###  http://www.w3.org/ns/shacl#datatype
<http://www.w3.org/ns/shacl#datatype> rdfs:comment "Specifies an RDF datatype that all value nodes must have."@en .


###  http://www.w3.org/ns/shacl#deactivated
<http://www.w3.org/ns/shacl#deactivated> rdfs:comment "If set to true then all nodes conform to this."@en .


###  http://www.w3.org/ns/shacl#declare
<http://www.w3.org/ns/shacl#declare> rdfs:comment "Links a resource with its namespace prefix declarations."@en .


###  http://www.w3.org/ns/shacl#defaultValue
<http://www.w3.org/ns/shacl#defaultValue> rdfs:comment "A default value for a property, for example for user interface tools to pre-populate input fields."@en .


###  http://www.w3.org/ns/shacl#description
<http://www.w3.org/ns/shacl#description> rdfs:comment "Human-readable descriptions for the property in the context of the surrounding shape."@en .


###  http://www.w3.org/ns/shacl#detail
<http://www.w3.org/ns/shacl#detail> rdfs:comment "Links a result with other results that provide more details, for example to describe violations against nested shapes."@en .


###  http://www.w3.org/ns/shacl#disjoint
<http://www.w3.org/ns/shacl#disjoint> rdfs:comment "Specifies a property where the set of values must be disjoint with the value nodes."@en .


###  http://www.w3.org/ns/shacl#entailment
<http://www.w3.org/ns/shacl#entailment> rdfs:comment "An entailment regime that indicates what kind of inferencing is required by a shapes graph."@en .


###  http://www.w3.org/ns/shacl#equals
<http://www.w3.org/ns/shacl#equals> rdfs:comment "Specifies a property that must have the same values as the value nodes."@en .


###  http://www.w3.org/ns/shacl#expression
<http://www.w3.org/ns/shacl#expression> rdfs:comment "The node expression that must return true for the value nodes."@en ;
                                        rdfs:isDefinedBy <http://www.w3.org/ns/shacl#> ;
                                        rdfs:label "expression"@en .


###  http://www.w3.org/ns/shacl#filterShape
<http://www.w3.org/ns/shacl#filterShape> rdfs:comment "The shape that all input nodes of the expression need to conform to."@en .


###  http://www.w3.org/ns/shacl#flags
<http://www.w3.org/ns/shacl#flags> rdfs:comment "An optional flag to be used with regular expression pattern matching."@en .


###  http://www.w3.org/ns/shacl#focusNode
<http://www.w3.org/ns/shacl#focusNode> rdfs:comment "The focus node that was validated when the result was produced."@en .


###  http://www.w3.org/ns/shacl#group
<http://www.w3.org/ns/shacl#group> rdfs:comment "Can be used to link to a property group to indicate that a property shape belongs to a group of related property shapes."@en .


###  http://www.w3.org/ns/shacl#hasValue
<http://www.w3.org/ns/shacl#hasValue> rdfs:comment "Specifies a value that must be among the value nodes."@en ;
                                      rdfs:isDefinedBy <http://www.w3.org/ns/shacl#> ;
                                      rdfs:label "has value"@en .


###  http://www.w3.org/ns/shacl#ignoredProperties
<http://www.w3.org/ns/shacl#ignoredProperties> rdfs:comment "An optional RDF list of properties that are also permitted in addition to those explicitly enumerated via sh:property/sh:path."@en .


###  http://www.w3.org/ns/shacl#in
<http://www.w3.org/ns/shacl#in> rdfs:comment "Specifies a list of allowed values so that each value node must be among the members of the given list."@en .


###  http://www.w3.org/ns/shacl#intersection
<http://www.w3.org/ns/shacl#intersection> rdfs:comment "A list of node expressions that shall be intersected."@en ;
                                          rdfs:isDefinedBy <http://www.w3.org/ns/shacl#> ;
                                          rdfs:label "intersection"@en .


###  http://www.w3.org/ns/shacl#inversePath
<http://www.w3.org/ns/shacl#inversePath> rdfs:comment "The (single) value of this property represents an inverse path (object to subject)."@en .


###  http://www.w3.org/ns/shacl#js
<http://www.w3.org/ns/shacl#js> rdfs:comment "Constraints expressed in JavaScript." .


###  http://www.w3.org/ns/shacl#jsFunctionName
<http://www.w3.org/ns/shacl#jsFunctionName> rdfs:comment "The name of the JavaScript function to execute."@en .


###  http://www.w3.org/ns/shacl#jsLibrary
<http://www.w3.org/ns/shacl#jsLibrary> rdfs:comment "Declares which JavaScript libraries are needed to execute this."@en .


###  http://www.w3.org/ns/shacl#jsLibraryURL
<http://www.w3.org/ns/shacl#jsLibraryURL> rdfs:comment "Declares the URLs of a JavaScript library. This should be the absolute URL of a JavaScript file. Implementations may redirect those to local files."@en .


###  http://www.w3.org/ns/shacl#labelTemplate
<http://www.w3.org/ns/shacl#labelTemplate> rdfs:comment "Outlines how human-readable labels of instances of the associated Parameterizable shall be produced. The values can contain {?paramName} as placeholders for the actual values of the given parameter."@en .


###  http://www.w3.org/ns/shacl#languageIn
<http://www.w3.org/ns/shacl#languageIn> rdfs:comment "Specifies a list of language tags that all value nodes must have."@en .


###  http://www.w3.org/ns/shacl#lessThan
<http://www.w3.org/ns/shacl#lessThan> rdfs:comment "Specifies a property that must have smaller values than the value nodes."@en .


###  http://www.w3.org/ns/shacl#lessThanOrEquals
<http://www.w3.org/ns/shacl#lessThanOrEquals> rdfs:comment "Specifies a property that must have smaller or equal values than the value nodes."@en .


###  http://www.w3.org/ns/shacl#maxCount
<http://www.w3.org/ns/shacl#maxCount> rdfs:comment "Specifies the maximum number of values in the set of value nodes."@en .


###  http://www.w3.org/ns/shacl#maxExclusive
<http://www.w3.org/ns/shacl#maxExclusive> rdfs:comment "Specifies the maximum exclusive value of each value node."@en ;
                                          rdfs:isDefinedBy <http://www.w3.org/ns/shacl#> ;
                                          rdfs:label "max exclusive"@en .


###  http://www.w3.org/ns/shacl#maxInclusive
<http://www.w3.org/ns/shacl#maxInclusive> rdfs:comment "Specifies the maximum inclusive value of each value node."@en ;
                                          rdfs:isDefinedBy <http://www.w3.org/ns/shacl#> ;
                                          rdfs:label "max inclusive"@en .


###  http://www.w3.org/ns/shacl#maxLength
<http://www.w3.org/ns/shacl#maxLength> rdfs:comment "Specifies the maximum string length of each value node."@en .


###  http://www.w3.org/ns/shacl#message
<http://www.w3.org/ns/shacl#message> rdfs:comment "A human-readable message (possibly with placeholders for variables) explaining the cause of the result."@en ;
                                     rdfs:isDefinedBy <http://www.w3.org/ns/shacl#> ;
                                     rdfs:label "message"@en .


###  http://www.w3.org/ns/shacl#minCount
<http://www.w3.org/ns/shacl#minCount> rdfs:comment "Specifies the minimum number of values in the set of value nodes."@en .


###  http://www.w3.org/ns/shacl#minExclusive
<http://www.w3.org/ns/shacl#minExclusive> rdfs:comment "Specifies the minimum exclusive value of each value node."@en ;
                                          rdfs:isDefinedBy <http://www.w3.org/ns/shacl#> ;
                                          rdfs:label "min exclusive"@en .


###  http://www.w3.org/ns/shacl#minInclusive
<http://www.w3.org/ns/shacl#minInclusive> rdfs:comment "Specifies the minimum inclusive value of each value node."@en ;
                                          rdfs:isDefinedBy <http://www.w3.org/ns/shacl#> ;
                                          rdfs:label "min inclusive"@en .


###  http://www.w3.org/ns/shacl#minLength
<http://www.w3.org/ns/shacl#minLength> rdfs:comment "Specifies the minimum string length of each value node."@en .


###  http://www.w3.org/ns/shacl#name
<http://www.w3.org/ns/shacl#name> rdfs:comment "Human-readable labels for the property in the context of the surrounding shape."@en .


###  http://www.w3.org/ns/shacl#namespace
<http://www.w3.org/ns/shacl#namespace> rdfs:comment "The namespace associated with a prefix in a prefix declaration."@en .


###  http://www.w3.org/ns/shacl#node
<http://www.w3.org/ns/shacl#node> rdfs:comment "Specifies the node shape that all value nodes must conform to."@en .


###  http://www.w3.org/ns/shacl#nodeKind
<http://www.w3.org/ns/shacl#nodeKind> rdfs:comment "Specifies the node kind (e.g. IRI or literal) each value node."@en .


###  http://www.w3.org/ns/shacl#nodeValidator
<http://www.w3.org/ns/shacl#nodeValidator> rdfs:comment "The validator(s) used to evaluate a constraint in the context of a node shape."@en .


###  http://www.w3.org/ns/shacl#nodes
<http://www.w3.org/ns/shacl#nodes> rdfs:comment "The node expression producing the input nodes of a filter shape expression."@en ;
                                   rdfs:isDefinedBy <http://www.w3.org/ns/shacl#> ;
                                   rdfs:label "nodes"@en .


###  http://www.w3.org/ns/shacl#not
<http://www.w3.org/ns/shacl#not> rdfs:comment "Specifies a shape that the value nodes must not conform to."@en .


###  http://www.w3.org/ns/shacl#object
<http://www.w3.org/ns/shacl#object> rdfs:comment "An expression producing the nodes that shall be inferred as objects."@en .


###  http://www.w3.org/ns/shacl#oneOrMorePath
<http://www.w3.org/ns/shacl#oneOrMorePath> rdfs:comment "The (single) value of this property represents a path that is matched one or more times."@en .


###  http://www.w3.org/ns/shacl#optional
<http://www.w3.org/ns/shacl#optional> rdfs:comment "Indicates whether a parameter is optional."@en .


###  http://www.w3.org/ns/shacl#or
<http://www.w3.org/ns/shacl#or> rdfs:comment "Specifies a list of shapes so that the value nodes must conform to at least one of the shapes."@en .


###  http://www.w3.org/ns/shacl#order
<http://www.w3.org/ns/shacl#order> rdfs:comment "Specifies the relative order of this compared to its siblings. For example use 0 for the first, 1 for the second."@en ;
                                   rdfs:isDefinedBy <http://www.w3.org/ns/shacl#> ;
                                   rdfs:label "order"@en .


###  http://www.w3.org/ns/shacl#parameter
<http://www.w3.org/ns/shacl#parameter> rdfs:comment "The parameters of a function or constraint component."@en .


###  http://www.w3.org/ns/shacl#path
<http://www.w3.org/ns/shacl#path> rdfs:comment "Specifies the property path of a property shape."@en .


###  http://www.w3.org/ns/shacl#pattern
<http://www.w3.org/ns/shacl#pattern> rdfs:comment "Specifies a regular expression pattern that the string representations of the value nodes must match."@en .


###  http://www.w3.org/ns/shacl#predicate
<http://www.w3.org/ns/shacl#predicate> rdfs:comment "An expression producing the properties that shall be inferred as predicates."@en .


###  http://www.w3.org/ns/shacl#prefix
<http://www.w3.org/ns/shacl#prefix> rdfs:comment "The prefix of a prefix declaration."@en .


###  http://www.w3.org/ns/shacl#prefixes
<http://www.w3.org/ns/shacl#prefixes> rdfs:comment "The prefixes that shall be applied before parsing the associated SPARQL query."@en .


###  http://www.w3.org/ns/shacl#property
<http://www.w3.org/ns/shacl#property> rdfs:comment "Links a shape to its property shapes."@en .


###  http://www.w3.org/ns/shacl#propertyValidator
<http://www.w3.org/ns/shacl#propertyValidator> rdfs:comment "The validator(s) used to evaluate a constraint in the context of a property shape."@en .


###  http://www.w3.org/ns/shacl#qualifiedMaxCount
<http://www.w3.org/ns/shacl#qualifiedMaxCount> rdfs:comment "The maximum number of value nodes that can conform to the shape."@en .


###  http://www.w3.org/ns/shacl#qualifiedMinCount
<http://www.w3.org/ns/shacl#qualifiedMinCount> rdfs:comment "The minimum number of value nodes that must conform to the shape."@en .


###  http://www.w3.org/ns/shacl#qualifiedValueShape
<http://www.w3.org/ns/shacl#qualifiedValueShape> rdfs:comment "The shape that a specified number of values must conform to."@en .


###  http://www.w3.org/ns/shacl#qualifiedValueShapesDisjoint
<http://www.w3.org/ns/shacl#qualifiedValueShapesDisjoint> rdfs:comment "Can be used to mark the qualified value shape to be disjoint with its sibling shapes."@en .


###  http://www.w3.org/ns/shacl#result
<http://www.w3.org/ns/shacl#result> rdfs:comment "The validation results contained in a validation report."@en .


###  http://www.w3.org/ns/shacl#resultAnnotation
<http://www.w3.org/ns/shacl#resultAnnotation> rdfs:comment "Links a SPARQL validator with zero or more sh:ResultAnnotation instances, defining how to derive additional result properties based on the variables of the SELECT query."@en .


###  http://www.w3.org/ns/shacl#resultMessage
<http://www.w3.org/ns/shacl#resultMessage> rdfs:comment "Human-readable messages explaining the cause of the result."@en .


###  http://www.w3.org/ns/shacl#resultPath
<http://www.w3.org/ns/shacl#resultPath> rdfs:comment "The path of a validation result, based on the path of the validated property shape."@en .


###  http://www.w3.org/ns/shacl#resultSeverity
<http://www.w3.org/ns/shacl#resultSeverity> rdfs:comment "The severity of the result, e.g. warning."@en .


###  http://www.w3.org/ns/shacl#returnType
<http://www.w3.org/ns/shacl#returnType> rdfs:comment "The expected type of values returned by the associated function."@en .


###  http://www.w3.org/ns/shacl#rule
<http://www.w3.org/ns/shacl#rule> rdfs:comment "The rules linked to a shape."@en .


###  http://www.w3.org/ns/shacl#select
<http://www.w3.org/ns/shacl#select> rdfs:comment "The SPARQL SELECT query to execute."@en .


###  http://www.w3.org/ns/shacl#severity
<http://www.w3.org/ns/shacl#severity> rdfs:comment "Defines the severity that validation results produced by a shape must have. Defaults to sh:Violation."@en .


###  http://www.w3.org/ns/shacl#shapesGraph
<http://www.w3.org/ns/shacl#shapesGraph> rdfs:comment "Shapes graphs that should be used when validating this data graph."@en .


###  http://www.w3.org/ns/shacl#shapesGraphWellFormed
<http://www.w3.org/ns/shacl#shapesGraphWellFormed> rdfs:comment "If true then the validation engine was certain that the shapes graph has passed all SHACL syntax requirements during the validation process."@en .


###  http://www.w3.org/ns/shacl#sourceConstraint
<http://www.w3.org/ns/shacl#sourceConstraint> rdfs:comment "The constraint that was validated when the result was produced."@en .


###  http://www.w3.org/ns/shacl#sourceConstraintComponent
<http://www.w3.org/ns/shacl#sourceConstraintComponent> rdfs:comment "The constraint component that is the source of the result."@en .


###  http://www.w3.org/ns/shacl#sourceShape
<http://www.w3.org/ns/shacl#sourceShape> rdfs:comment "The shape that is was validated when the result was produced."@en .


###  http://www.w3.org/ns/shacl#sparql
<http://www.w3.org/ns/shacl#sparql> rdfs:comment "Links a shape with SPARQL constraints."@en .


###  http://www.w3.org/ns/shacl#subject
<http://www.w3.org/ns/shacl#subject> rdfs:comment "An expression producing the resources that shall be inferred as subjects."@en .


###  http://www.w3.org/ns/shacl#suggestedShapesGraph
<http://www.w3.org/ns/shacl#suggestedShapesGraph> rdfs:comment "Suggested shapes graphs for this ontology. The values of this property may be used in the absence of specific sh:shapesGraph statements."@en .


###  http://www.w3.org/ns/shacl#target
<http://www.w3.org/ns/shacl#target> rdfs:comment "Links a shape to a target specified by an extension language, for example instances of sh:SPARQLTarget."@en .


###  http://www.w3.org/ns/shacl#targetClass
<http://www.w3.org/ns/shacl#targetClass> rdfs:comment "Links a shape to a class, indicating that all instances of the class must conform to the shape."@en .


###  http://www.w3.org/ns/shacl#targetNode
<http://www.w3.org/ns/shacl#targetNode> rdfs:comment "Links a shape to individual nodes, indicating that these nodes must conform to the shape."@en .


###  http://www.w3.org/ns/shacl#targetObjectsOf
<http://www.w3.org/ns/shacl#targetObjectsOf> rdfs:comment "Links a shape to a property, indicating that all all objects of triples that have the given property as their predicate must conform to the shape."@en .


###  http://www.w3.org/ns/shacl#targetSubjectsOf
<http://www.w3.org/ns/shacl#targetSubjectsOf> rdfs:comment "Links a shape to a property, indicating that all subjects of triples that have the given property as their predicate must conform to the shape."@en .


###  http://www.w3.org/ns/shacl#this
<http://www.w3.org/ns/shacl#this> rdf:type rdfs:Resource ;
                                  rdfs:comment "A node expression that represents the current focus node."@en ;
                                  rdfs:isDefinedBy <http://www.w3.org/ns/shacl#> ;
                                  rdfs:label "this"@en .


###  http://www.w3.org/ns/shacl#union
<http://www.w3.org/ns/shacl#union> rdfs:comment "A list of node expressions that shall be used together."@en ;
                                   rdfs:isDefinedBy <http://www.w3.org/ns/shacl#> ;
                                   rdfs:label "union"@en .


###  http://www.w3.org/ns/shacl#uniqueLang
<http://www.w3.org/ns/shacl#uniqueLang> rdfs:comment "Specifies whether all node values must have a unique (or no) language tag."@en .


###  http://www.w3.org/ns/shacl#update
<http://www.w3.org/ns/shacl#update> rdfs:comment "The SPARQL UPDATE to execute."@en .


###  http://www.w3.org/ns/shacl#validator
<http://www.w3.org/ns/shacl#validator> rdfs:comment "The validator(s) used to evaluate constraints of either node or property shapes."@en .


###  http://www.w3.org/ns/shacl#value
<http://www.w3.org/ns/shacl#value> rdfs:comment "An RDF node that has caused the result."@en .


###  http://www.w3.org/ns/shacl#xone
<http://www.w3.org/ns/shacl#xone> rdfs:comment "Specifies a list of shapes so that the value nodes must conform to exactly one of the shapes."@en .


###  http://www.w3.org/ns/shacl#zeroOrMorePath
<http://www.w3.org/ns/shacl#zeroOrMorePath> rdfs:comment "The (single) value of this property represents a path that is matched zero or more times."@en .


###  http://www.w3.org/ns/shacl#zeroOrOnePath
<http://www.w3.org/ns/shacl#zeroOrOnePath> rdfs:comment "The (single) value of this property represents a path that is matched zero or one times."@en .


###  https://data.digichecks.eu/def/Allocation
:Allocation rdf:type owl:NamedIndividual ;
            <http://www.w3.org/2004/02/skos/core#prefLabel> "Allocation" .


###  https://data.digichecks.eu/def/Decision
:Decision rdf:type owl:NamedIndividual ;
          <http://www.w3.org/2004/02/skos/core#prefLabel> "Decision" .


###  https://data.digichecks.eu/def/Document
:Document rdf:type owl:NamedIndividual ;
          <http://www.w3.org/2004/02/skos/core#prefLabel> "Document" .


###  https://data.digichecks.eu/def/GenericRequirement
:GenericRequirement rdf:type owl:NamedIndividual ;
                    <http://www.w3.org/2004/02/skos/core#prefLabel> "Generic Requirement" .


###  https://data.digichecks.eu/def/MachineReadableRule
:MachineReadableRule rdf:type owl:NamedIndividual ;
                     <http://www.w3.org/2004/02/skos/core#prefLabel> "Machine readable rule" .


###  https://data.digichecks.eu/def/Parcel
:Parcel rdf:type owl:NamedIndividual ;
        <http://www.w3.org/2004/02/skos/core#prefLabel> "Parcel" .


###  https://data.digichecks.eu/def/Permit
:Permit rdf:type owl:NamedIndividual ;
        <http://www.w3.org/2004/02/skos/core#prefLabel> "Permit" .


###  https://data.digichecks.eu/def/PermitRequest
:PermitRequest rdf:type owl:NamedIndividual ;
               <http://www.w3.org/2004/02/skos/core#prefLabel> "Permit request" .


###  https://data.digichecks.eu/def/Project
:Project rdf:type owl:NamedIndividual ;
         <http://www.w3.org/2004/02/skos/core#prefLabel> "Project" .


###  https://data.digichecks.eu/def/ProjectRequirement
:ProjectRequirement rdf:type owl:NamedIndividual ;
                    <http://www.w3.org/2004/02/skos/core#prefLabel> "Project Requirement" .


###  https://data.digichecks.eu/def/Verification
:Verification rdf:type owl:NamedIndividual ;
              <http://www.w3.org/2004/02/skos/core#prefLabel> "Verification" .


###  https://data.digichecks.eu/def/VerificationMethod
:VerificationMethod rdf:type owl:NamedIndividual ;
                    <http://www.w3.org/2004/02/skos/core#prefLabel> "Verification method" .


###  https://data.digichecks.eu/def/decisionOutcome
:decisionOutcome rdf:type owl:NamedIndividual ;
                 <http://www.w3.org/2004/02/skos/core#prefLabel> "decision outcome" .


###  https://data.digichecks.eu/def/hasAsOutput
:hasAsOutput rdf:type owl:NamedIndividual ;
             <http://www.w3.org/2004/02/skos/core#prefLabel> "has as output" .


###  https://data.digichecks.eu/def/hasParcel
:hasParcel rdf:type owl:NamedIndividual ;
           <http://www.w3.org/2004/02/skos/core#prefLabel> "has parcel" .


###  https://data.digichecks.eu/def/hasPermitRequest
:hasPermitRequest rdf:type owl:NamedIndividual ;
                  <http://www.w3.org/2004/02/skos/core#prefLabel> "has permit request" .


###  https://data.digichecks.eu/def/hasSource
:hasSource rdf:type owl:NamedIndividual ;
           <http://www.w3.org/2004/02/skos/core#prefLabel> "has source" .


###  https://data.digichecks.eu/def/hasVerificationMethod
:hasVerificationMethod rdf:type owl:NamedIndividual ;
                       <http://www.w3.org/2004/02/skos/core#prefLabel> "has verification method" .


###  https://data.digichecks.eu/def/isAddressFor
:isAddressFor rdf:type owl:NamedIndividual ;
              <http://www.w3.org/2004/02/skos/core#prefLabel> "is address for" .


###  https://data.digichecks.eu/def/isAllocationfor
:isAllocationfor rdf:type owl:NamedIndividual ;
                 <http://www.w3.org/2004/02/skos/core#prefLabel> "is allocation for" .


###  https://data.digichecks.eu/def/isCollectedIn
:isCollectedIn rdf:type owl:NamedIndividual ;
               <http://www.w3.org/2004/02/skos/core#prefLabel> "is collected in" .


###  https://data.digichecks.eu/def/isControlledBy
:isControlledBy rdf:type owl:NamedIndividual ;
                <http://www.w3.org/2004/02/skos/core#prefLabel> "is controlled by" .


###  https://data.digichecks.eu/def/isDecisionFor
:isDecisionFor rdf:type owl:NamedIndividual ;
               <http://www.w3.org/2004/02/skos/core#prefLabel> "is decision for" .


###  https://data.digichecks.eu/def/isDerivedIn
:isDerivedIn rdf:type owl:NamedIndividual ;
             <http://www.w3.org/2004/02/skos/core#prefLabel> "is derived in" .


###  https://data.digichecks.eu/def/isExpressedAs
:isExpressedAs rdf:type owl:NamedIndividual ;
               <http://www.w3.org/2004/02/skos/core#prefLabel> "is expressed as" .


###  https://data.digichecks.eu/def/isGeometryOf
:isGeometryOf rdf:type owl:NamedIndividual ;
              <http://www.w3.org/2004/02/skos/core#prefLabel> "is geometry of" .


###  https://data.digichecks.eu/def/isInputFor
:isInputFor rdf:type owl:NamedIndividual ;
            <http://www.w3.org/2004/02/skos/core#prefLabel> "is input for" .


###  https://data.digichecks.eu/def/isMadeBy
:isMadeBy rdf:type owl:NamedIndividual ;
          <http://www.w3.org/2004/02/skos/core#prefLabel> "is made by" .


###  https://data.digichecks.eu/def/isParcelFor
:isParcelFor rdf:type owl:NamedIndividual ;
             <http://www.w3.org/2004/02/skos/core#prefLabel> "is parcel for" .


###  https://data.digichecks.eu/def/isPermitFor
:isPermitFor rdf:type owl:NamedIndividual ;
             <http://www.w3.org/2004/02/skos/core#prefLabel> "is permit for" .


###  https://data.digichecks.eu/def/isPermitForRequest
:isPermitForRequest rdf:type owl:NamedIndividual ;
                    <http://www.w3.org/2004/02/skos/core#prefLabel> "is permit for request" .


###  https://data.digichecks.eu/def/isRequestForPermit
:isRequestForPermit rdf:type owl:NamedIndividual ;
                    <http://www.w3.org/2004/02/skos/core#prefLabel> "is request for permit" .


###  https://data.digichecks.eu/def/isSubmittedBy
:isSubmittedBy rdf:type owl:NamedIndividual ;
               <http://www.w3.org/2004/02/skos/core#prefLabel> "is submitted by" .


###  https://data.digichecks.eu/def/isVerifiedIn
:isVerifiedIn rdf:type owl:NamedIndividual ;
              <http://www.w3.org/2004/02/skos/core#prefLabel> "is verified in" .


###  https://data.digichecks.eu/def/logicalOperator
:logicalOperator rdf:type owl:NamedIndividual ;
                 <http://www.w3.org/2004/02/skos/core#prefLabel> "logical operator" .


###  https://data.digichecks.eu/def/role
:role rdf:type owl:NamedIndividual ;
      <http://www.w3.org/2004/02/skos/core#prefLabel> "role" .


###  https://data.digichecks.eu/def/shallBeCompliantWith
:shallBeCompliantWith rdf:type owl:NamedIndividual ;
                      <http://www.w3.org/2004/02/skos/core#prefLabel> "shall be compliant with" .


###  https://data.digichecks.eu/def/wasDescribedBy
:wasDescribedBy rdf:type owl:NamedIndividual ;
                <http://www.w3.org/2004/02/skos/core#prefLabel> "was described by" .


###  https://data.digichecks.eu/def/34e82a97-fdd5-3176-ab61-f75c778939ca
<https://data.digichecks.eu/def/34e82a97-fdd5-3176-ab61-f75c778939ca> rdf:type owl:NamedIndividual ;
                                                                      <http://www.w3.org/2004/02/skos/core#prefLabel> "outcomes for Decision for permits" .


###  https://data.digichecks.eu/def/64b000ca27b0605cddb2d646
<https://data.digichecks.eu/def/64b000ca27b0605cddb2d646> rdf:type owl:NamedIndividual ,
                                                                   <http://www.w3.org/ns/shacl#NodeShape> ;
                                                          <http://www.w3.org/ns/shacl#property> _:genid3 ,
                                                                                                _:genid4 ,
                                                                                                _:genid5 ,
                                                                                                _:genid6 ;
                                                          <http://www.w3.org/ns/shacl#targetClass> <https://w3id.org/sml/def#TopConcept> .

_:genid3 <http://www.w3.org/ns/shacl#class> <https://w3id.org/idsa/core/Resource> ;
          <http://www.w3.org/ns/shacl#path> <https://w3id.org/sml/def#isDescribedBy> .

_:genid4 <http://www.w3.org/ns/shacl#class> <https://w3id.org/idsa/core/Resource> ;
          <http://www.w3.org/ns/shacl#path> :wasDescribedBy .

_:genid5 <http://www.w3.org/ns/shacl#datatype> xsd:string ;
          <http://www.w3.org/ns/shacl#path> <http://www.w3.org/2004/02/skos/core#prefLabel> .

_:genid6 <http://www.w3.org/ns/shacl#datatype> xsd:string ;
          <http://www.w3.org/ns/shacl#path> rdfs:comment .


###  https://data.digichecks.eu/def/64b000d827b0605cddb2d64c
<https://data.digichecks.eu/def/64b000d827b0605cddb2d64c> rdf:type owl:NamedIndividual ,
                                                                   <http://www.w3.org/ns/shacl#NodeShape> ;
                                                          <http://www.w3.org/ns/shacl#property> _:genid7 ,
                                                                                                _:genid8 ,
                                                                                                _:genid9 ;
                                                          <http://www.w3.org/ns/shacl#targetClass> :Allocation .

_:genid7 <http://www.w3.org/ns/shacl#class> :Verification ;
          <http://www.w3.org/ns/shacl#path> :isVerifiedIn .

_:genid8 <http://www.w3.org/ns/shacl#class> <https://w3id.org/sml/def#TopConcept> ;
          <http://www.w3.org/ns/shacl#path> :isAllocationfor ;
          <http://www.w3.org/ns/shacl#maxCount> 1 ;
          <http://www.w3.org/ns/shacl#minCount> 1 .

_:genid9 <http://www.w3.org/ns/shacl#class> <https://w3id.org/sml/def#Requirement> ;
          <http://www.w3.org/ns/shacl#path> <https://w3id.org/sml/def#hasRequirement> ;
          <http://www.w3.org/ns/shacl#maxCount> 1 ;
          <http://www.w3.org/ns/shacl#minCount> 1 .


###  https://data.digichecks.eu/def/64d4a25fec98ce2e4c41a07d
<https://data.digichecks.eu/def/64d4a25fec98ce2e4c41a07d> rdf:type owl:NamedIndividual ,
                                                                   <http://www.w3.org/ns/shacl#NodeShape> ;
                                                          <http://www.w3.org/ns/shacl#property> _:genid10 ,
                                                                                                _:genid12 ,
                                                                                                _:genid13 ,
                                                                                                _:genid14 ;
                                                          <http://www.w3.org/ns/shacl#targetClass> :Verification .

_:genid10 <http://www.w3.org/ns/shacl#or> [ ] ;
<http://www.w3.org/ns/shacl#path> :hasAsOutput .

_:genid12 <http://www.w3.org/ns/shacl#class> :VerificationMethod ;
           <http://www.w3.org/ns/shacl#path> :hasVerificationMethod ;
           <http://www.w3.org/ns/shacl#maxCount> 1 ;
           <http://www.w3.org/ns/shacl#minCount> 1 .

_:genid13 <http://www.w3.org/ns/shacl#class> <http://www.w3.org/ns/prov#Agent> ;
           <http://www.w3.org/ns/shacl#path> <http://www.w3.org/ns/prov#wasAssociatedWith> ;
           <http://www.w3.org/ns/shacl#maxCount> 1 ;
           <http://www.w3.org/ns/shacl#minCount> 1 .

_:genid14 <http://www.w3.org/ns/shacl#class> :Decision ;
           <http://www.w3.org/ns/shacl#path> :isInputFor ;
           <http://www.w3.org/ns/shacl#minCount> 1 .


###  https://data.digichecks.eu/def/64d5f40dec98ce2e4c41a100
<https://data.digichecks.eu/def/64d5f40dec98ce2e4c41a100> rdf:type owl:NamedIndividual ,
                                                                   <http://www.w3.org/ns/shacl#NodeShape> ;
                                                          <http://www.w3.org/ns/shacl#property> _:genid15 ,
                                                                                                _:genid16 ,
                                                                                                _:genid17 ;
                                                          <http://www.w3.org/ns/shacl#targetClass> <http://www.w3.org/ns/prov#Agent> .

_:genid15 <http://www.w3.org/ns/shacl#class> <http://www.w3.org/ns/prov#Agent> ;
           <http://www.w3.org/ns/shacl#path> <http://www.w3.org/ns/prov#actedOnBehalfOf> .

_:genid16 <http://www.w3.org/ns/shacl#datatype> xsd:string ;
           <http://www.w3.org/ns/shacl#path> rdfs:comment .

_:genid17 <http://www.w3.org/ns/shacl#datatype> xsd:string ;
           <http://www.w3.org/ns/shacl#path> <http://www.w3.org/2004/02/skos/core#prefLabel> .


###  https://data.digichecks.eu/def/64da30f3ec98ce2e4c41a20b
<https://data.digichecks.eu/def/64da30f3ec98ce2e4c41a20b> rdf:type owl:NamedIndividual ,
                                                                   <http://www.w3.org/ns/shacl#NodeShape> ;
                                                          <http://www.w3.org/ns/shacl#property> _:genid18 ,
                                                                                                _:genid19 ,
                                                                                                _:genid20 ,
                                                                                                _:genid21 ;
                                                          <http://www.w3.org/ns/shacl#targetClass> :Project .

_:genid18 <http://www.w3.org/ns/shacl#class> <https://w3id.org/sml/def#TopConcept> ;
           <http://www.w3.org/ns/shacl#path> <http://purl.org/dc/terms/subject> .

_:genid19 <http://www.w3.org/ns/shacl#class> <http://www.w3.org/ns/prov#Association> ;
           <http://www.w3.org/ns/shacl#path> <http://www.w3.org/ns/prov#qualifiedAssociation> ;
           <http://www.w3.org/ns/shacl#minCount> 1 .

_:genid20 <http://www.w3.org/ns/shacl#class> <http://www.w3.org/ns/prov#Location> ;
           <http://www.w3.org/ns/shacl#path> <http://www.w3.org/ns/prov#atLocation> .

_:genid21 <http://www.w3.org/ns/shacl#class> :PermitRequest ;
           <http://www.w3.org/ns/shacl#path> :hasPermitRequest .


###  https://data.digichecks.eu/def/64da320fec98ce2e4c41a220
<https://data.digichecks.eu/def/64da320fec98ce2e4c41a220> rdf:type owl:NamedIndividual ,
                                                                   <http://www.w3.org/ns/shacl#NodeShape> ;
                                                          <http://www.w3.org/ns/shacl#property> _:genid22 ,
                                                                                                _:genid23 ,
                                                                                                _:genid24 ,
                                                                                                _:genid26 ;
                                                          <http://www.w3.org/ns/shacl#targetClass> <https://w3id.org/sml/def#Requirement> .

_:genid22 <http://www.w3.org/ns/shacl#class> <https://w3id.org/sml/def#Requirement> ;
           <http://www.w3.org/ns/shacl#path> <https://w3id.org/sml/def#hasPart> .

_:genid23 <http://www.w3.org/ns/shacl#class> :Document ;
           <http://www.w3.org/ns/shacl#path> :hasSource .

_:genid24 <http://www.w3.org/ns/shacl#or> [ ] ;
<http://www.w3.org/ns/shacl#path> :isExpressedAs .

_:genid26 <http://www.w3.org/ns/shacl#in> <https://data.digichecks.eu/def/95414b38-5a62-3cf9-beed-42cbc73f4b9e> ;
           <http://www.w3.org/ns/shacl#path> :logicalOperator ;
           <http://www.w3.org/ns/shacl#maxCount> 1 .


###  https://data.digichecks.eu/def/64da327fec98ce2e4c41a229
<https://data.digichecks.eu/def/64da327fec98ce2e4c41a229> rdf:type owl:NamedIndividual ,
                                                                   <http://www.w3.org/ns/shacl#NodeShape> ;
                                                          <http://www.w3.org/ns/shacl#property> _:genid27 ,
                                                                                                _:genid28 ,
                                                                                                _:genid29 ,
                                                                                                _:genid30 ;
                                                          <http://www.w3.org/ns/shacl#targetClass> :Permit .

_:genid27 <http://www.w3.org/ns/shacl#class> <https://w3id.org/idsa/core/Resource> ;
           <http://www.w3.org/ns/shacl#path> <https://w3id.org/sml/def#isDescribedBy> ;
           <http://www.w3.org/ns/shacl#minCount> 1 .

_:genid28 <http://www.w3.org/ns/shacl#class> :PermitRequest ;
           <http://www.w3.org/ns/shacl#path> :isPermitFor ;
           <http://www.w3.org/ns/shacl#minCount> 1 .

_:genid29 <http://www.w3.org/ns/shacl#class> <https://w3id.org/sml/def#Requirement> ;
           <http://www.w3.org/ns/shacl#path> <https://w3id.org/sml/def#hasRequirement> ;
           <http://www.w3.org/ns/shacl#minCount> 1 .

_:genid30 <http://www.w3.org/ns/shacl#class> :Permit ;
           <http://www.w3.org/ns/shacl#path> <https://w3id.org/sml/def#hasPart> .


###  https://data.digichecks.eu/def/64da32f2ec98ce2e4c41a232
<https://data.digichecks.eu/def/64da32f2ec98ce2e4c41a232> rdf:type owl:NamedIndividual ,
                                                                   <http://www.w3.org/ns/shacl#NodeShape> ;
                                                          <http://www.w3.org/ns/shacl#property> _:genid31 ,
                                                                                                _:genid32 ,
                                                                                                _:genid33 ;
                                                          <http://www.w3.org/ns/shacl#targetClass> :Decision .

_:genid31 <http://www.w3.org/ns/shacl#class> <http://www.w3.org/ns/prov#Agent> ;
           <http://www.w3.org/ns/shacl#path> <http://www.w3.org/ns/prov#wasAssociatedWith> ;
           <http://www.w3.org/ns/shacl#maxCount> 1 ;
           <http://www.w3.org/ns/shacl#minCount> 1 .

_:genid32 <http://www.w3.org/ns/shacl#class> :PermitRequest ;
           <http://www.w3.org/ns/shacl#path> :isDecisionFor ;
           <http://www.w3.org/ns/shacl#maxCount> 1 ;
           <http://www.w3.org/ns/shacl#minCount> 1 .

_:genid33 <http://www.w3.org/ns/shacl#in> <https://data.digichecks.eu/def/34e82a97-fdd5-3176-ab61-f75c778939ca> ;
           <http://www.w3.org/ns/shacl#path> :decisionOutcome ;
           <http://www.w3.org/ns/shacl#maxCount> 1 .


###  https://data.digichecks.eu/def/64ddde554ef5931bfc406a34
<https://data.digichecks.eu/def/64ddde554ef5931bfc406a34> rdf:type owl:NamedIndividual ,
                                                                   <http://www.w3.org/ns/shacl#NodeShape> ;
                                                          <http://www.w3.org/ns/shacl#property> _:genid34 ,
                                                                                                _:genid35 ,
                                                                                                _:genid36 ,
                                                                                                _:genid37 ,
                                                                                                _:genid38 ;
                                                          <http://www.w3.org/ns/shacl#targetClass> <http://www.w3.org/ns/prov#Location> .

_:genid34 <http://www.w3.org/ns/shacl#datatype> xsd:string ;
           <http://www.w3.org/ns/shacl#path> <http://www.w3.org/2004/02/skos/core#prefLabel> .

_:genid35 <http://www.w3.org/ns/shacl#datatype> xsd:string ;
           <http://www.w3.org/ns/shacl#path> rdfs:comment .

_:genid36 <http://www.w3.org/ns/shacl#class> <http://www.opengis.net/ont/geosparql#Geometry> ;
           <http://www.w3.org/ns/shacl#path> <http://www.opengis.net/ont/geosparql#hasGeometry> ;
           <http://www.w3.org/ns/shacl#maxCount> 1 .

_:genid37 <http://www.w3.org/ns/shacl#class> <http://www.w3.org/2006/vcard/ns#Address> ;
           <http://www.w3.org/ns/shacl#path> <http://www.w3.org/2006/vcard/ns#hasAddress> ;
           <http://www.w3.org/ns/shacl#maxCount> 1 .

_:genid38 <http://www.w3.org/ns/shacl#class> :Parcel ;
           <http://www.w3.org/ns/shacl#path> :hasParcel ;
           <http://www.w3.org/ns/shacl#maxCount> 1 .


###  https://data.digichecks.eu/def/64dde72c4ef5931bfc406a64
<https://data.digichecks.eu/def/64dde72c4ef5931bfc406a64> rdf:type owl:NamedIndividual ,
                                                                   <http://www.w3.org/ns/shacl#NodeShape> ;
                                                          <http://www.w3.org/ns/shacl#targetClass> :Document .


###  https://data.digichecks.eu/def/64eccb68d8a9bc575cd0c914
<https://data.digichecks.eu/def/64eccb68d8a9bc575cd0c914> rdf:type owl:NamedIndividual ,
                                                                   <http://www.w3.org/ns/shacl#NodeShape> ;
                                                          <http://www.w3.org/ns/shacl#property> _:genid39 ,
                                                                                                _:genid40 ,
                                                                                                _:genid41 ,
                                                                                                _:genid42 ;
                                                          <http://www.w3.org/ns/shacl#targetClass> <http://www.w3.org/ns/shacl#NodeShape> .

_:genid39 <http://www.w3.org/ns/shacl#class> <https://w3id.org/idsa/core/Resource> ;
           <http://www.w3.org/ns/shacl#path> :wasDescribedBy .

_:genid40 <http://www.w3.org/ns/shacl#class> <https://w3id.org/idsa/core/Resource> ;
           <http://www.w3.org/ns/shacl#path> <https://w3id.org/sml/def#isDescribedBy> .

_:genid41 <http://www.w3.org/ns/shacl#datatype> xsd:string ;
           <http://www.w3.org/ns/shacl#path> <http://www.w3.org/2004/02/skos/core#prefLabel> .

_:genid42 <http://www.w3.org/ns/shacl#datatype> xsd:string ;
           <http://www.w3.org/ns/shacl#path> rdfs:comment .


###  https://data.digichecks.eu/def/65d3dc1c13b8ea5093980dfc
<https://data.digichecks.eu/def/65d3dc1c13b8ea5093980dfc> rdf:type owl:NamedIndividual ,
                                                                   <http://www.w3.org/ns/shacl#NodeShape> ;
                                                          <http://www.w3.org/ns/shacl#property> _:genid43 ,
                                                                                                _:genid44 ;
                                                          <http://www.w3.org/ns/shacl#targetClass> <http://www.w3.org/ns/prov#Association> .

_:genid43 <http://www.w3.org/ns/shacl#path> :role .

_:genid44 <http://www.w3.org/ns/shacl#class> <http://www.w3.org/ns/prov#Agent> ;
           <http://www.w3.org/ns/shacl#path> <http://www.w3.org/ns/prov#agent> ;
           <http://www.w3.org/ns/shacl#maxCount> 1 ;
           <http://www.w3.org/ns/shacl#minCount> 1 .


###  https://data.digichecks.eu/def/65e60b91ebc1577ef9381cbb
<https://data.digichecks.eu/def/65e60b91ebc1577ef9381cbb> rdf:type owl:NamedIndividual ,
                                                                   <http://www.w3.org/ns/shacl#NodeShape> ;
                                                          <http://www.w3.org/ns/shacl#property> _:genid45 ,
                                                                                                _:genid46 ,
                                                                                                _:genid47 ,
                                                                                                _:genid48 ;
                                                          <http://www.w3.org/ns/shacl#targetClass> :PermitRequest .

_:genid45 <http://www.w3.org/ns/shacl#class> :Project ;
           <http://www.w3.org/ns/shacl#path> :isPermitForRequest ;
           <http://www.w3.org/ns/shacl#minCount> 1 .

_:genid46 <http://www.w3.org/ns/shacl#class> <http://www.w3.org/ns/prov#Agent> ;
           <http://www.w3.org/ns/shacl#path> :isSubmittedBy ;
           <http://www.w3.org/ns/shacl#minCount> 1 .

_:genid47 <http://www.w3.org/ns/shacl#class> <http://www.w3.org/ns/prov#Agent> ;
           <http://www.w3.org/ns/shacl#path> :isControlledBy .

_:genid48 <http://www.w3.org/ns/shacl#class> :Permit ;
           <http://www.w3.org/ns/shacl#path> :isRequestForPermit ;
           <http://www.w3.org/ns/shacl#maxCount> 1 .


###  https://data.digichecks.eu/def/6606a7ae965733652c7f6783
<https://data.digichecks.eu/def/6606a7ae965733652c7f6783> rdf:type owl:NamedIndividual ,
                                                                   <http://www.w3.org/ns/shacl#NodeShape> ;
                                                          <http://www.w3.org/ns/shacl#property> _:genid49 ,
                                                                                                _:genid50 ,
                                                                                                _:genid51 ;
                                                          <http://www.w3.org/ns/shacl#targetClass> <http://www.w3.org/ns/shacl#ValidationReport> .

_:genid49 <http://www.w3.org/ns/shacl#class> <https://w3id.org/idsa/core/Resource> ;
           <http://www.w3.org/ns/shacl#path> <https://w3id.org/sml/def#isDescribedBy> .

_:genid50 <http://www.w3.org/ns/shacl#datatype> xsd:string ;
           <http://www.w3.org/ns/shacl#path> <http://www.w3.org/2004/02/skos/core#prefLabel> .

_:genid51 <http://www.w3.org/ns/shacl#datatype> xsd:string ;
           <http://www.w3.org/ns/shacl#path> rdfs:comment .


###  https://data.digichecks.eu/def/661525befd34eb2f8e03f5a4
<https://data.digichecks.eu/def/661525befd34eb2f8e03f5a4> rdf:type owl:NamedIndividual ,
                                                                   <http://www.w3.org/ns/shacl#NodeShape> ;
                                                          <http://www.w3.org/ns/shacl#property> _:genid52 ,
                                                                                                _:genid53 ,
                                                                                                _:genid54 ;
                                                          <http://www.w3.org/ns/shacl#targetClass> <http://www.opengis.net/ont/geosparql#Geometry> .

_:genid52 <http://www.w3.org/ns/shacl#class> <http://www.w3.org/ns/prov#Location> ;
           <http://www.w3.org/ns/shacl#path> :isGeometryOf ;
           <http://www.w3.org/ns/shacl#maxCount> 1 ;
           <http://www.w3.org/ns/shacl#minCount> 1 .

_:genid53 <http://www.w3.org/ns/shacl#datatype> xsd:string ;
           <http://www.w3.org/ns/shacl#path> <http://www.w3.org/2004/02/skos/core#prefLabel> .

_:genid54 <http://www.w3.org/ns/shacl#datatype> xsd:string ;
           <http://www.w3.org/ns/shacl#path> rdfs:comment .


###  https://data.digichecks.eu/def/661525d6fd34eb2f8e03f5b4
<https://data.digichecks.eu/def/661525d6fd34eb2f8e03f5b4> rdf:type owl:NamedIndividual ,
                                                                   <http://www.w3.org/ns/shacl#NodeShape> ;
                                                          <http://www.w3.org/ns/shacl#property> _:genid55 ,
                                                                                                _:genid56 ,
                                                                                                _:genid57 ;
                                                          <http://www.w3.org/ns/shacl#targetClass> :Parcel .

_:genid55 <http://www.w3.org/ns/shacl#datatype> xsd:string ;
           <http://www.w3.org/ns/shacl#path> <http://www.w3.org/2004/02/skos/core#prefLabel> .

_:genid56 <http://www.w3.org/ns/shacl#datatype> xsd:string ;
           <http://www.w3.org/ns/shacl#path> rdfs:comment .

_:genid57 <http://www.w3.org/ns/shacl#class> <http://www.w3.org/ns/prov#Location> ;
           <http://www.w3.org/ns/shacl#path> :isParcelFor ;
           <http://www.w3.org/ns/shacl#maxCount> 1 ;
           <http://www.w3.org/ns/shacl#minCount> 1 .


###  https://data.digichecks.eu/def/661525e1fd34eb2f8e03f5bc
<https://data.digichecks.eu/def/661525e1fd34eb2f8e03f5bc> rdf:type owl:NamedIndividual ,
                                                                   <http://www.w3.org/ns/shacl#NodeShape> ;
                                                          <http://www.w3.org/ns/shacl#property> _:genid58 ,
                                                                                                _:genid59 ;
                                                          <http://www.w3.org/ns/shacl#targetClass> <https://w3id.org/idsa/core/Resource> .

_:genid58 <http://www.w3.org/ns/shacl#datatype> xsd:string ;
           <http://www.w3.org/ns/shacl#path> <http://www.w3.org/2004/02/skos/core#prefLabel> .

_:genid59 <http://www.w3.org/ns/shacl#datatype> xsd:string ;
           <http://www.w3.org/ns/shacl#path> rdfs:comment .


###  https://data.digichecks.eu/def/6615257dfd34eb2f8e03f59a
<https://data.digichecks.eu/def/6615257dfd34eb2f8e03f59a> rdf:type owl:NamedIndividual ,
                                                                   <http://www.w3.org/ns/shacl#NodeShape> ;
                                                          <http://www.w3.org/ns/shacl#property> _:genid60 ,
                                                                                                _:genid61 ,
                                                                                                _:genid62 ;
                                                          <http://www.w3.org/ns/shacl#targetClass> <http://www.w3.org/2006/vcard/ns#Address> .

_:genid60 <http://www.w3.org/ns/shacl#class> <http://www.w3.org/ns/prov#Location> ;
           <http://www.w3.org/ns/shacl#path> :isAddressFor ;
           <http://www.w3.org/ns/shacl#maxCount> 1 ;
           <http://www.w3.org/ns/shacl#minCount> 1 .

_:genid61 <http://www.w3.org/ns/shacl#datatype> xsd:string ;
           <http://www.w3.org/ns/shacl#path> <http://www.w3.org/2004/02/skos/core#prefLabel> .

_:genid62 <http://www.w3.org/ns/shacl#datatype> xsd:string ;
           <http://www.w3.org/ns/shacl#path> rdfs:comment .


###  https://data.digichecks.eu/def/95414b38-5a62-3cf9-beed-42cbc73f4b9e
<https://data.digichecks.eu/def/95414b38-5a62-3cf9-beed-42cbc73f4b9e> rdf:type owl:NamedIndividual ;
                                                                      <http://www.w3.org/2004/02/skos/core#prefLabel> "Logical operator list for requirements" .


###  https://w3id.org/idsa/core/Resource
<https://w3id.org/idsa/core/Resource> rdf:type owl:NamedIndividual ;
                                      <http://www.w3.org/2004/02/skos/core#prefLabel> "Resource" .


###  https://w3id.org/sml/def#AbstractConcept
<https://w3id.org/sml/def#AbstractConcept> rdf:type owl:NamedIndividual ;
                                           <http://www.w3.org/2004/02/skos/core#prefLabel> "Abstract Concept" .


###  https://w3id.org/sml/def#Activity
<https://w3id.org/sml/def#Activity> rdf:type owl:NamedIndividual ;
                                    <http://www.w3.org/2004/02/skos/core#prefLabel> "Activity" .


###  https://w3id.org/sml/def#ConceptType
<https://w3id.org/sml/def#ConceptType> rdf:type owl:NamedIndividual ;
                                       <http://www.w3.org/2004/02/skos/core#prefLabel> "Concept Type" .


###  https://w3id.org/sml/def#ConcreteConcept
<https://w3id.org/sml/def#ConcreteConcept> rdf:type owl:NamedIndividual ;
                                           <http://www.w3.org/2004/02/skos/core#prefLabel> "Concrete Concept" .


###  https://w3id.org/sml/def#Entity
<https://w3id.org/sml/def#Entity> rdf:type owl:NamedIndividual ;
                                  <http://www.w3.org/2004/02/skos/core#prefLabel> "Entitiy" .


###  https://w3id.org/sml/def#EnumerationType
<https://w3id.org/sml/def#EnumerationType> rdf:type owl:NamedIndividual ;
                                           <http://www.w3.org/2004/02/skos/core#prefLabel> "Enumeration Type" .


###  https://w3id.org/sml/def#Event
<https://w3id.org/sml/def#Event> rdf:type owl:NamedIndividual ;
                                 <http://www.w3.org/2004/02/skos/core#prefLabel> "Event" .


###  https://w3id.org/sml/def#GeometricEntity
<https://w3id.org/sml/def#GeometricEntity> rdf:type owl:NamedIndividual ;
                                           <http://www.w3.org/2004/02/skos/core#prefLabel> "Geometric Entity" .


###  https://w3id.org/sml/def#InformationObject
<https://w3id.org/sml/def#InformationObject> rdf:type owl:NamedIndividual ;
                                             <http://www.w3.org/2004/02/skos/core#prefLabel> "Information Object" .


###  https://w3id.org/sml/def#Object
<https://w3id.org/sml/def#Object> rdf:type owl:NamedIndividual ;
                                  <http://www.w3.org/2004/02/skos/core#prefLabel> "Object" .


###  https://w3id.org/sml/def#Objectification
<https://w3id.org/sml/def#Objectification> rdf:type owl:NamedIndividual ;
                                           <http://www.w3.org/2004/02/skos/core#prefLabel> "Objectification" .


###  https://w3id.org/sml/def#PhysicalObject
<https://w3id.org/sml/def#PhysicalObject> rdf:type owl:NamedIndividual ;
                                          <http://www.w3.org/2004/02/skos/core#prefLabel> "Physical Object" .


###  https://w3id.org/sml/def#QualityValue
<https://w3id.org/sml/def#QualityValue> rdf:type owl:NamedIndividual ;
                                        <http://www.w3.org/2004/02/skos/core#prefLabel> "Quality Value" .


###  https://w3id.org/sml/def#QuantityValue
<https://w3id.org/sml/def#QuantityValue> rdf:type owl:NamedIndividual ;
                                         <http://www.w3.org/2004/02/skos/core#prefLabel> "Quantity Value" .


###  https://w3id.org/sml/def#RelationReference
<https://w3id.org/sml/def#RelationReference> rdf:type owl:NamedIndividual ;
                                             <http://www.w3.org/2004/02/skos/core#prefLabel> "Relation Reference" .


###  https://w3id.org/sml/def#Representation
<https://w3id.org/sml/def#Representation> rdf:type owl:NamedIndividual ;
                                          <http://www.w3.org/2004/02/skos/core#prefLabel> "Representation" .


###  https://w3id.org/sml/def#Requirement
<https://w3id.org/sml/def#Requirement> rdf:type owl:NamedIndividual ;
                                       <http://www.w3.org/2004/02/skos/core#prefLabel> "Requirement" .


###  https://w3id.org/sml/def#State
<https://w3id.org/sml/def#State> rdf:type owl:NamedIndividual ;
                                 <http://www.w3.org/2004/02/skos/core#prefLabel> "State" .


###  https://w3id.org/sml/def#TemporalEntity
<https://w3id.org/sml/def#TemporalEntity> rdf:type owl:NamedIndividual ;
                                          <http://www.w3.org/2004/02/skos/core#prefLabel> "Temporal Entity" .


###  https://w3id.org/sml/def#TopConcept
<https://w3id.org/sml/def#TopConcept> rdf:type owl:NamedIndividual ;
                                      <http://www.w3.org/2004/02/skos/core#prefLabel> "Top Concept" .


###  https://w3id.org/sml/def#Type
<https://w3id.org/sml/def#Type> rdf:type owl:NamedIndividual ;
                                <http://www.w3.org/2004/02/skos/core#prefLabel> "Type" .


###  https://w3id.org/sml/def#hasPart
<https://w3id.org/sml/def#hasPart> rdf:type owl:NamedIndividual ;
                                   <http://www.w3.org/2004/02/skos/core#prefLabel> "has part" .


###  https://w3id.org/sml/def#hasRequirement
<https://w3id.org/sml/def#hasRequirement> rdf:type owl:NamedIndividual ;
                                          <http://www.w3.org/2004/02/skos/core#prefLabel> "has requirement" .


###  https://w3id.org/sml/def#isDescribedBy
<https://w3id.org/sml/def#isDescribedBy> rdf:type owl:NamedIndividual ;
                                         <http://www.w3.org/2004/02/skos/core#prefLabel> "is described by" .


[ <http://www.w3.org/ns/shacl#class> <http://www.w3.org/ns/shacl#ValidationReport>
] .

[ <http://www.w3.org/ns/shacl#class> :MachineReadableRule
 ] .

[ <http://www.w3.org/ns/shacl#class> <http://www.w3.org/ns/shacl#NodeShape>
 ] .

[ <http://www.w3.org/ns/shacl#class> :Document
 ] .

#################################################################
#    Annotations
#################################################################

rdfs:Class rdfs:isDefinedBy rdfs: ;
            rdfs:label "Class" .


rdfs:Container rdfs:isDefinedBy rdfs: ;
               rdfs:label "Container" .


rdfs:ContainerMembershipProperty rdfs:isDefinedBy rdfs: ;
                                 rdfs:label "ContainerMembershipProperty" .


rdfs:Datatype rdfs:isDefinedBy rdfs: ;
              rdfs:label "Datatype" .


rdfs:Literal rdfs:isDefinedBy rdfs: ;
             rdfs:label "Literal" .


rdfs:Resource rdfs:isDefinedBy rdfs: ;
              rdfs:label "Resource" .


rdfs:comment rdfs:isDefinedBy rdfs: ;
             rdfs:label "comment" .


rdfs:domain rdfs:isDefinedBy rdfs: ;
            rdfs:label "domain" .


rdfs:isDefinedBy rdfs:isDefinedBy rdfs: ;
                 rdfs:label "isDefinedBy" .


rdfs:label rdfs:isDefinedBy rdfs: ;
           rdfs:label "label" .


rdfs:member rdfs:isDefinedBy rdfs: ;
            rdfs:label "member" .


rdfs:range rdfs:isDefinedBy rdfs: ;
           rdfs:label "range" .


rdfs:seeAlso rdfs:isDefinedBy rdfs: ;
             rdfs:label "seeAlso" .


rdfs:subClassOf rdfs:isDefinedBy rdfs: ;
                rdfs:label "subClassOf" .


rdfs:subPropertyOf rdfs:isDefinedBy rdfs: ;
                   rdfs:label "subPropertyOf" .


owl:AllDifferent rdfs:isDefinedBy owl: ;
                 rdfs:label "AllDifferent" .


owl:AllDisjointClasses rdfs:isDefinedBy owl: ;
                       rdfs:label "AllDisjointClasses" .


owl:AllDisjointProperties rdfs:isDefinedBy owl: ;
                          rdfs:label "AllDisjointProperties" .


owl:Annotation rdfs:isDefinedBy owl: ;
               rdfs:label "Annotation" .


owl:AnnotationProperty rdfs:isDefinedBy owl: ;
                       rdfs:label "AnnotationProperty" .


owl:AsymmetricProperty rdfs:isDefinedBy owl: ;
                       rdfs:label "AsymmetricProperty" .


owl:Axiom rdfs:isDefinedBy owl: ;
          rdfs:label "Axiom" .


owl:Class rdfs:isDefinedBy owl: ;
          rdfs:label "Class" .


owl:DataRange rdfs:isDefinedBy owl: ;
              rdfs:label "DataRange" .


owl:DatatypeProperty rdfs:isDefinedBy owl: ;
                     rdfs:label "DatatypeProperty" .


owl:DeprecatedClass rdfs:isDefinedBy owl: ;
                    rdfs:label "DeprecatedClass" .


owl:DeprecatedProperty rdfs:isDefinedBy owl: ;
                       rdfs:label "DeprecatedProperty" .


owl:FunctionalProperty rdfs:isDefinedBy owl: ;
                       rdfs:label "FunctionalProperty" .


owl:InverseFunctionalProperty rdfs:isDefinedBy owl: ;
                              rdfs:label "InverseFunctionalProperty" .


owl:IrreflexiveProperty rdfs:isDefinedBy owl: ;
                        rdfs:label "IrreflexiveProperty" .


owl:NamedIndividual rdfs:isDefinedBy owl: ;
                    rdfs:label "NamedIndividual" .


owl:NegativePropertyAssertion rdfs:isDefinedBy owl: ;
                              rdfs:label "NegativePropertyAssertion" .


owl:Nothing rdfs:isDefinedBy owl: ;
            rdfs:label "Nothing" .


owl:ObjectProperty rdfs:isDefinedBy owl: ;
                   rdfs:label "ObjectProperty" .


owl:Ontology rdfs:isDefinedBy owl: ;
             rdfs:label "Ontology" .


owl:OntologyProperty rdfs:isDefinedBy owl: ;
                     rdfs:label "OntologyProperty" .


owl:ReflexiveProperty rdfs:isDefinedBy owl: ;
                      rdfs:label "ReflexiveProperty" .


owl:Restriction rdfs:isDefinedBy owl: ;
                rdfs:label "Restriction" .


owl:SymmetricProperty rdfs:isDefinedBy owl: ;
                      rdfs:label "SymmetricProperty" .


owl:Thing rdfs:isDefinedBy owl: ;
          rdfs:label "Thing" .


owl:TransitiveProperty rdfs:isDefinedBy owl: ;
                       rdfs:label "TransitiveProperty" .


owl:allValuesFrom rdfs:isDefinedBy owl: ;
                  rdfs:label "allValuesFrom" .


owl:annotatedProperty rdfs:isDefinedBy owl: ;
                      rdfs:label "annotatedProperty" .


owl:annotatedSource rdfs:isDefinedBy owl: ;
                    rdfs:label "annotatedSource" .


owl:annotatedTarget rdfs:isDefinedBy owl: ;
                    rdfs:label "annotatedTarget" .


owl:assertionProperty rdfs:isDefinedBy owl: ;
                      rdfs:label "assertionProperty" .


owl:backwardCompatibleWith rdfs:isDefinedBy owl: ;
                           rdfs:label "backwardCompatibleWith" .


owl:bottomDataProperty rdfs:isDefinedBy owl: ;
                       rdfs:label "bottomDataProperty" .


owl:bottomObjectProperty rdfs:isDefinedBy owl: ;
                         rdfs:label "bottomObjectProperty" .


owl:cardinality rdfs:isDefinedBy owl: ;
                rdfs:label "cardinality" .


owl:complementOf rdfs:isDefinedBy owl: ;
                 rdfs:label "complementOf" .


owl:datatypeComplementOf rdfs:isDefinedBy owl: ;
                         rdfs:label "datatypeComplementOf" .


owl:deprecated rdfs:isDefinedBy owl: ;
               rdfs:label "deprecated" .


owl:differentFrom rdfs:isDefinedBy owl: ;
                  rdfs:label "differentFrom" .


owl:disjointUnionOf rdfs:isDefinedBy owl: ;
                    rdfs:label "disjointUnionOf" .


owl:disjointWith rdfs:isDefinedBy owl: ;
                 rdfs:label "disjointWith" .


owl:distinctMembers rdfs:isDefinedBy owl: ;
                    rdfs:label "distinctMembers" .


owl:equivalentClass rdfs:isDefinedBy owl: ;
                    rdfs:label "equivalentClass" .


owl:equivalentProperty rdfs:isDefinedBy owl: ;
                       rdfs:label "equivalentProperty" .


owl:hasKey rdfs:isDefinedBy owl: ;
           rdfs:label "hasKey" .


owl:hasSelf rdfs:isDefinedBy owl: ;
            rdfs:label "hasSelf" .


owl:hasValue rdfs:isDefinedBy owl: ;
             rdfs:label "hasValue" .


owl:imports rdfs:isDefinedBy owl: ;
            rdfs:label "imports" .


owl:incompatibleWith rdfs:isDefinedBy owl: ;
                     rdfs:label "incompatibleWith" .


owl:intersectionOf rdfs:isDefinedBy owl: ;
                   rdfs:label "intersectionOf" .


owl:inverseOf rdfs:isDefinedBy owl: ;
              rdfs:label "inverseOf" .


owl:maxCardinality rdfs:isDefinedBy owl: ;
                   rdfs:label "maxCardinality" .


owl:maxQualifiedCardinality rdfs:isDefinedBy owl: ;
                            rdfs:label "maxQualifiedCardinality" .


owl:members rdfs:isDefinedBy owl: ;
            rdfs:label "members" .


owl:minCardinality rdfs:isDefinedBy owl: ;
                   rdfs:label "minCardinality" .


owl:minQualifiedCardinality rdfs:isDefinedBy owl: ;
                            rdfs:label "minQualifiedCardinality" .


owl:onClass rdfs:isDefinedBy owl: ;
            rdfs:label "onClass" .


owl:onDataRange rdfs:isDefinedBy owl: ;
                rdfs:label "onDataRange" .


owl:onDatatype rdfs:isDefinedBy owl: ;
               rdfs:label "onDatatype" .


owl:onProperties rdfs:isDefinedBy owl: ;
                 rdfs:label "onProperties" .


owl:onProperty rdfs:isDefinedBy owl: ;
               rdfs:label "onProperty" .


owl:oneOf rdfs:isDefinedBy owl: ;
          rdfs:label "oneOf" .


owl:priorVersion rdfs:isDefinedBy owl: ;
                 rdfs:label "priorVersion" .


owl:propertyChainAxiom rdfs:isDefinedBy owl: ;
                       rdfs:label "propertyChainAxiom" .


owl:propertyDisjointWith rdfs:isDefinedBy owl: ;
                         rdfs:label "propertyDisjointWith" .


owl:qualifiedCardinality rdfs:isDefinedBy owl: ;
                         rdfs:label "qualifiedCardinality" .


owl:sameAs rdfs:isDefinedBy owl: ;
           rdfs:label "sameAs" .


owl:someValuesFrom rdfs:isDefinedBy owl: ;
                   rdfs:label "someValuesFrom" .


owl:sourceIndividual rdfs:isDefinedBy owl: ;
                     rdfs:label "sourceIndividual" .


owl:targetIndividual rdfs:isDefinedBy owl: ;
                     rdfs:label "targetIndividual" .


owl:targetValue rdfs:isDefinedBy owl: ;
                rdfs:label "targetValue" .


owl:topDataProperty rdfs:isDefinedBy owl: ;
                    rdfs:label "topDataProperty" .


owl:topObjectProperty rdfs:isDefinedBy owl: ;
                      rdfs:label "topObjectProperty" .


owl:unionOf rdfs:isDefinedBy owl: ;
            rdfs:label "unionOf" .


owl:versionIRI rdfs:isDefinedBy owl: ;
               rdfs:label "versionIRI" .


owl:versionInfo rdfs:isDefinedBy owl: ;
                rdfs:label "versionInfo" .


owl:withRestrictions rdfs:isDefinedBy owl: ;
                     rdfs:label "withRestrictions" .


<http://www.w3.org/ns/shacl#AbstractResult> rdfs:isDefinedBy <http://www.w3.org/ns/shacl#> ;
                                            rdfs:label "Abstract result"@en .


<http://www.w3.org/ns/shacl#ConstraintComponent> rdfs:isDefinedBy <http://www.w3.org/ns/shacl#> ;
                                                 rdfs:label "Constraint component"@en .


<http://www.w3.org/ns/shacl#Function> rdfs:isDefinedBy <http://www.w3.org/ns/shacl#> ;
                                      rdfs:label "Function"@en .


<http://www.w3.org/ns/shacl#JSConstraint> rdfs:isDefinedBy <http://www.w3.org/ns/shacl#> ;
                                          rdfs:label "JavaScript-based constraint"@en .


<http://www.w3.org/ns/shacl#JSExecutable> rdfs:isDefinedBy <http://www.w3.org/ns/shacl#> ;
                                          rdfs:label "JavaScript executable"@en .


<http://www.w3.org/ns/shacl#JSFunction> rdfs:isDefinedBy <http://www.w3.org/ns/shacl#> ;
                                        rdfs:label "JavaScript function"@en .


<http://www.w3.org/ns/shacl#JSLibrary> rdfs:isDefinedBy <http://www.w3.org/ns/shacl#> ;
                                       rdfs:label "JavaScript library"@en .


<http://www.w3.org/ns/shacl#JSRule> rdfs:isDefinedBy <http://www.w3.org/ns/shacl#> ;
                                    rdfs:label "JavaScript rule"@en .


<http://www.w3.org/ns/shacl#JSTarget> rdfs:isDefinedBy <http://www.w3.org/ns/shacl#> ;
                                      rdfs:label "JavaScript target"@en .


<http://www.w3.org/ns/shacl#JSTargetType> rdfs:isDefinedBy <http://www.w3.org/ns/shacl#> ;
                                          rdfs:label "JavaScript target type"@en .


<http://www.w3.org/ns/shacl#JSValidator> rdfs:isDefinedBy <http://www.w3.org/ns/shacl#> ;
                                         rdfs:label "JavaScript validator"@en .


<http://www.w3.org/ns/shacl#NodeKind> rdfs:isDefinedBy <http://www.w3.org/ns/shacl#> ;
                                      rdfs:label "Node kind"@en .


<http://www.w3.org/ns/shacl#NodeShape> rdfs:isDefinedBy <http://www.w3.org/ns/shacl#> ;
                                       rdfs:label "Node shape"@en .


<http://www.w3.org/ns/shacl#Parameter> rdfs:isDefinedBy <http://www.w3.org/ns/shacl#> ;
                                       rdfs:label "Parameter"@en .


<http://www.w3.org/ns/shacl#Parameterizable> rdfs:isDefinedBy <http://www.w3.org/ns/shacl#> ;
                                             rdfs:label "Parameterizable"@en .


<http://www.w3.org/ns/shacl#PrefixDeclaration> rdfs:isDefinedBy <http://www.w3.org/ns/shacl#> ;
                                               rdfs:label "Prefix declaration"@en .


<http://www.w3.org/ns/shacl#PropertyGroup> rdfs:isDefinedBy <http://www.w3.org/ns/shacl#> ;
                                           rdfs:label "Property group"@en .


<http://www.w3.org/ns/shacl#PropertyShape> rdfs:isDefinedBy <http://www.w3.org/ns/shacl#> ;
                                           rdfs:label "Property shape"@en .


<http://www.w3.org/ns/shacl#ResultAnnotation> rdfs:isDefinedBy <http://www.w3.org/ns/shacl#> ;
                                              rdfs:label "Result annotation"@en .


<http://www.w3.org/ns/shacl#Rule> rdfs:isDefinedBy <http://www.w3.org/ns/shacl#> ;
                                  rdfs:label "Rule"@en .


<http://www.w3.org/ns/shacl#SPARQLAskExecutable> rdfs:isDefinedBy <http://www.w3.org/ns/shacl#> ;
                                                 rdfs:label "SPARQL ASK executable"@en .


<http://www.w3.org/ns/shacl#SPARQLAskValidator> rdfs:isDefinedBy <http://www.w3.org/ns/shacl#> ;
                                                rdfs:label "SPARQL ASK validator"@en .


<http://www.w3.org/ns/shacl#SPARQLConstraint> rdfs:isDefinedBy <http://www.w3.org/ns/shacl#> ;
                                              rdfs:label "SPARQL constraint"@en .


<http://www.w3.org/ns/shacl#SPARQLConstructExecutable> rdfs:isDefinedBy <http://www.w3.org/ns/shacl#> ;
                                                       rdfs:label "SPARQL CONSTRUCT executable"@en .


<http://www.w3.org/ns/shacl#SPARQLExecutable> rdfs:isDefinedBy <http://www.w3.org/ns/shacl#> ;
                                              rdfs:label "SPARQL executable"@en .


<http://www.w3.org/ns/shacl#SPARQLFunction> rdfs:isDefinedBy <http://www.w3.org/ns/shacl#> ;
                                            rdfs:label "SPARQL function"@en .


<http://www.w3.org/ns/shacl#SPARQLRule> rdfs:isDefinedBy <http://www.w3.org/ns/shacl#> ;
                                        rdfs:label "SPARQL CONSTRUCT rule"@en .


<http://www.w3.org/ns/shacl#SPARQLSelectExecutable> rdfs:isDefinedBy <http://www.w3.org/ns/shacl#> ;
                                                    rdfs:label "SPARQL SELECT executable"@en .


<http://www.w3.org/ns/shacl#SPARQLSelectValidator> rdfs:isDefinedBy <http://www.w3.org/ns/shacl#> ;
                                                   rdfs:label "SPARQL SELECT validator"@en .


<http://www.w3.org/ns/shacl#SPARQLTarget> rdfs:isDefinedBy <http://www.w3.org/ns/shacl#> ;
                                          rdfs:label "SPARQL target"@en .


<http://www.w3.org/ns/shacl#SPARQLTargetType> rdfs:isDefinedBy <http://www.w3.org/ns/shacl#> ;
                                              rdfs:label "SPARQL target type"@en .


<http://www.w3.org/ns/shacl#SPARQLUpdateExecutable> rdfs:isDefinedBy <http://www.w3.org/ns/shacl#> ;
                                                    rdfs:label "SPARQL UPDATE executable"@en .


<http://www.w3.org/ns/shacl#Severity> rdfs:isDefinedBy <http://www.w3.org/ns/shacl#> ;
                                      rdfs:label "Severity"@en .


<http://www.w3.org/ns/shacl#Shape> rdfs:isDefinedBy <http://www.w3.org/ns/shacl#> ;
                                   rdfs:label "Shape"@en .


<http://www.w3.org/ns/shacl#Target> rdfs:isDefinedBy <http://www.w3.org/ns/shacl#> ;
                                    rdfs:label "Target"@en .


<http://www.w3.org/ns/shacl#TargetType> rdfs:isDefinedBy <http://www.w3.org/ns/shacl#> ;
                                        rdfs:label "Target type"@en .


<http://www.w3.org/ns/shacl#ValidationReport> rdfs:isDefinedBy <http://www.w3.org/ns/shacl#> ;
                                              rdfs:label "Validation report"@en .


<http://www.w3.org/ns/shacl#ValidationResult> rdfs:isDefinedBy <http://www.w3.org/ns/shacl#> ;
                                              rdfs:label "Validation result"@en .


<http://www.w3.org/ns/shacl#Validator> rdfs:isDefinedBy <http://www.w3.org/ns/shacl#> ;
                                       rdfs:label "Validator"@en .


<http://www.w3.org/ns/shacl#alternativePath> rdfs:isDefinedBy <http://www.w3.org/ns/shacl#> ;
                                             rdfs:label "alternative path"@en .


<http://www.w3.org/ns/shacl#and> rdfs:isDefinedBy <http://www.w3.org/ns/shacl#> ;
                                 rdfs:label "and"@en .


<http://www.w3.org/ns/shacl#annotationProperty> rdfs:isDefinedBy <http://www.w3.org/ns/shacl#> ;
                                                rdfs:label "annotation property"@en .


<http://www.w3.org/ns/shacl#annotationValue> rdfs:isDefinedBy <http://www.w3.org/ns/shacl#> ;
                                             rdfs:label "annotation value"@en .


<http://www.w3.org/ns/shacl#annotationVarName> rdfs:isDefinedBy <http://www.w3.org/ns/shacl#> ;
                                               rdfs:label "annotation variable name"@en .


<http://www.w3.org/ns/shacl#ask> rdfs:isDefinedBy <http://www.w3.org/ns/shacl#> ;
                                 rdfs:label "ask"@en .


<http://www.w3.org/ns/shacl#class> rdfs:isDefinedBy <http://www.w3.org/ns/shacl#> ;
                                   rdfs:label "class"@en .


<http://www.w3.org/ns/shacl#closed> rdfs:isDefinedBy <http://www.w3.org/ns/shacl#> ;
                                    rdfs:label "closed"@en .


<http://www.w3.org/ns/shacl#condition> rdfs:isDefinedBy <http://www.w3.org/ns/shacl#> ;
                                       rdfs:label "condition"@en .


<http://www.w3.org/ns/shacl#conforms> rdfs:isDefinedBy <http://www.w3.org/ns/shacl#> ;
                                      rdfs:label "conforms"@en .


<http://www.w3.org/ns/shacl#construct> rdfs:isDefinedBy <http://www.w3.org/ns/shacl#> ;
                                       rdfs:label "construct"@en .


<http://www.w3.org/ns/shacl#datatype> rdfs:isDefinedBy <http://www.w3.org/ns/shacl#> ;
                                      rdfs:label "datatype"@en .


<http://www.w3.org/ns/shacl#deactivated> rdfs:isDefinedBy <http://www.w3.org/ns/shacl#> ;
                                         rdfs:label "deactivated"@en .


<http://www.w3.org/ns/shacl#declare> rdfs:isDefinedBy <http://www.w3.org/ns/shacl#> ;
                                     rdfs:label "declare"@en .


<http://www.w3.org/ns/shacl#defaultValue> rdfs:isDefinedBy <http://www.w3.org/ns/shacl#> ;
                                          rdfs:label "default value"@en .


<http://www.w3.org/ns/shacl#description> rdfs:isDefinedBy <http://www.w3.org/ns/shacl#> ;
                                         rdfs:label "description"@en .


<http://www.w3.org/ns/shacl#detail> rdfs:isDefinedBy <http://www.w3.org/ns/shacl#> ;
                                    rdfs:label "detail"@en .


<http://www.w3.org/ns/shacl#disjoint> rdfs:isDefinedBy <http://www.w3.org/ns/shacl#> ;
                                      rdfs:label "disjoint"@en .


<http://www.w3.org/ns/shacl#entailment> rdfs:isDefinedBy <http://www.w3.org/ns/shacl#> ;
                                        rdfs:label "entailment"@en .


<http://www.w3.org/ns/shacl#equals> rdfs:isDefinedBy <http://www.w3.org/ns/shacl#> ;
                                    rdfs:label "equals"@en .


<http://www.w3.org/ns/shacl#filterShape> rdfs:isDefinedBy <http://www.w3.org/ns/shacl#> ;
                                         rdfs:label "filter shape"@en .


<http://www.w3.org/ns/shacl#flags> rdfs:isDefinedBy <http://www.w3.org/ns/shacl#> ;
                                   rdfs:label "flags"@en .


<http://www.w3.org/ns/shacl#focusNode> rdfs:isDefinedBy <http://www.w3.org/ns/shacl#> ;
                                       rdfs:label "focus node"@en .


<http://www.w3.org/ns/shacl#group> rdfs:isDefinedBy <http://www.w3.org/ns/shacl#> ;
                                   rdfs:label "group"@en .


<http://www.w3.org/ns/shacl#ignoredProperties> rdfs:isDefinedBy <http://www.w3.org/ns/shacl#> ;
                                               rdfs:label "ignored properties"@en .


<http://www.w3.org/ns/shacl#in> rdfs:isDefinedBy <http://www.w3.org/ns/shacl#> ;
                                rdfs:label "in"@en .


<http://www.w3.org/ns/shacl#inversePath> rdfs:isDefinedBy <http://www.w3.org/ns/shacl#> ;
                                         rdfs:label "inverse path"@en .


<http://www.w3.org/ns/shacl#js> rdfs:isDefinedBy <http://www.w3.org/ns/shacl#> ;
                                rdfs:label "JavaScript constraint"@en .


<http://www.w3.org/ns/shacl#jsFunctionName> rdfs:isDefinedBy <http://www.w3.org/ns/shacl#> ;
                                            rdfs:label "JavaScript function name"@en .


<http://www.w3.org/ns/shacl#jsLibrary> rdfs:isDefinedBy <http://www.w3.org/ns/shacl#> ;
                                       rdfs:label "JavaScript library"@en .


<http://www.w3.org/ns/shacl#jsLibraryURL> rdfs:isDefinedBy <http://www.w3.org/ns/shacl#> ;
                                          rdfs:label "JavaScript library URL"@en .


<http://www.w3.org/ns/shacl#labelTemplate> rdfs:isDefinedBy <http://www.w3.org/ns/shacl#> ;
                                           rdfs:label "label template"@en .


<http://www.w3.org/ns/shacl#languageIn> rdfs:isDefinedBy <http://www.w3.org/ns/shacl#> ;
                                        rdfs:label "language in"@en .


<http://www.w3.org/ns/shacl#lessThan> rdfs:isDefinedBy <http://www.w3.org/ns/shacl#> ;
                                      rdfs:label "less than"@en .


<http://www.w3.org/ns/shacl#lessThanOrEquals> rdfs:isDefinedBy <http://www.w3.org/ns/shacl#> ;
                                              rdfs:label "less than or equals"@en .


<http://www.w3.org/ns/shacl#maxCount> rdfs:isDefinedBy <http://www.w3.org/ns/shacl#> ;
                                      rdfs:label "max count"@en .


<http://www.w3.org/ns/shacl#maxLength> rdfs:isDefinedBy <http://www.w3.org/ns/shacl#> ;
                                       rdfs:label "max length"@en .


<http://www.w3.org/ns/shacl#minCount> rdfs:isDefinedBy <http://www.w3.org/ns/shacl#> ;
                                      rdfs:label "min count"@en .


<http://www.w3.org/ns/shacl#minLength> rdfs:isDefinedBy <http://www.w3.org/ns/shacl#> ;
                                       rdfs:label "min length"@en .


<http://www.w3.org/ns/shacl#name> rdfs:isDefinedBy <http://www.w3.org/ns/shacl#> ;
                                  rdfs:label "name"@en .


<http://www.w3.org/ns/shacl#namespace> rdfs:isDefinedBy <http://www.w3.org/ns/shacl#> ;
                                       rdfs:label "namespace"@en .


<http://www.w3.org/ns/shacl#node> rdfs:isDefinedBy <http://www.w3.org/ns/shacl#> ;
                                  rdfs:label "node"@en .


<http://www.w3.org/ns/shacl#nodeKind> rdfs:isDefinedBy <http://www.w3.org/ns/shacl#> ;
                                      rdfs:label "node kind"@en .


<http://www.w3.org/ns/shacl#nodeValidator> rdfs:isDefinedBy <http://www.w3.org/ns/shacl#> ;
                                           rdfs:label "shape validator"@en .


<http://www.w3.org/ns/shacl#not> rdfs:isDefinedBy <http://www.w3.org/ns/shacl#> ;
                                 rdfs:label "not"@en .


<http://www.w3.org/ns/shacl#object> rdfs:isDefinedBy <http://www.w3.org/ns/shacl#> ;
                                    rdfs:label "object"@en .


<http://www.w3.org/ns/shacl#oneOrMorePath> rdfs:isDefinedBy <http://www.w3.org/ns/shacl#> ;
                                           rdfs:label "one or more path"@en .


<http://www.w3.org/ns/shacl#optional> rdfs:isDefinedBy <http://www.w3.org/ns/shacl#> ;
                                      rdfs:label "optional"@en .


<http://www.w3.org/ns/shacl#or> rdfs:isDefinedBy <http://www.w3.org/ns/shacl#> ;
                                rdfs:label "or"@en .


<http://www.w3.org/ns/shacl#parameter> rdfs:isDefinedBy <http://www.w3.org/ns/shacl#> ;
                                       rdfs:label "parameter"@en .


<http://www.w3.org/ns/shacl#path> rdfs:isDefinedBy <http://www.w3.org/ns/shacl#> ;
                                  rdfs:label "path"@en .


<http://www.w3.org/ns/shacl#pattern> rdfs:isDefinedBy <http://www.w3.org/ns/shacl#> ;
                                     rdfs:label "pattern"@en .


<http://www.w3.org/ns/shacl#predicate> rdfs:isDefinedBy <http://www.w3.org/ns/shacl#> ;
                                       rdfs:label "predicate"@en .


<http://www.w3.org/ns/shacl#prefix> rdfs:isDefinedBy <http://www.w3.org/ns/shacl#> ;
                                    rdfs:label "prefix"@en .


<http://www.w3.org/ns/shacl#prefixes> rdfs:isDefinedBy <http://www.w3.org/ns/shacl#> ;
                                      rdfs:label "prefixes"@en .


<http://www.w3.org/ns/shacl#property> rdfs:isDefinedBy <http://www.w3.org/ns/shacl#> ;
                                      rdfs:label "property"@en .


<http://www.w3.org/ns/shacl#propertyValidator> rdfs:isDefinedBy <http://www.w3.org/ns/shacl#> ;
                                               rdfs:label "property validator"@en .


<http://www.w3.org/ns/shacl#qualifiedMaxCount> rdfs:isDefinedBy <http://www.w3.org/ns/shacl#> ;
                                               rdfs:label "qualified max count"@en .


<http://www.w3.org/ns/shacl#qualifiedMinCount> rdfs:isDefinedBy <http://www.w3.org/ns/shacl#> ;
                                               rdfs:label "qualified min count"@en .


<http://www.w3.org/ns/shacl#qualifiedValueShape> rdfs:isDefinedBy <http://www.w3.org/ns/shacl#> ;
                                                 rdfs:label "qualified value shape"@en .


<http://www.w3.org/ns/shacl#qualifiedValueShapesDisjoint> rdfs:isDefinedBy <http://www.w3.org/ns/shacl#> ;
                                                          rdfs:label "qualified value shapes disjoint"@en .


<http://www.w3.org/ns/shacl#result> rdfs:isDefinedBy <http://www.w3.org/ns/shacl#> ;
                                    rdfs:label "result"@en .


<http://www.w3.org/ns/shacl#resultAnnotation> rdfs:isDefinedBy <http://www.w3.org/ns/shacl#> ;
                                              rdfs:label "result annotation"@en .


<http://www.w3.org/ns/shacl#resultMessage> rdfs:isDefinedBy <http://www.w3.org/ns/shacl#> ;
                                           rdfs:label "result message"@en .


<http://www.w3.org/ns/shacl#resultPath> rdfs:isDefinedBy <http://www.w3.org/ns/shacl#> ;
                                        rdfs:label "result path"@en .


<http://www.w3.org/ns/shacl#resultSeverity> rdfs:isDefinedBy <http://www.w3.org/ns/shacl#> ;
                                            rdfs:label "result severity"@en .


<http://www.w3.org/ns/shacl#returnType> rdfs:isDefinedBy <http://www.w3.org/ns/shacl#> ;
                                        rdfs:label "return type"@en .


<http://www.w3.org/ns/shacl#rule> rdfs:isDefinedBy <http://www.w3.org/ns/shacl#> ;
                                  rdfs:label "rule"@en .


<http://www.w3.org/ns/shacl#select> rdfs:isDefinedBy <http://www.w3.org/ns/shacl#> ;
                                    rdfs:label "select"@en .


<http://www.w3.org/ns/shacl#severity> rdfs:isDefinedBy <http://www.w3.org/ns/shacl#> ;
                                      rdfs:label "severity"@en .


<http://www.w3.org/ns/shacl#shapesGraph> rdfs:isDefinedBy <http://www.w3.org/ns/shacl#> ;
                                         rdfs:label "shapes graph"@en .


<http://www.w3.org/ns/shacl#shapesGraphWellFormed> rdfs:isDefinedBy <http://www.w3.org/ns/shacl#> ;
                                                   rdfs:label "shapes graph well-formed"@en .


<http://www.w3.org/ns/shacl#sourceConstraint> rdfs:isDefinedBy <http://www.w3.org/ns/shacl#> ;
                                              rdfs:label "source constraint"@en .


<http://www.w3.org/ns/shacl#sourceConstraintComponent> rdfs:isDefinedBy <http://www.w3.org/ns/shacl#> ;
                                                       rdfs:label "source constraint component"@en .


<http://www.w3.org/ns/shacl#sourceShape> rdfs:isDefinedBy <http://www.w3.org/ns/shacl#> ;
                                         rdfs:label "source shape"@en .


<http://www.w3.org/ns/shacl#sparql> rdfs:isDefinedBy <http://www.w3.org/ns/shacl#> ;
                                    rdfs:label "constraint (in SPARQL)"@en .


<http://www.w3.org/ns/shacl#subject> rdfs:isDefinedBy <http://www.w3.org/ns/shacl#> ;
                                     rdfs:label "subject"@en .


<http://www.w3.org/ns/shacl#suggestedShapesGraph> rdfs:isDefinedBy <http://www.w3.org/ns/shacl#> ;
                                                  rdfs:label "suggested shapes graph"@en .


<http://www.w3.org/ns/shacl#target> rdfs:isDefinedBy <http://www.w3.org/ns/shacl#> ;
                                    rdfs:label "target"@en .


<http://www.w3.org/ns/shacl#targetClass> rdfs:isDefinedBy <http://www.w3.org/ns/shacl#> ;
                                         rdfs:label "target class"@en .


<http://www.w3.org/ns/shacl#targetNode> rdfs:isDefinedBy <http://www.w3.org/ns/shacl#> ;
                                        rdfs:label "target node"@en .


<http://www.w3.org/ns/shacl#targetObjectsOf> rdfs:isDefinedBy <http://www.w3.org/ns/shacl#> ;
                                             rdfs:label "target objects of"@en .


<http://www.w3.org/ns/shacl#targetSubjectsOf> rdfs:isDefinedBy <http://www.w3.org/ns/shacl#> ;
                                              rdfs:label "target subjects of"@en .


<http://www.w3.org/ns/shacl#uniqueLang> rdfs:isDefinedBy <http://www.w3.org/ns/shacl#> ;
                                        rdfs:label "unique languages"@en .


<http://www.w3.org/ns/shacl#update> rdfs:isDefinedBy <http://www.w3.org/ns/shacl#> ;
                                    rdfs:label "update"@en .


<http://www.w3.org/ns/shacl#validator> rdfs:isDefinedBy <http://www.w3.org/ns/shacl#> ;
                                       rdfs:label "validator"@en .


<http://www.w3.org/ns/shacl#value> rdfs:isDefinedBy <http://www.w3.org/ns/shacl#> ;
                                   rdfs:label "value"@en .


<http://www.w3.org/ns/shacl#xone> rdfs:isDefinedBy <http://www.w3.org/ns/shacl#> ;
                                  rdfs:label "exactly one"@en .


<http://www.w3.org/ns/shacl#zeroOrMorePath> rdfs:isDefinedBy <http://www.w3.org/ns/shacl#> ;
                                            rdfs:label "zero or more path"@en .


<http://www.w3.org/ns/shacl#zeroOrOnePath> rdfs:isDefinedBy <http://www.w3.org/ns/shacl#> ;
                                           rdfs:label "zero or one path"@en .


:Allocation <http://www.w3.org/2004/02/skos/core#definition> "An explicit relation between subject and requirement that shows that the subject needs to fulfill the stated requirement."@en .


:Decision <http://www.w3.org/2004/02/skos/core#definition> "A decision is an activity of making a choice or judgement based on the available resources."@en .


:Document <http://www.w3.org/2004/02/skos/core#definition> "A piece of written, printed, or electronic matter that provides information or evidence or that serves as an official record or acts as a reference."@en .


:GenericRequirement <http://www.w3.org/2004/02/skos/core#definition> "A requirement that is not specific for any projects / use case."@en .


:MachineReadableRule <http://www.w3.org/2004/02/skos/core#definition> "A set of instructions or guidelines that are structured in a format that can be easily interpreted and processed by a computer or software program. The term \"rule\" refers here to checking rules specifically and is not to be confused with inferencing rules for deriving knowledge."@en .


:Parcel <http://www.w3.org/2004/02/skos/core#definition> "Any quantity of land capable of being described with such definiteness that its locations and boundaries may be established."@en .


:Permit <http://www.w3.org/2004/02/skos/core#definition> "A permit is a written permission or authorisation delivered by a competent authority, entity, or person, that is legally delegated to allow someone to do something or to go somewhere."@en .


:PermitRequest <http://www.w3.org/2004/02/skos/core#definition> "A permit request is a written appeal or application made to obtain official approval for something from a designated authority."@en .


:Project <http://www.w3.org/2004/02/skos/core#definition> "A temporary process undertaken to solve a well-defined goal or objective with clearly defined start and end times, a set of clearly defined tasks, and a budget."@en .


:ProjectRequirement <http://www.w3.org/2004/02/skos/core#definition> "A requirement that is specific to projects / use case. It cannot be generalized over multiple projects / use cases."@en .


:Verification <http://www.w3.org/2004/02/skos/core#definition> "A Verification is an activity that checks if a subject is compliant with a requirement."@en .


:VerificationMethod <http://www.w3.org/2004/02/skos/core#definition> "A set of procedures to check if the subject is compliant with requirement."@en .


:decisionOutcome <http://www.w3.org/2004/02/skos/core#definition> "Provides a list of possible decision outcomes which impact the permit request."@en .


:hasAsOutput <http://www.w3.org/2004/02/skos/core#definition> "Is an involvement in an occurrence that indicates that the involved object has been operated upon by the occurrence."@en .


:hasParcel <http://www.w3.org/2004/02/skos/core#definition> "Indicates the link between location and parcel."@en .


:hasPermitRequest <http://www.w3.org/2004/02/skos/core#definition> "Indicates the link from a project to a / multiple permit requests."@en .


:hasSource <http://www.w3.org/2004/02/skos/core#definition> "Is a relation that indicates the involved object has a origin or source from another object."@en .


:hasVerificationMethod <http://www.w3.org/2004/02/skos/core#definition> "Is an association that indicates a method to verify if the verification object has a method linked to it."@en .


:isAddressFor <http://www.w3.org/2004/02/skos/core#definition> "Relation to check if the address is linked to a location."@en .


:isAllocationfor <http://www.w3.org/2004/02/skos/core#definition> "Is an association to ensure that the involved object has an allocation to the corresponding requirement."@en .


:isCollectedIn <http://www.w3.org/2004/02/skos/core#definition> "Is a relation between a single thing and a plurality that indicates that the collected object is element of the collection of objects, under the constraint that the element may not be the same object as the plural object. In other words a collection cannot be an element of itself."@en .


:isControlledBy <http://www.w3.org/2004/02/skos/core#definition> "Is an involvement in an occurrence that indicates that the involved object has a role as controller of the occurrence."@en .


:isDecisionFor <http://www.w3.org/2004/02/skos/core#definition> "Is a relation indicating the choice or judgment made based on available resources."@en .


:isDerivedIn <http://www.w3.org/2004/02/skos/core#definition> "Is an association that indicates that the object has been derived in the source object."@en .


:isExpressedAs <http://www.w3.org/2004/02/skos/core#definition> "Is a relation that determines how an object is represented similar to a target object"@en .


:isGeometryOf <http://www.w3.org/2004/02/skos/core#definition> "Indicates that a geometry has a location linked to it."@en .


:isInputFor <http://www.w3.org/2004/02/skos/core#definition> "Indicates that a / multiple verifications where carried out as a foundation for certain decision taken."@en .


:isMadeBy <http://www.w3.org/2004/02/skos/core#definition> "Is an involvement in an occurrence that indicates that the involved object has a role as performer of the occurrence."@en .


:isParcelFor <http://www.w3.org/2004/02/skos/core#definition> "Indicates that a parcel is located at a certain location."@en .


:isPermitFor <http://www.w3.org/2004/02/skos/core#definition> "Indicates the link between a permit and corresponding permit request that are / were made to obtain certain permit"@en .


:isPermitForRequest <http://www.w3.org/2004/02/skos/core#definition> "Indicates the relation between a permit and the related request for it"@en .


:isRequestForPermit <http://www.w3.org/2004/02/skos/core#definition> "Indicates the relation between a request and the specific permit it was requesting."@en .


:isSubmittedBy <http://www.w3.org/2004/02/skos/core#definition> "Indicates that a permit request was made by appropriate associated person / organization that is authorized to make the specific request."@en .


:isVerifiedIn <http://www.w3.org/2004/02/skos/core#definition> "Is an association that indicates that the representer object represents the represented object."@en .


:logicalOperator <http://www.w3.org/2004/02/skos/core#definition> "Provides the possibility to indicate if certain conditions are complementary (AND) or supplementary (OR)."@en .


:role <http://www.w3.org/2004/02/skos/core#definition> "Indicates in what capacity someone/something is linked to a project, permit, ..."@en .


:shallBeCompliantWith <http://www.w3.org/2004/02/skos/core#definition> "Is a conceptual requirement for compliancy to a criterion that indicates that a member of the class shall be conformant to a qualitative requirement. Typically an item, story or document of a kind that should be conform to the content of a document."@en .


:wasDescribedBy <http://www.w3.org/2004/02/skos/core#definition> "Relation that is used to indicate that a concept was linked to certain resource in the past. this is meant to keep track of different versions of resources, keep history on all links ever made from concept to resource."@en .


<https://w3id.org/sml/def#Requirement> <http://www.w3.org/2004/02/skos/core#definition> "A rule that should hold for something, defined via its attributes or relations"@en .


<https://w3id.org/sml/def#isDescribedBy> <http://www.w3.org/2004/02/skos/core#definition> "Relation that is used to link various concepts to a resource. Many concepts require to be linked to certain proof documents / descriptions. This relation is set on Top Concept level."@en .


###  Generated by the OWL API (version 5.1.18) https://github.com/owlcs/owlapi/
